
{
    "@context": {
        "unece": "https://service.unece.org/trade/uncefact/vocabulary/unece#",
        "rdf": "http://www.w3.org/1999/02/22-rdf-syntax-ns#",
        "rdfs": "http://www.w3.org/2000/01/rdf-schema#",
        "schema": "http://schema.org/",
        "fisheries": "https://service.unece.org/trade/uncefact/vocabulary/unece/fisheries#",
        "cefact": "https://service.unece.org/trade/uncefact/vocabulary/cefact#",
        "xsd": "http://www.w3.org/2001/XMLSchema#"
    },
    "@graph": [
        {
            "@id": "fisheries:ACDRReport",
            "@type": "rdfs:Class",
            "rdfs:comment": "Information contained in a Fisheries Language for Universal eXchange (FLUX) Aggregated Catch Data Report (ACDR) report.",
            "rdfs:label": "ACDRReport",
            "unece:cefactElementMetadata": [
                {
                    "@id": "cefact:FLUX_ACDRReport.Details",
                    "@type": "unece:AggregateBIE",
                    "unece:cefactUNId": "UN01010269",
                    "rdfs:comment": "Information contained in a Fisheries Language for Universal eXchange (FLUX) Aggregated Catch Data Report (ACDR) report."
                }
            ]
        },
        {
            "@id": "fisheries:Activity",
            "@type": "rdfs:Class",
            "rdfs:comment": "An action taken by a person or group during a fishing trip.",
            "rdfs:label": "Activity",
            "unece:cefactElementMetadata": [
                {
                    "@id": "cefact:Fishing_Activity.Details",
                    "@type": "unece:AggregateBIE",
                    "unece:cefactUNId": "UN01011168",
                    "rdfs:comment": "An action taken by a person or group during a fishing trip."
                }
            ]
        },
        {
            "@id": "fisheries:Batch",
            "@type": "rdfs:Class",
            "rdfs:comment": "A group of products dealt with together for selling.",
            "rdfs:label": "Batch",
            "unece:cefactElementMetadata": [
                {
                    "@id": "cefact:Sales_Batch.Details",
                    "@type": "unece:AggregateBIE",
                    "unece:cefactUNId": "UN01010929",
                    "rdfs:comment": "A group of products dealt with together for selling."
                }
            ]
        },
        {
            "@id": "fisheries:BinaryFile",
            "@type": "rdfs:Class",
            "rdfs:comment": "A computer file stored in a binary format used in the Fisheries Language for Universal eXchange (FLUX).",
            "rdfs:label": "BinaryFile",
            "unece:cefactElementMetadata": [
                {
                    "@id": "cefact:FLUX_BinaryFile.Details",
                    "@type": "unece:AggregateBIE",
                    "unece:cefactUNId": "UN01010799",
                    "rdfs:comment": "A computer file stored in a binary format used in the Fisheries Language for Universal eXchange (FLUX)."
                }
            ]
        },
        {
            "@id": "fisheries:Catch",
            "@type": "rdfs:Class",
            "rdfs:comment": [
                "Fishing Activity (FA) information about the species and quantity of an aquatic animal or plant.",
                "Aggregated Catch Data Report (ACDR) information about the species and quantity of fish caught."
            ],
            "rdfs:label": "Catch",
            "unece:cefactElementMetadata": [
                {
                    "@id": "cefact:ACDR_Catch.Details",
                    "@type": "unece:AggregateBIE",
                    "unece:cefactUNId": "UN01010264",
                    "rdfs:comment": "Aggregated Catch Data Report (ACDR) information about the species and quantity of fish caught."
                },
                {
                    "@id": "cefact:FA_Catch.Details",
                    "@type": "unece:AggregateBIE",
                    "unece:cefactUNId": "UN01010971",
                    "rdfs:comment": "Fishing Activity (FA) information about the species and quantity of an aquatic animal or plant."
                }
            ]
        },
        {
            "@id": "fisheries:Category",
            "@type": "rdfs:Class",
            "rdfs:comment": "A division of fishing sharing characteristics, such as a type of vessel, a type of fishing activity or a type of fishing gear deployed.",
            "rdfs:label": "Category",
            "unece:cefactElementMetadata": [
                {
                    "@id": "cefact:Fishing_Category.Details",
                    "@type": "unece:AggregateBIE",
                    "unece:cefactUNId": "UN01010837",
                    "rdfs:comment": "A division of fishing sharing characteristics, such as a type of vessel, a type of fishing activity or a type of fishing gear deployed."
                }
            ]
        },
        {
            "@id": "fisheries:Characteristic",
            "@type": "rdfs:Class",
            "rdfs:comment": [
                "A prominent attribute or aspect related to a gear.",
                "An attribute or aspect of an item or object related to an Inspection or Surveillance Report (ISR), such as an indicator specifying whether a Fishing Logbook is completed.",
                "A prominent attribute or aspect of a fish catch.",
                "A prominent technical attribute or aspect related to a particular vessel, such as the speed or hull material.",
                "A prominent attribute or aspect of equipment related to a particular vessel.",
                "A prominent attribute or aspect of an administrative decision related to a vessel.",
                "A prominent attribute or aspect of the history related to a particular vessel.",
                "A prominent attribute or aspect related to the storage in a particular vessel.",
                "A prominent attribute or aspect of a Fisheries Language for Universal eXchange (FLUX) element."
            ],
            "rdfs:label": "Characteristic",
            "unece:cefactElementMetadata": [
                {
                    "@id": "cefact:VesselEquipment_Characteristic.Details",
                    "@type": "unece:AggregateBIE",
                    "unece:cefactUNId": "UN01010692",
                    "rdfs:comment": "A prominent attribute or aspect of equipment related to a particular vessel."
                },
                {
                    "@id": "cefact:Gear_Characteristic.Details",
                    "@type": "unece:AggregateBIE",
                    "unece:cefactUNId": "UN01010819",
                    "rdfs:comment": "A prominent attribute or aspect related to a gear."
                },
                {
                    "@id": "cefact:ISRItem_Characteristic.Details",
                    "@type": "unece:AggregateBIE",
                    "unece:cefactUNId": "UN01012602",
                    "rdfs:comment": "An attribute or aspect of an item or object related to an Inspection or Surveillance Report (ISR), such as an indicator specifying whether a Fishing Logbook is completed."
                },
                {
                    "@id": "cefact:VesselAdministrative_Characteristic.Details",
                    "@type": "unece:AggregateBIE",
                    "unece:cefactUNId": "UN01010700",
                    "rdfs:comment": "A prominent attribute or aspect of an administrative decision related to a vessel."
                },
                {
                    "@id": "cefact:FishCatch_Characteristic.Details",
                    "@type": "unece:AggregateBIE",
                    "unece:cefactUNId": "UN01011282",
                    "rdfs:comment": "A prominent attribute or aspect of a fish catch."
                },
                {
                    "@id": "cefact:VesselHistorical_Characteristic.Details",
                    "@type": "unece:AggregateBIE",
                    "unece:cefactUNId": "UN01010650",
                    "rdfs:comment": "A prominent attribute or aspect of the history related to a particular vessel."
                },
                {
                    "@id": "cefact:VesselStorage_Characteristic.Details",
                    "@type": "unece:AggregateBIE",
                    "unece:cefactUNId": "UN01010806",
                    "rdfs:comment": "A prominent attribute or aspect related to the storage in a particular vessel."
                },
                {
                    "@id": "cefact:FLUX_Characteristic.Details",
                    "@type": "unece:AggregateBIE",
                    "unece:cefactUNId": "UN01010865",
                    "rdfs:comment": "A prominent attribute or aspect of a Fisheries Language for Universal eXchange (FLUX) element."
                },
                {
                    "@id": "cefact:VesselTechnical_Characteristic.Details",
                    "@type": "unece:AggregateBIE",
                    "unece:cefactUNId": "UN01010789",
                    "rdfs:comment": "A prominent technical attribute or aspect related to a particular vessel, such as the speed or hull material."
                }
            ]
        },
        {
            "@id": "fisheries:Country",
            "@type": "rdfs:Class",
            "rdfs:comment": "A country associated to a vessel.",
            "rdfs:label": "Country",
            "unece:cefactElementMetadata": [
                {
                    "@id": "cefact:Vessel_Country.Details",
                    "@type": "unece:AggregateBIE",
                    "unece:cefactUNId": "UN01010231",
                    "rdfs:comment": "A country associated to a vessel."
                }
            ]
        },
        {
            "@id": "fisheries:Crew",
            "@type": "rdfs:Class",
            "rdfs:comment": "A group of people who work on or operate a vessel.",
            "rdfs:label": "Crew",
            "unece:cefactElementMetadata": [
                {
                    "@id": "cefact:Vessel_Crew.Details",
                    "@type": "unece:AggregateBIE",
                    "unece:cefactUNId": "UN01010812",
                    "rdfs:comment": "A group of people who work on or operate a vessel."
                }
            ]
        },
        {
            "@id": "fisheries:DataNode",
            "@type": "rdfs:Class",
            "rdfs:comment": [
                "A single element or node within a Master Data Register (MDR) data structure, usually a hierarchical structure.",
                "An element which is part of a Master Data Register (MDR) node."
            ],
            "rdfs:label": "DataNode",
            "unece:cefactElementMetadata": [
                {
                    "@id": "cefact:MDRElement_DataNode.Details",
                    "@type": "unece:AggregateBIE",
                    "unece:cefactUNId": "UN01010595",
                    "rdfs:comment": "An element which is part of a Master Data Register (MDR) node."
                },
                {
                    "@id": "cefact:MDR_DataNode.Details",
                    "@type": "unece:AggregateBIE",
                    "unece:cefactUNId": "UN01010589",
                    "rdfs:comment": "A single element or node within a Master Data Register (MDR) data structure, usually a hierarchical structure."
                }
            ]
        },
        {
            "@id": "fisheries:DataSet",
            "@type": "rdfs:Class",
            "rdfs:comment": "A collection of data provided from a Master Data Register (MDR).",
            "rdfs:label": "DataSet",
            "unece:cefactElementMetadata": [
                {
                    "@id": "cefact:MDR_DataSet.Details",
                    "@type": "unece:AggregateBIE",
                    "unece:cefactUNId": "UN01010582",
                    "rdfs:comment": "A collection of data provided from a Master Data Register (MDR)."
                }
            ]
        },
        {
            "@id": "fisheries:Dimension",
            "@type": "rdfs:Class",
            "rdfs:comment": "A measure of length, tonnage, depth or breadth, expressed as type and value, for this vessel.",
            "rdfs:label": "Dimension",
            "unece:cefactElementMetadata": [
                {
                    "@id": "cefact:Vessel_Dimension.Details",
                    "@type": "unece:AggregateBIE",
                    "unece:cefactUNId": "UN01010689",
                    "rdfs:comment": "A measure of length, tonnage, depth or breadth, expressed as type and value, for this vessel."
                }
            ]
        },
        {
            "@id": "fisheries:Distribution",
            "@type": "rdfs:Class",
            "rdfs:comment": "A way based on the size of something which is shared out among a group, spread over an area or arranged in a box.",
            "rdfs:label": "Distribution",
            "unece:cefactElementMetadata": [
                {
                    "@id": "cefact:Size_Distribution.Details",
                    "@type": "unece:AggregateBIE",
                    "unece:cefactUNId": "UN01011152",
                    "rdfs:comment": "A way based on the size of something which is shared out among a group, spread over an area or arranged in a box."
                }
            ]
        },
        {
            "@id": "fisheries:Document",
            "@type": "rdfs:Class",
            "rdfs:comment": [
                "A document that provides information for a Fishing Licence, Authorization, Permit (FLAP) request.",
                "A collection of data for a piece of written, printed or electronic matter that is exchanged between two or more parties in every aggregated catch report.",
                "A document that provides information for a Fisheries Language for Universal eXchange (FLUX) report.",
                "A document that provides information for a Fishing Licence, Authorization, Permit (FLAP), primarily for a vessel.",
                "A document that provides information for a Fishing Activity (FA) report.",
                "The response to a received Fisheries Language for Universal eXchange FLUX document.",
                "A document that provides information for a specific sale or sales.",
                "A collection of data that reports information or evidence of a validation."
            ],
            "rdfs:label": "Document",
            "unece:cefactElementMetadata": [
                {
                    "@id": "cefact:FLAP_Document.Details",
                    "@type": "unece:AggregateBIE",
                    "unece:cefactUNId": "UN01010845",
                    "rdfs:comment": "A document that provides information for a Fishing Licence, Authorization, Permit (FLAP), primarily for a vessel."
                },
                {
                    "@id": "cefact:FLUXResponse_Document.Details",
                    "@type": "unece:AggregateBIE",
                    "unece:cefactUNId": "UN01010248",
                    "rdfs:comment": "The response to a received Fisheries Language for Universal eXchange FLUX document."
                },
                {
                    "@id": "cefact:AggregatedCatchReport_Document.Details",
                    "@type": "unece:AggregateBIE",
                    "unece:cefactUNId": "UN01010255",
                    "rdfs:comment": "A collection of data for a piece of written, printed or electronic matter that is exchanged between two or more parties in every aggregated catch report."
                },
                {
                    "@id": "cefact:FAReport_Document.Details",
                    "@type": "unece:AggregateBIE",
                    "unece:cefactUNId": "UN01011156",
                    "rdfs:comment": "A document that provides information for a Fishing Activity (FA) report."
                },
                {
                    "@id": "cefact:FLUXReport_Document.Details",
                    "@type": "unece:AggregateBIE",
                    "unece:cefactUNId": "UN01010238",
                    "rdfs:comment": "A document that provides information for a Fisheries Language for Universal eXchange (FLUX) report."
                },
                {
                    "@id": "cefact:Sales_Document.Details",
                    "@type": "unece:AggregateBIE",
                    "unece:cefactUNId": "UN01010909",
                    "rdfs:comment": "A document that provides information for a specific sale or sales."
                },
                {
                    "@id": "cefact:FLAPRequest_Document.Details",
                    "@type": "unece:AggregateBIE",
                    "unece:cefactUNId": "UN01010829",
                    "rdfs:comment": "A document that provides information for a Fishing Licence, Authorization, Permit (FLAP) request."
                },
                {
                    "@id": "cefact:ValidationResult_Document.Details",
                    "@type": "unece:AggregateBIE",
                    "unece:cefactUNId": "UN01010750",
                    "rdfs:comment": "A collection of data that reports information or evidence of a validation."
                }
            ]
        },
        {
            "@id": "fisheries:Engine",
            "@type": "rdfs:Class",
            "rdfs:comment": "An engine which is used to move a ship or boat.",
            "rdfs:label": "Engine",
            "unece:cefactElementMetadata": [
                {
                    "@id": "cefact:Vessel_Engine.Details",
                    "@type": "unece:AggregateBIE",
                    "unece:cefactUNId": "UN01010717",
                    "rdfs:comment": "An engine which is used to move a ship or boat."
                }
            ]
        },
        {
            "@id": "fisheries:Equipment",
            "@type": "rdfs:Class",
            "rdfs:comment": "A necessary item or object fixed to a fishing gear for a particular purpose.",
            "rdfs:label": "Equipment",
            "unece:cefactElementMetadata": [
                {
                    "@id": "cefact:FishingGear_Equipment.Details",
                    "@type": "unece:AggregateBIE",
                    "unece:cefactUNId": "UN01012657",
                    "rdfs:comment": "A necessary item or object fixed to a fishing gear for a particular purpose."
                }
            ]
        },
        {
            "@id": "fisheries:Event",
            "@type": "rdfs:Class",
            "rdfs:comment": [
                "A significant occurrence or happening related to a vessel.",
                "A significant occurrence or happening related to an inspection of a gear or gear attachment.",
                "A significant occurrence or happening related to an inspection of a gear.",
                "A significant occurrence or happening related to a sales activity or sales business.",
                "A significant occurrence or happening related to an Inspection or Surveillance (IS) operation.",
                "Information obtained related to the position of a vessel."
            ],
            "rdfs:label": "Event",
            "unece:cefactElementMetadata": [
                {
                    "@id": "cefact:GearEquipmentInspection_Event.Details",
                    "@type": "unece:AggregateBIE",
                    "unece:cefactUNId": "UN01013329",
                    "rdfs:comment": "A significant occurrence or happening related to an inspection of a gear or gear attachment."
                },
                {
                    "@id": "cefact:Vessel_Event.Details",
                    "@type": "unece:AggregateBIE",
                    "unece:cefactUNId": "UN01010658",
                    "rdfs:comment": "A significant occurrence or happening related to a vessel."
                },
                {
                    "@id": "cefact:GearInspection_Event.Details",
                    "@type": "unece:AggregateBIE",
                    "unece:cefactUNId": "UN01012623",
                    "rdfs:comment": "A significant occurrence or happening related to an inspection of a gear."
                },
                {
                    "@id": "cefact:IS_Event.Details",
                    "@type": "unece:AggregateBIE",
                    "unece:cefactUNId": "UN01012613",
                    "rdfs:comment": "A significant occurrence or happening related to an Inspection or Surveillance (IS) operation."
                },
                {
                    "@id": "cefact:Sales_Event.Details",
                    "@type": "unece:AggregateBIE",
                    "unece:cefactUNId": "UN01010947",
                    "rdfs:comment": "A significant occurrence or happening related to a sales activity or sales business."
                },
                {
                    "@id": "cefact:VesselPosition_Event.Details",
                    "@type": "unece:AggregateBIE",
                    "unece:cefactUNId": "UN01010233",
                    "rdfs:comment": "Information obtained related to the position of a vessel."
                }
            ]
        },
        {
            "@id": "fisheries:Gear",
            "@type": "rdfs:Class",
            "rdfs:comment": "An apparatus which is used for fishing.",
            "rdfs:label": "Gear",
            "unece:cefactElementMetadata": [
                {
                    "@id": "cefact:Fishing_Gear.Details",
                    "@type": "unece:AggregateBIE",
                    "unece:cefactUNId": "UN01010726",
                    "rdfs:comment": "An apparatus which is used for fishing."
                }
            ]
        },
        {
            "@id": "fisheries:GeographicalCoordinate",
            "@type": "rdfs:Class",
            "rdfs:comment": [
                "The latitude, longitude and altitude of a specified place, by which a Fisheries Language for Universal eXchange (FLUX) relative situation on the globe is known.",
                "The latitude and longitude of a specified place, by which a vessel's relative situation on the globe is known. The height above the sea level constitutes a third coordinate."
            ],
            "rdfs:label": "GeographicalCoordinate",
            "unece:cefactElementMetadata": [
                {
                    "@id": "cefact:Vessel_GeographicalCoordinate.Details",
                    "@type": "unece:AggregateBIE",
                    "unece:cefactUNId": "UN01010221",
                    "rdfs:comment": "The latitude and longitude of a specified place, by which a vessel's relative situation on the globe is known. The height above the sea level constitutes a third coordinate."
                },
                {
                    "@id": "cefact:FLUX_GeographicalCoordinate.Details",
                    "@type": "unece:AggregateBIE",
                    "unece:cefactUNId": "UN01010966",
                    "rdfs:comment": "The latitude, longitude and altitude of a specified place, by which a Fisheries Language for Universal eXchange (FLUX) relative situation on the globe is known."
                }
            ]
        },
        {
            "@id": "fisheries:Identity",
            "@type": "rdfs:Class",
            "rdfs:comment": [
                "Information which uniquely identifies a Fishing License, Authorization, Permit (FLAP) object.",
                "Information which uniquely identifies a Master Data Register (MDR) Query object.",
                "Information which uniquely identifies a vessel."
            ],
            "rdfs:label": "Identity",
            "unece:cefactElementMetadata": [
                {
                    "@id": "cefact:MDRQuery_Identity.Details",
                    "@type": "unece:AggregateBIE",
                    "unece:cefactUNId": "UN01010577",
                    "rdfs:comment": "Information which uniquely identifies a Master Data Register (MDR) Query object."
                },
                {
                    "@id": "cefact:Vessel_Identity.Details",
                    "@type": "unece:AggregateBIE",
                    "unece:cefactUNId": "UN01010743",
                    "rdfs:comment": "Information which uniquely identifies a vessel."
                },
                {
                    "@id": "cefact:FLAP_Identity.Details",
                    "@type": "unece:AggregateBIE",
                    "unece:cefactUNId": "UN01010894",
                    "rdfs:comment": "Information which uniquely identifies a Fishing License, Authorization, Permit (FLAP) object."
                }
            ]
        },
        {
            "@id": "fisheries:Location",
            "@type": "rdfs:Class",
            "rdfs:comment": "A physical location or place defined for Fisheries Language for Universal eXchange (FLUX), such as a port or a region at sea.",
            "rdfs:label": "Location",
            "unece:cefactElementMetadata": [
                {
                    "@id": "cefact:FLUX_Location.Details",
                    "@type": "unece:AggregateBIE",
                    "unece:cefactUNId": "UN01010959",
                    "rdfs:comment": "A physical location or place defined for Fisheries Language for Universal eXchange (FLUX), such as a port or a region at sea."
                }
            ]
        },
        {
            "@id": "fisheries:Means",
            "@type": "rdfs:Class",
            "rdfs:comment": "A method or object, such as an aircraft or radar, used for achieving a surveillance operation.",
            "rdfs:label": "Means",
            "unece:cefactElementMetadata": [
                {
                    "@id": "cefact:Surveillance_Means.Details",
                    "@type": "unece:AggregateBIE",
                    "unece:cefactUNId": "UN01012629",
                    "rdfs:comment": "A method or object, such as an aircraft or radar, used for achieving a surveillance operation."
                }
            ]
        },
        {
            "@id": "fisheries:Organization",
            "@type": "rdfs:Class",
            "rdfs:comment": "An organization, such as a business or government body, that participates in a Fisheries Language for Universal eXchange (FLUX) process.",
            "rdfs:label": "Organization",
            "unece:cefactElementMetadata": [
                {
                    "@id": "cefact:FLUX_Organization.Details",
                    "@type": "unece:AggregateBIE",
                    "unece:cefactUNId": "UN01010984",
                    "rdfs:comment": "An organization, such as a business or government body, that participates in a Fisheries Language for Universal eXchange (FLUX) process."
                }
            ]
        },
        {
            "@id": "fisheries:Party",
            "@type": "rdfs:Class",
            "rdfs:comment": [
                "An individual, a group, or a body having a role in a sales business function.",
                "An individual, a group, or a body having a role in a Fisheries Language for Universal eXchange (FLUX) business function. Party has a legal connotation in a business transaction."
            ],
            "rdfs:label": "Party",
            "unece:cefactElementMetadata": [
                {
                    "@id": "cefact:Sales_Party.Details",
                    "@type": "unece:AggregateBIE",
                    "unece:cefactUNId": "UN01010922",
                    "rdfs:comment": "An individual, a group, or a body having a role in a sales business function."
                },
                {
                    "@id": "cefact:FLUX_Party.Details",
                    "@type": "unece:AggregateBIE",
                    "unece:cefactUNId": "UN01010245",
                    "rdfs:comment": "An individual, a group, or a body having a role in a Fisheries Language for Universal eXchange (FLUX) business function. Party has a legal connotation in a business transaction."
                }
            ]
        },
        {
            "@id": "fisheries:Picture",
            "@type": "rdfs:Class",
            "rdfs:comment": "A picture, such as a digital photograph, used in the context of Fisheries Languages for Universal eXchange (FLUX).",
            "rdfs:label": "Picture",
            "unece:cefactElementMetadata": [
                {
                    "@id": "cefact:FLUX_Picture.Details",
                    "@type": "unece:AggregateBIE",
                    "unece:cefactUNId": "UN01010729",
                    "rdfs:comment": "A picture, such as a digital photograph, used in the context of Fisheries Languages for Universal eXchange (FLUX)."
                }
            ]
        },
        {
            "@id": "fisheries:Price",
            "@type": "rdfs:Class",
            "rdfs:comment": "A sum of money for which something is or may be sold.",
            "rdfs:label": "Price",
            "unece:cefactElementMetadata": [
                {
                    "@id": "cefact:Sales_Price.Details",
                    "@type": "unece:AggregateBIE",
                    "unece:cefactUNId": "UN01010945",
                    "rdfs:comment": "A sum of money for which something is or may be sold."
                }
            ]
        },
        {
            "@id": "fisheries:Problem",
            "@type": "rdfs:Class",
            "rdfs:comment": "A matter or situation regarded as unwelcome or harmful which occurred on a gear, such as a lost fishing gear.",
            "rdfs:label": "Problem",
            "unece:cefactElementMetadata": [
                {
                    "@id": "cefact:Gear_Problem.Details",
                    "@type": "unece:AggregateBIE",
                    "unece:cefactUNId": "UN01011208",
                    "rdfs:comment": "A matter or situation regarded as unwelcome or harmful which occurred on a gear, such as a lost fishing gear."
                }
            ]
        },
        {
            "@id": "fisheries:Process",
            "@type": "rdfs:Class",
            "rdfs:comment": "A designed sequence of operations applied on Aquatic Animal or Plants (AAP).",
            "rdfs:label": "Process",
            "unece:cefactElementMetadata": [
                {
                    "@id": "cefact:AAP_Process.Details",
                    "@type": "unece:AggregateBIE",
                    "unece:cefactUNId": "UN01010942",
                    "rdfs:comment": "A designed sequence of operations applied on Aquatic Animal or Plants (AAP)."
                }
            ]
        },
        {
            "@id": "fisheries:Product",
            "@type": "rdfs:Class",
            "rdfs:comment": "An Aquatic Animals or Plants (AAP) output produced by human or mechanical effort or by a natural process.",
            "rdfs:label": "Product",
            "unece:cefactElementMetadata": [
                {
                    "@id": "cefact:AAP_Product.Details",
                    "@type": "unece:AggregateBIE",
                    "unece:cefactUNId": "UN01010933",
                    "rdfs:comment": "An Aquatic Animals or Plants (AAP) output produced by human or mechanical effort or by a natural process."
                }
            ]
        },
        {
            "@id": "fisheries:QualityAnalysis",
            "@type": "rdfs:Class",
            "rdfs:comment": "The data that demonstrate conclusively whether or not the validation process meets a requirement.",
            "rdfs:label": "QualityAnalysis",
            "unece:cefactElementMetadata": [
                {
                    "@id": "cefact:Validation_QualityAnalysis.Details",
                    "@type": "unece:AggregateBIE",
                    "unece:cefactUNId": "UN01010754",
                    "rdfs:comment": "The data that demonstrate conclusively whether or not the validation process meets a requirement."
                }
            ]
        },
        {
            "@id": "fisheries:Query",
            "@type": "rdfs:Class",
            "rdfs:comment": [
                "A formally raised question or request for information about a vessel.",
                "A formally raised question or request for Master Data Register (MDR) information.",
                "A formally raised question or request for information about an Inspection and/or Surveillance Report (ISR).",
                "A formally raised question or request for Fishing Licence, Authorization, Permit (FLAP) information.",
                "A formally raised question or request for information for a Fishing Activity (FA) report document.",
                "A formally raised question or request for vessel position information.",
                "A formally raised question or request for information related to a sale, such as for a sales note, takeover or transport document."
            ],
            "rdfs:label": "Query",
            "unece:cefactElementMetadata": [
                {
                    "@id": "cefact:VesselPosition_Query.Details",
                    "@type": "unece:AggregateBIE",
                    "unece:cefactUNId": "UN01012646",
                    "rdfs:comment": "A formally raised question or request for vessel position information."
                },
                {
                    "@id": "cefact:ISR_Query.Details",
                    "@type": "unece:AggregateBIE",
                    "unece:cefactUNId": "UN01012634",
                    "rdfs:comment": "A formally raised question or request for information about an Inspection and/or Surveillance Report (ISR)."
                },
                {
                    "@id": "cefact:FLAP_Query.Details",
                    "@type": "unece:AggregateBIE",
                    "unece:cefactUNId": "UN01010887",
                    "rdfs:comment": "A formally raised question or request for Fishing Licence, Authorization, Permit (FLAP) information."
                },
                {
                    "@id": "cefact:FA_Query.Details",
                    "@type": "unece:AggregateBIE",
                    "unece:cefactUNId": "UN01011217",
                    "rdfs:comment": "A formally raised question or request for information for a Fishing Activity (FA) report document."
                },
                {
                    "@id": "cefact:Sales_Query.Details",
                    "@type": "unece:AggregateBIE",
                    "unece:cefactUNId": "UN01010993",
                    "rdfs:comment": "A formally raised question or request for information related to a sale, such as for a sales note, takeover or transport document."
                },
                {
                    "@id": "cefact:MDR_Query.Details",
                    "@type": "unece:AggregateBIE",
                    "unece:cefactUNId": "UN01010570",
                    "rdfs:comment": "A formally raised question or request for Master Data Register (MDR) information."
                },
                {
                    "@id": "cefact:Vessel_Query.Details",
                    "@type": "unece:AggregateBIE",
                    "unece:cefactUNId": "UN01010736",
                    "rdfs:comment": "A formally raised question or request for information about a vessel."
                }
            ]
        },
        {
            "@id": "fisheries:QueryParameter",
            "@type": "rdfs:Class",
            "rdfs:comment": [
                "Information that limits or restricts the scope of an Inspection and/or Surveillance Report (ISR) query.",
                "Information that limits or restricts the scope of a sales query.",
                "Information that limits or restricts the scope of a vessel query.",
                "Information that limits or restricts the scope of a Fishing Activity (FA) query."
            ],
            "rdfs:label": "QueryParameter",
            "unece:cefactElementMetadata": [
                {
                    "@id": "cefact:FA_QueryParameter.Details",
                    "@type": "unece:AggregateBIE",
                    "unece:cefactUNId": "UN01011224",
                    "rdfs:comment": "Information that limits or restricts the scope of a Fishing Activity (FA) query."
                },
                {
                    "@id": "cefact:Vessel_QueryParameter.Details",
                    "@type": "unece:AggregateBIE",
                    "unece:cefactUNId": "UN01010748",
                    "rdfs:comment": "Information that limits or restricts the scope of a vessel query."
                },
                {
                    "@id": "cefact:Sales_QueryParameter.Details",
                    "@type": "unece:AggregateBIE",
                    "unece:cefactUNId": "UN01011000",
                    "rdfs:comment": "Information that limits or restricts the scope of a sales query."
                },
                {
                    "@id": "cefact:ISR_QueryParameter.Details",
                    "@type": "unece:AggregateBIE",
                    "unece:cefactUNId": "UN01012641",
                    "rdfs:comment": "Information that limits or restricts the scope of an Inspection and/or Surveillance Report (ISR) query."
                }
            ]
        },
        {
            "@id": "fisheries:Quota",
            "@type": "rdfs:Class",
            "rdfs:comment": "A limited quantity, such as of fish or effort, which under official controls is targeted to be caught, produced, exported, imported or consumed.",
            "rdfs:label": "Quota",
            "unece:cefactElementMetadata": [
                {
                    "@id": "cefact:Targeted_Quota.Details",
                    "@type": "unece:AggregateBIE",
                    "unece:cefactUNId": "UN01010878",
                    "rdfs:comment": "A limited quantity, such as of fish or effort, which under official controls is targeted to be caught, produced, exported, imported or consumed."
                }
            ]
        },
        {
            "@id": "fisheries:Report",
            "@type": "rdfs:Class",
            "rdfs:comment": [
                "A compilation of information which is pertinent to an Inspection and/or Surveillance (IS).",
                "A record of products sold, such as a sales note report, takeover note report or transport note report."
            ],
            "rdfs:label": "Report",
            "unece:cefactElementMetadata": [
                {
                    "@id": "cefact:Sales_Report.Details",
                    "@type": "unece:AggregateBIE",
                    "unece:cefactUNId": "UN01010904",
                    "rdfs:comment": "A record of products sold, such as a sales note report, takeover note report or transport note report."
                },
                {
                    "@id": "cefact:IS_Report.Details",
                    "@type": "unece:AggregateBIE",
                    "unece:cefactUNId": "UN01012588",
                    "rdfs:comment": "A compilation of information which is pertinent to an Inspection and/or Surveillance (IS)."
                }
            ]
        },
        {
            "@id": "fisheries:ReportedArea",
            "@type": "rdfs:Class",
            "rdfs:comment": "An area related to a reported catch for an Aggregated Catch Data Report (ACDR).",
            "rdfs:label": "ReportedArea",
            "unece:cefactElementMetadata": [
                {
                    "@id": "cefact:ACDR_ReportedArea.Details",
                    "@type": "unece:AggregateBIE",
                    "unece:cefactUNId": "UN01010258",
                    "rdfs:comment": "An area related to a reported catch for an Aggregated Catch Data Report (ACDR)."
                }
            ]
        },
        {
            "@id": "fisheries:Status",
            "@type": "rdfs:Class",
            "rdfs:comment": "Details concerning the status of an inspected vessel.",
            "rdfs:label": "Status",
            "unece:cefactElementMetadata": [
                {
                    "@id": "cefact:InspectedVessel_Status.Details",
                    "@type": "unece:AggregateBIE",
                    "unece:cefactUNId": "UN01013334",
                    "rdfs:comment": "Details concerning the status of an inspected vessel."
                }
            ]
        },
        {
            "@id": "fisheries:Stock",
            "@type": "rdfs:Class",
            "rdfs:comment": "A quantity of Aquatic Animal or Plant (AAP), such as a stock of fish, available for being up-taken.",
            "rdfs:label": "Stock",
            "unece:cefactElementMetadata": [
                {
                    "@id": "cefact:AAP_Stock.Details",
                    "@type": "unece:AggregateBIE",
                    "unece:cefactUNId": "UN01011199",
                    "rdfs:comment": "A quantity of Aquatic Animal or Plant (AAP), such as a stock of fish, available for being up-taken."
                }
            ]
        },
        {
            "@id": "fisheries:Suspicion",
            "@type": "rdfs:Class",
            "rdfs:comment": "A compilation of information about suspected infringements noted in the Inspection or Surveillance Report (ISR).",
            "rdfs:label": "Suspicion",
            "unece:cefactElementMetadata": [
                {
                    "@id": "cefact:ISRInfringement_Suspicion.Details",
                    "@type": "unece:AggregateBIE",
                    "unece:cefactUNId": "UN01013322",
                    "rdfs:comment": "A compilation of information about suspected infringements noted in the Inspection or Surveillance Report (ISR)."
                }
            ]
        },
        {
            "@id": "fisheries:TransportCharter",
            "@type": "rdfs:Class",
            "rdfs:comment": "The reservation of a vessel for a particular usage.",
            "rdfs:label": "TransportCharter",
            "unece:cefactElementMetadata": [
                {
                    "@id": "cefact:Vessel_TransportCharter.Details",
                    "@type": "unece:AggregateBIE",
                    "unece:cefactUNId": "UN01010874",
                    "rdfs:comment": "The reservation of a vessel for a particular usage."
                }
            ]
        },
        {
            "@id": "fisheries:TransportMeans",
            "@type": "rdfs:Class",
            "rdfs:comment": [
                "The identification and registration of a vehicle, such as a truck or lorry.",
                "The identification and characteristic information of a ship or boat."
            ],
            "rdfs:label": "TransportMeans",
            "unece:cefactElementMetadata": [
                {
                    "@id": "cefact:Vehicle_TransportMeans.Details",
                    "@type": "unece:AggregateBIE",
                    "unece:cefactUNId": "UN01010987",
                    "rdfs:comment": "The identification and registration of a vehicle, such as a truck or lorry."
                },
                {
                    "@id": "cefact:Vessel_TransportMeans.Details",
                    "@type": "unece:AggregateBIE",
                    "unece:cefactUNId": "UN01010227",
                    "rdfs:comment": "The identification and characteristic information of a ship or boat."
                }
            ]
        },
        {
            "@id": "fisheries:Trip",
            "@type": "rdfs:Class",
            "rdfs:comment": "A journey or a trip having some fishing activity.",
            "rdfs:label": "Trip",
            "unece:cefactElementMetadata": [
                {
                    "@id": "cefact:Fishing_Trip.Details",
                    "@type": "unece:AggregateBIE",
                    "unece:cefactUNId": "UN01011164",
                    "rdfs:comment": "A journey or a trip having some fishing activity."
                }
            ]
        },
        {
            "@id": "fisheries:Version",
            "@type": "rdfs:Class",
            "rdfs:comment": "A specific issuance of a data set object.",
            "rdfs:label": "Version",
            "unece:cefactElementMetadata": [
                {
                    "@id": "cefact:DataSet_Version.Details",
                    "@type": "unece:AggregateBIE",
                    "unece:cefactUNId": "UN01010598",
                    "rdfs:comment": "A specific issuance of a data set object."
                }
            ]
        },
        {
            "@id": "fisheries:aAPProcessTypeCode",
            "@type": "rdf:Property",
            "schema:rangeIncludes": {
                "@id": "unece:UNECECL7187Code"
            },
            "schema:domainIncludes": {
                "@id": "fisheries:Process"
            },
            "rdfs:comment": "A code specifying the type of AAP process, such as presentation type, preservation type.",
            "rdfs:label": "aAPProcessTypeCode",
            "unece:cefactElementMetadata": [
                {
                    "@id": "cefact:AAP_Process.Type.Code",
                    "@type": "unece:BasicBIE",
                    "unece:TDED": "7187",
                    "unece:cefactUNId": "UN01010944",
                    "unece:cefactBieDomainClass": "cefact:AAP_Process.Details",
                    "rdfs:comment": "A code specifying the type of AAP process, such as presentation type, preservation type."
                }
            ]
        },
        {
            "@id": "fisheries:aboveDeckSizeQuantity",
            "@type": "rdf:Property",
            "schema:rangeIncludes": {
                "@id": "xsd:decimal"
            },
            "schema:domainIncludes": {
                "@id": "fisheries:Crew"
            },
            "rdfs:comment": "The size, expressed as a quantity, of this vessel crew working above the deck.",
            "rdfs:label": "aboveDeckSizeQuantity",
            "unece:cefactElementMetadata": [
                {
                    "@id": "cefact:Vessel_Crew.AboveDeck_Size.Quantity",
                    "@type": "unece:BasicBIE",
                    "unece:cefactUNId": "UN01010818",
                    "unece:cefactBieDomainClass": "cefact:Vessel_Crew.Details",
                    "rdfs:comment": "The size, expressed as a quantity, of this vessel crew working above the deck."
                }
            ]
        },
        {
            "@id": "fisheries:acceptanceDateTime",
            "@type": "rdf:Property",
            "schema:rangeIncludes": {
                "@id": "xsd:dateTime"
            },
            "schema:domainIncludes": {
                "@id": "fisheries:Document"
            },
            "rdfs:comment": "The date, time, date time, or other date time value, of the acceptance of this FA report document.",
            "rdfs:label": "acceptanceDateTime",
            "unece:cefactElementMetadata": [
                {
                    "@id": "cefact:FAReport_Document.Acceptance.DateTime",
                    "@type": "unece:BasicBIE",
                    "unece:TDED": "2097",
                    "unece:cefactUNId": "UN01011160",
                    "unece:cefactBieDomainClass": "cefact:FAReport_Document.Details",
                    "rdfs:comment": "The date, time, date time, or other date time value, of the acceptance of this FA report document."
                }
            ]
        },
        {
            "@id": "fisheries:activityTypeCode",
            "@type": "rdf:Property",
            "schema:rangeIncludes": {
                "@id": "xsd:token"
            },
            "schema:domainIncludes": {
                "@id": "fisheries:Event"
            },
            "rdfs:comment": "The code specifying the type of activity, such as of the vessel or the crew, at this vessel position event.",
            "rdfs:label": "activityTypeCode",
            "unece:cefactElementMetadata": [
                {
                    "@id": "cefact:VesselPosition_Event.Activity_Type.Code",
                    "@type": "unece:BasicBIE",
                    "unece:TDED": "9171",
                    "unece:cefactUNId": "UN01012114",
                    "unece:cefactBieDomainClass": "cefact:VesselPosition_Event.Details",
                    "rdfs:comment": "The code specifying the type of activity, such as of the vessel or the crew, at this vessel position event."
                }
            ]
        },
        {
            "@id": "fisheries:affectedQuantity",
            "@type": "rdf:Property",
            "schema:rangeIncludes": {
                "@id": "xsd:decimal"
            },
            "schema:domainIncludes": {
                "@id": "fisheries:Problem"
            },
            "rdfs:comment": "The number of gears affected by this gear problem.",
            "rdfs:label": "affectedQuantity",
            "unece:cefactElementMetadata": [
                {
                    "@id": "cefact:Gear_Problem.Affected.Quantity",
                    "@type": "unece:BasicBIE",
                    "unece:cefactUNId": "UN01011210",
                    "unece:cefactBieDomainClass": "cefact:Gear_Problem.Details",
                    "rdfs:comment": "The number of gears affected by this gear problem."
                }
            ]
        },
        {
            "@id": "fisheries:altitudeMeasure",
            "@type": "rdf:Property",
            "schema:rangeIncludes": {
                "@id": "xsd:decimal"
            },
            "schema:domainIncludes": {
                "@id": "fisheries:GeographicalCoordinate"
            },
            "rdfs:comment": [
                "The measure of the altitude of this FLUX geographical coordinate.",
                "The measure of the altitude that reflects the vertical elevation of an object above a surface for this vessel geographical coordinate."
            ],
            "rdfs:label": "altitudeMeasure",
            "unece:cefactElementMetadata": [
                {
                    "@id": "cefact:Vessel_GeographicalCoordinate.Altitude.Measure",
                    "@type": "unece:BasicBIE",
                    "unece:cefactUNId": "UN01010222",
                    "unece:cefactBieDomainClass": "cefact:Vessel_GeographicalCoordinate.Details",
                    "rdfs:comment": "The measure of the altitude that reflects the vertical elevation of an object above a surface for this vessel geographical coordinate."
                },
                {
                    "@id": "cefact:FLUX_GeographicalCoordinate.Altitude.Measure",
                    "@type": "unece:BasicBIE",
                    "unece:cefactUNId": "UN01010969",
                    "unece:cefactBieDomainClass": "cefact:FLUX_GeographicalCoordinate.Details",
                    "rdfs:comment": "The measure of the altitude of this FLUX geographical coordinate."
                }
            ]
        },
        {
            "@id": "fisheries:applicableCharacteristic",
            "@type": "rdf:Property",
            "schema:rangeIncludes": {
                "@id": "fisheries:Characteristic"
            },
            "schema:domainIncludes": [
                {
                    "@id": "fisheries:Catch"
                },
                {
                    "@id": "fisheries:Equipment"
                },
                {
                    "@id": "fisheries:Event"
                },
                {
                    "@id": "fisheries:Gear"
                },
                {
                    "@id": "fisheries:Location"
                },
                {
                    "@id": "fisheries:TransportMeans"
                }
            ],
            "rdfs:comment": [
                "A Fisheries Language Universal eXchange (FLUX) characteristic applicable to this fishing gear equipment.",
                "A Fisheries Language for Universal eXchange (FLUX) characteristic applicable to this FA catch.",
                "A characteristic applicable to this FLUX location.",
                "A characteristic applicable to this fishing gear.",
                "A gear characteristic applicable to this gear equipment inspection event.",
                "A storage characteristic applicable to this transport means vessel.",
                "A technical characteristic applicable to this transport means vessel.",
                "A vessel administrative characteristic applicable to this transport means vessel.",
                "A vessel equipment characteristic applicable to this transport means vessel."
            ],
            "rdfs:label": "applicableCharacteristic",
            "unece:cefactElementMetadata": [
                {
                    "@id": "cefact:Vessel_TransportMeans.Applicable.VesselEquipment_Characteristic",
                    "@type": "unece:AssociationBIE",
                    "unece:cefactUNId": "UN01010646",
                    "unece:cefactBieDomainClass": "cefact:Vessel_TransportMeans.Details",
                    "rdfs:comment": "A vessel equipment characteristic applicable to this transport means vessel."
                },
                {
                    "@id": "cefact:FishingGear_Equipment.Applicable.FLUX_Characteristic",
                    "@type": "unece:AssociationBIE",
                    "unece:cefactUNId": "UN01012659",
                    "unece:cefactBieDomainClass": "cefact:FishingGear_Equipment.Details",
                    "rdfs:comment": "A Fisheries Language Universal eXchange (FLUX) characteristic applicable to this fishing gear equipment."
                },
                {
                    "@id": "cefact:Fishing_Gear.Applicable.Gear_Characteristic",
                    "@type": "unece:AssociationBIE",
                    "unece:cefactUNId": "UN01010780",
                    "unece:cefactBieDomainClass": "cefact:Fishing_Gear.Details",
                    "rdfs:comment": "A characteristic applicable to this fishing gear."
                },
                {
                    "@id": "cefact:GearEquipmentInspection_Event.Applicable.Gear_Characteristic",
                    "@type": "unece:AssociationBIE",
                    "unece:cefactUNId": "UN01013332",
                    "unece:cefactBieDomainClass": "cefact:GearEquipmentInspection_Event.Details",
                    "rdfs:comment": "A gear characteristic applicable to this gear equipment inspection event."
                },
                {
                    "@id": "cefact:FA_Catch.Applicable.FLUX_Characteristic",
                    "@type": "unece:AssociationBIE",
                    "unece:cefactUNId": "UN01011198",
                    "unece:cefactBieDomainClass": "cefact:FA_Catch.Details",
                    "rdfs:comment": "A Fisheries Language for Universal eXchange (FLUX) characteristic applicable to this FA catch."
                },
                {
                    "@id": "cefact:Vessel_TransportMeans.Applicable.VesselStorage_Characteristic",
                    "@type": "unece:AssociationBIE",
                    "unece:cefactUNId": "UN01010772",
                    "unece:cefactBieDomainClass": "cefact:Vessel_TransportMeans.Details",
                    "rdfs:comment": "A storage characteristic applicable to this transport means vessel."
                },
                {
                    "@id": "cefact:Vessel_TransportMeans.Applicable.VesselTechnical_Characteristic",
                    "@type": "unece:AssociationBIE",
                    "unece:cefactUNId": "UN01010773",
                    "unece:cefactBieDomainClass": "cefact:Vessel_TransportMeans.Details",
                    "rdfs:comment": "A technical characteristic applicable to this transport means vessel."
                },
                {
                    "@id": "cefact:FLUX_Location.Applicable.FLUX_Characteristic",
                    "@type": "unece:AssociationBIE",
                    "unece:cefactUNId": "UN01011206",
                    "unece:cefactBieDomainClass": "cefact:FLUX_Location.Details",
                    "rdfs:comment": "A characteristic applicable to this FLUX location."
                },
                {
                    "@id": "cefact:Vessel_TransportMeans.Applicable.VesselAdministrative_Characteristic",
                    "@type": "unece:AssociationBIE",
                    "unece:cefactUNId": "UN01010647",
                    "unece:cefactBieDomainClass": "cefact:Vessel_TransportMeans.Details",
                    "rdfs:comment": "A vessel administrative characteristic applicable to this transport means vessel."
                }
            ]
        },
        {
            "@id": "fisheries:applicablePeriod",
            "@type": "rdf:Property",
            "schema:rangeIncludes": {
                "@id": "fisheries:Period"
            },
            "schema:domainIncludes": [
                {
                    "@id": "fisheries:Document"
                },
                {
                    "@id": "fisheries:TransportCharter"
                }
            ],
            "rdfs:comment": [
                "A delimited period applicable to this FLAP document.",
                "A delimited period applicable to this vessel transport charter."
            ],
            "rdfs:label": "applicablePeriod",
            "unece:cefactElementMetadata": [
                {
                    "@id": "cefact:Vessel_TransportCharter.Applicable.Delimited_Period",
                    "@type": "unece:AssociationBIE",
                    "unece:cefactUNId": "UN01010876",
                    "unece:cefactBieDomainClass": "cefact:Vessel_TransportCharter.Details",
                    "rdfs:comment": "A delimited period applicable to this vessel transport charter."
                },
                {
                    "@id": "cefact:FLAP_Document.Applicable.Delimited_Period",
                    "@type": "unece:AssociationBIE",
                    "unece:cefactUNId": "UN01010855",
                    "unece:cefactBieDomainClass": "cefact:FLAP_Document.Details",
                    "rdfs:comment": "A delimited period applicable to this FLAP document."
                }
            ]
        },
        {
            "@id": "fisheries:appliedProcess",
            "@type": "rdf:Property",
            "schema:rangeIncludes": {
                "@id": "fisheries:Process"
            },
            "schema:domainIncludes": [
                {
                    "@id": "fisheries:Catch"
                },
                {
                    "@id": "fisheries:Product"
                }
            ],
            "rdfs:comment": [
                "A Aquatic Animal or Plant (AAP) process applied to this FA catch.",
                "A process applied to this AAP product."
            ],
            "rdfs:label": "appliedProcess",
            "unece:cefactElementMetadata": [
                {
                    "@id": "cefact:FA_Catch.Applied.AAP_Process",
                    "@type": "unece:AssociationBIE",
                    "unece:cefactUNId": "UN01011194",
                    "unece:cefactBieDomainClass": "cefact:FA_Catch.Details",
                    "rdfs:comment": "A Aquatic Animal or Plant (AAP) process applied to this FA catch."
                },
                {
                    "@id": "cefact:AAP_Product.Applied.AAP_Process",
                    "@type": "unece:AssociationBIE",
                    "unece:cefactUNId": "UN01010940",
                    "unece:cefactBieDomainClass": "cefact:AAP_Product.Details",
                    "rdfs:comment": "A process applied to this AAP product."
                }
            ]
        },
        {
            "@id": "fisheries:areaIncludedId",
            "@type": "rdf:Property",
            "schema:rangeIncludes": {
                "@id": "xsd:token"
            },
            "schema:domainIncludes": {
                "@id": "fisheries:Picture"
            },
            "rdfs:comment": "The area or location, expressed as an identifier, that is included in this FLUX picture.",
            "rdfs:label": "areaIncludedId",
            "unece:cefactElementMetadata": [
                {
                    "@id": "cefact:FLUX_Picture.AreaIncluded.Identifier",
                    "@type": "unece:BasicBIE",
                    "unece:cefactUNId": "UN01010733",
                    "unece:cefactBieDomainClass": "cefact:FLUX_Picture.Details",
                    "rdfs:comment": "The area or location, expressed as an identifier, that is included in this FLUX picture."
                }
            ]
        },
        {
            "@id": "fisheries:arrivalSpecifiedLocation",
            "@type": "rdf:Property",
            "schema:rangeIncludes": {
                "@id": "fisheries:Location"
            },
            "schema:domainIncludes": {
                "@id": "fisheries:Document"
            },
            "rdfs:comment": "The arrival Fisheries Language for Universal eXchange (FLUX) location specified in this sales document.",
            "rdfs:label": "arrivalSpecifiedLocation",
            "unece:cefactElementMetadata": [
                {
                    "@id": "cefact:Sales_Document.Arrival_Specified.FLUX_Location",
                    "@type": "unece:AssociationBIE",
                    "unece:cefactUNId": "UN01012118",
                    "unece:cefactBieDomainClass": "cefact:Sales_Document.Details",
                    "rdfs:comment": "The arrival Fisheries Language for Universal eXchange (FLUX) location specified in this sales document."
                }
            ]
        },
        {
            "@id": "fisheries:attachedBinaryFile",
            "@type": "rdf:Property",
            "schema:rangeIncludes": {
                "@id": "fisheries:BinaryFile"
            },
            "schema:domainIncludes": {
                "@id": "fisheries:Document"
            },
            "rdfs:comment": "A Fisheries Language for Universal eXchange (FLUX) binary file attached to this FLAP document.",
            "rdfs:label": "attachedBinaryFile",
            "unece:cefactElementMetadata": [
                {
                    "@id": "cefact:FLAP_Document.Attached.FLUX_BinaryFile",
                    "@type": "unece:AssociationBIE",
                    "unece:cefactUNId": "UN01010860",
                    "unece:cefactBieDomainClass": "cefact:FLAP_Document.Details",
                    "rdfs:comment": "A Fisheries Language for Universal eXchange (FLUX) binary file attached to this FLAP document."
                }
            ]
        },
        {
            "@id": "fisheries:attachedEngine",
            "@type": "rdf:Property",
            "schema:rangeIncludes": {
                "@id": "fisheries:Engine"
            },
            "schema:domainIncludes": {
                "@id": "fisheries:TransportMeans"
            },
            "rdfs:comment": "A vessel engine attached to this transport means vessel.",
            "rdfs:label": "attachedEngine",
            "unece:cefactElementMetadata": [
                {
                    "@id": "cefact:Vessel_TransportMeans.Attached.Vessel_Engine",
                    "@type": "unece:AssociationBIE",
                    "unece:cefactUNId": "UN01010643",
                    "unece:cefactBieDomainClass": "cefact:Vessel_TransportMeans.Details",
                    "rdfs:comment": "A vessel engine attached to this transport means vessel."
                }
            ]
        },
        {
            "@id": "fisheries:attachedEquipment",
            "@type": "rdf:Property",
            "schema:rangeIncludes": {
                "@id": "fisheries:Equipment"
            },
            "schema:domainIncludes": {
                "@id": "fisheries:Gear"
            },
            "rdfs:comment": "Equipment attached to this fishing gear.",
            "rdfs:label": "attachedEquipment",
            "unece:cefactElementMetadata": [
                {
                    "@id": "cefact:Fishing_Gear.Attached.FishingGear_Equipment",
                    "@type": "unece:AssociationBIE",
                    "unece:cefactUNId": "UN01012660",
                    "unece:cefactBieDomainClass": "cefact:Fishing_Gear.Details",
                    "rdfs:comment": "Equipment attached to this fishing gear."
                }
            ]
        },
        {
            "@id": "fisheries:authorizedGear",
            "@type": "rdf:Property",
            "schema:rangeIncludes": {
                "@id": "fisheries:Gear"
            },
            "schema:domainIncludes": {
                "@id": "fisheries:Category"
            },
            "rdfs:comment": "Fishing gear authorized for this fishing category.",
            "rdfs:label": "authorizedGear",
            "unece:cefactElementMetadata": [
                {
                    "@id": "cefact:Fishing_Category.Authorized.Fishing_Gear",
                    "@type": "unece:AssociationBIE",
                    "unece:cefactUNId": "UN01010844",
                    "unece:cefactBieDomainClass": "cefact:Fishing_Category.Details",
                    "rdfs:comment": "Fishing gear authorized for this fishing category."
                }
            ]
        },
        {
            "@id": "fisheries:boundaryPolygon",
            "@type": "rdf:Property",
            "schema:rangeIncludes": {
                "@id": "fisheries:Polygon"
            },
            "schema:domainIncludes": {
                "@id": "fisheries:Location"
            },
            "rdfs:comment": "A specified polygon of the boundary for this FLUX location.",
            "rdfs:label": "boundaryPolygon",
            "unece:cefactElementMetadata": [
                {
                    "@id": "cefact:FLUX_Location.Boundary.Specified_Polygon",
                    "@type": "unece:AssociationBIE",
                    "unece:cefactUNId": "UN01011205",
                    "unece:cefactBieDomainClass": "cefact:FLUX_Location.Details",
                    "rdfs:comment": "A specified polygon of the boundary for this FLUX location."
                }
            ]
        },
        {
            "@id": "fisheries:buyerName",
            "@type": "rdf:Property",
            "schema:rangeIncludes": {
                "@id": "xsd:string"
            },
            "schema:domainIncludes": {
                "@id": "fisheries:Event"
            },
            "rdfs:comment": "The name of the buyer, such as company name or name of an individual, expressed as text, for this sales event.",
            "rdfs:label": "buyerName",
            "unece:cefactElementMetadata": [
                {
                    "@id": "cefact:Sales_Event.Buyer_Name.Text",
                    "@type": "unece:BasicBIE",
                    "unece:cefactUNId": "UN01010950",
                    "unece:cefactBieDomainClass": "cefact:Sales_Event.Details",
                    "rdfs:comment": "The name of the buyer, such as company name or name of an individual, expressed as text, for this sales event."
                }
            ]
        },
        {
            "@id": "fisheries:capacityValueMeasure",
            "@type": "rdf:Property",
            "schema:rangeIncludes": {
                "@id": "xsd:decimal"
            },
            "schema:domainIncludes": {
                "@id": "fisheries:Characteristic"
            },
            "rdfs:comment": "A capacity value, expressed as a measure, for this vessel storage characteristic.",
            "rdfs:label": "capacityValueMeasure",
            "unece:cefactElementMetadata": [
                {
                    "@id": "cefact:VesselStorage_Characteristic.Capacity_Value.Measure",
                    "@type": "unece:BasicBIE",
                    "unece:cefactUNId": "UN01010809",
                    "unece:cefactBieDomainClass": "cefact:VesselStorage_Characteristic.Details",
                    "rdfs:comment": "A capacity value, expressed as a measure, for this vessel storage characteristic."
                }
            ]
        },
        {
            "@id": "fisheries:catchStatusCode",
            "@type": "rdf:Property",
            "schema:rangeIncludes": {
                "@id": "xsd:token"
            },
            "schema:domainIncludes": {
                "@id": "fisheries:ReportedArea"
            },
            "rdfs:comment": "The code specifying the catch status, either transshipment or retention on board, reported for this ACDR area.",
            "rdfs:label": "catchStatusCode",
            "unece:cefactElementMetadata": [
                {
                    "@id": "cefact:ACDR_ReportedArea.CatchStatus.Code",
                    "@type": "unece:BasicBIE",
                    "unece:cefactUNId": "UN01010262",
                    "unece:cefactBieDomainClass": "cefact:ACDR_ReportedArea.Details",
                    "rdfs:comment": "The code specifying the catch status, either transshipment or retention on board, reported for this ACDR area."
                }
            ]
        },
        {
            "@id": "fisheries:categoryCode",
            "@type": "rdf:Property",
            "schema:rangeIncludes": {
                "@id": "xsd:token"
            },
            "schema:domainIncludes": {
                "@id": "fisheries:Distribution"
            },
            "rdfs:comment": "The code specifying a category for this size distribution, such as a range of sizes.",
            "rdfs:label": "categoryCode",
            "unece:cefactElementMetadata": [
                {
                    "@id": "cefact:Size_Distribution.Category.Code",
                    "@type": "unece:BasicBIE",
                    "unece:cefactUNId": "UN01011153",
                    "unece:cefactBieDomainClass": "cefact:Size_Distribution.Details",
                    "rdfs:comment": "The code specifying a category for this size distribution, such as a range of sizes."
                }
            ]
        },
        {
            "@id": "fisheries:chargeAmount",
            "@type": "rdf:Property",
            "schema:rangeIncludes": {
                "@id": "xsd:decimal"
            },
            "schema:domainIncludes": {
                "@id": "fisheries:Price"
            },
            "rdfs:comment": "A monetary value of this sales price charged.",
            "rdfs:label": "chargeAmount",
            "unece:cefactElementMetadata": [
                {
                    "@id": "cefact:Sales_Price.Charge.Amount",
                    "@type": "unece:BasicBIE",
                    "unece:cefactUNId": "UN01010946",
                    "unece:cefactBieDomainClass": "cefact:Sales_Price.Details",
                    "rdfs:comment": "A monetary value of this sales price charged."
                }
            ]
        },
        {
            "@id": "fisheries:checkInspectionCode",
            "@type": "rdf:Property",
            "schema:rangeIncludes": {
                "@id": "xsd:token"
            },
            "schema:domainIncludes": {
                "@id": "fisheries:Characteristic"
            },
            "rdfs:comment": "The code specifying inspection checks performed for this ISR Item characteristic and reported back as the check result.",
            "rdfs:label": "checkInspectionCode",
            "unece:cefactElementMetadata": [
                {
                    "@id": "cefact:ISRItem_Characteristic.Check_Inspection.Code",
                    "@type": "unece:BasicBIE",
                    "unece:cefactUNId": "UN01013321",
                    "unece:cefactBieDomainClass": "cefact:ISRItem_Characteristic.Details",
                    "rdfs:comment": "The code specifying inspection checks performed for this ISR Item characteristic and reported back as the check result."
                }
            ]
        },
        {
            "@id": "fisheries:classCode",
            "@type": "rdf:Property",
            "schema:rangeIncludes": {
                "@id": "xsd:token"
            },
            "schema:domainIncludes": {
                "@id": "fisheries:Distribution"
            },
            "rdfs:comment": "A code specifying a class for this size distribution, such as below minimum size.",
            "rdfs:label": "classCode",
            "unece:cefactElementMetadata": [
                {
                    "@id": "cefact:Size_Distribution.Class.Code",
                    "@type": "unece:BasicBIE",
                    "unece:cefactUNId": "UN01011154",
                    "unece:cefactBieDomainClass": "cefact:Size_Distribution.Details",
                    "rdfs:comment": "A code specifying a class for this size distribution, such as below minimum size."
                }
            ]
        },
        {
            "@id": "fisheries:commissioningDateTime",
            "@type": "rdf:Property",
            "schema:rangeIncludes": {
                "@id": "xsd:dateTime"
            },
            "schema:domainIncludes": {
                "@id": "fisheries:TransportMeans"
            },
            "rdfs:comment": "The date, time, date time or other date time value of the commissioning of this vessel transport means, such as the date of issue of the first safety certificate, the date of first entry in an official register of fishing vessels.",
            "rdfs:label": "commissioningDateTime",
            "unece:cefactElementMetadata": [
                {
                    "@id": "cefact:Vessel_TransportMeans.Commissioning.DateTime",
                    "@type": "unece:BasicBIE",
                    "unece:cefactUNId": "UN01010637",
                    "unece:cefactBieDomainClass": "cefact:Vessel_TransportMeans.Details",
                    "rdfs:comment": "The date, time, date time or other date time value of the commissioning of this vessel transport means, such as the date of issue of the first safety certificate, the date of first entry in an official register of fishing vessels."
                }
            ]
        },
        {
            "@id": "fisheries:compoundQueryParameter",
            "@type": "rdf:Property",
            "schema:rangeIncludes": {
                "@id": "fisheries:QueryParameter"
            },
            "schema:domainIncludes": {
                "@id": "fisheries:Query"
            },
            "rdfs:comment": "A compound logical query parameter for this vessel query.",
            "rdfs:label": "compoundQueryParameter",
            "unece:cefactElementMetadata": [
                {
                    "@id": "cefact:Vessel_Query.Compound.Logical_QueryParameter",
                    "@type": "unece:AssociationBIE",
                    "unece:cefactUNId": "UN01010741",
                    "unece:cefactBieDomainClass": "cefact:Vessel_Query.Details",
                    "rdfs:comment": "A compound logical query parameter for this vessel query."
                }
            ]
        },
        {
            "@id": "fisheries:containedDataNode",
            "@type": "rdf:Property",
            "schema:rangeIncludes": {
                "@id": "fisheries:DataNode"
            },
            "schema:domainIncludes": {
                "@id": "fisheries:DataSet"
            },
            "rdfs:comment": "A data node contained in this MDR data set.",
            "rdfs:label": "containedDataNode",
            "unece:cefactElementMetadata": [
                {
                    "@id": "cefact:MDR_DataSet.Contained.MDR_DataNode",
                    "@type": "unece:AssociationBIE",
                    "unece:cefactUNId": "UN01010588",
                    "unece:cefactBieDomainClass": "cefact:MDR_DataSet.Details",
                    "rdfs:comment": "A data node contained in this MDR data set."
                }
            ]
        },
        {
            "@id": "fisheries:contextCode",
            "@type": "rdf:Property",
            "schema:rangeIncludes": {
                "@id": "xsd:token"
            },
            "schema:domainIncludes": {
                "@id": "fisheries:Suspicion"
            },
            "rdfs:comment": "The code specifying the context for this ISR infringement suspicion.",
            "rdfs:label": "contextCode",
            "unece:cefactElementMetadata": [
                {
                    "@id": "cefact:ISRInfringement_Suspicion.Context.Code",
                    "@type": "unece:BasicBIE",
                    "unece:cefactUNId": "UN01013324",
                    "unece:cefactBieDomainClass": "cefact:ISRInfringement_Suspicion.Details",
                    "rdfs:comment": "The code specifying the context for this ISR infringement suspicion."
                }
            ]
        },
        {
            "@id": "fisheries:contextTypeCode",
            "@type": "rdf:Property",
            "schema:rangeIncludes": {
                "@id": "xsd:token"
            },
            "schema:domainIncludes": {
                "@id": "fisheries:Report"
            },
            "rdfs:comment": "A code specifying a context type for this IS report, such as inspection for an Regional Fisheries Management Organization (RFMO).",
            "rdfs:label": "contextTypeCode",
            "unece:cefactElementMetadata": [
                {
                    "@id": "cefact:IS_Report.Context_Type.Code",
                    "@type": "unece:BasicBIE",
                    "unece:cefactUNId": "UN01012590",
                    "unece:cefactBieDomainClass": "cefact:IS_Report.Details",
                    "rdfs:comment": "A code specifying a context type for this IS report, such as inspection for an Regional Fisheries Management Organization (RFMO)."
                }
            ]
        },
        {
            "@id": "fisheries:contractualLanguageCode",
            "@type": "rdf:Property",
            "schema:rangeIncludes": {
                "@id": "xsd:token"
            },
            "schema:domainIncludes": {
                "@id": "fisheries:Query"
            },
            "rdfs:comment": "The code specifying the contractual language for this MDR query.",
            "rdfs:label": "contractualLanguageCode",
            "unece:cefactElementMetadata": [
                {
                    "@id": "cefact:MDR_Query.ContractualLanguage.Code",
                    "@type": "unece:BasicBIE",
                    "unece:TDED": "3453",
                    "unece:cefactUNId": "UN01010574",
                    "unece:cefactBieDomainClass": "cefact:MDR_Query.Details",
                    "rdfs:comment": "The code specifying the contractual language for this MDR query."
                }
            ]
        },
        {
            "@id": "fisheries:conversionFactorNumeric",
            "@type": "rdf:Property",
            "schema:rangeIncludes": {
                "@id": "xsd:decimal"
            },
            "schema:domainIncludes": {
                "@id": "fisheries:Process"
            },
            "rdfs:comment": "The number used as the conversion factor for this AAP process.",
            "rdfs:label": "conversionFactorNumeric",
            "unece:cefactElementMetadata": [
                {
                    "@id": "cefact:AAP_Process.ConversionFactor.Numeric",
                    "@type": "unece:BasicBIE",
                    "unece:cefactUNId": "UN01011149",
                    "unece:cefactBieDomainClass": "cefact:AAP_Process.Details",
                    "rdfs:comment": "The number used as the conversion factor for this AAP process."
                }
            ]
        },
        {
            "@id": "fisheries:countryId",
            "@type": "rdf:Property",
            "schema:rangeIncludes": {
                "@id": "xsd:token"
            },
            "schema:domainIncludes": [
                {
                    "@id": "fisheries:Location"
                },
                {
                    "@id": "fisheries:Party"
                }
            ],
            "rdfs:comment": [
                "The country identifier for this sales party.",
                "The identifier of a country for this FLUX location."
            ],
            "rdfs:label": "countryId",
            "unece:cefactElementMetadata": [
                {
                    "@id": "cefact:Sales_Party.Country.Identifier",
                    "@type": "unece:BasicBIE",
                    "unece:cefactUNId": "UN01010926",
                    "unece:cefactBieDomainClass": "cefact:Sales_Party.Details",
                    "rdfs:comment": "The country identifier for this sales party."
                },
                {
                    "@id": "cefact:FLUX_Location.Country.Identifier",
                    "@type": "unece:BasicBIE",
                    "unece:cefactUNId": "UN01010961",
                    "unece:cefactBieDomainClass": "cefact:FLUX_Location.Details",
                    "rdfs:comment": "The identifier of a country for this FLUX location."
                }
            ]
        },
        {
            "@id": "fisheries:courseValueMeasure",
            "@type": "rdf:Property",
            "schema:rangeIncludes": {
                "@id": "xsd:decimal"
            },
            "schema:domainIncludes": {
                "@id": "fisheries:Event"
            },
            "rdfs:comment": "The measure of course of the vessel for this vessel position event.",
            "rdfs:label": "courseValueMeasure",
            "unece:cefactElementMetadata": [
                {
                    "@id": "cefact:VesselPosition_Event.Course_Value.Measure",
                    "@type": "unece:BasicBIE",
                    "unece:cefactUNId": "UN01010237",
                    "unece:cefactBieDomainClass": "cefact:VesselPosition_Event.Details",
                    "rdfs:comment": "The measure of course of the vessel for this vessel position event."
                }
            ]
        },
        {
            "@id": "fisheries:creationDateTime",
            "@type": "rdf:Property",
            "schema:rangeIncludes": {
                "@id": "xsd:dateTime"
            },
            "schema:domainIncludes": {
                "@id": "fisheries:Document"
            },
            "rdfs:comment": [
                "The date, time, date time or other date time value of a creation of this FLUX response document.",
                "The date, time, date time or other date time value of a creation of this validation result document.",
                "The date, time, date time or other date time value of the creation of this FLUX report document."
            ],
            "rdfs:label": "creationDateTime",
            "unece:cefactElementMetadata": [
                {
                    "@id": "cefact:FLUXResponse_Document.Creation.DateTime",
                    "@type": "unece:BasicBIE",
                    "unece:cefactUNId": "UN01010251",
                    "unece:cefactBieDomainClass": "cefact:FLUXResponse_Document.Details",
                    "rdfs:comment": "The date, time, date time or other date time value of a creation of this FLUX response document."
                },
                {
                    "@id": "cefact:FLUXReport_Document.Creation.DateTime",
                    "@type": "unece:BasicBIE",
                    "unece:cefactUNId": "UN01010241",
                    "unece:cefactBieDomainClass": "cefact:FLUXReport_Document.Details",
                    "rdfs:comment": "The date, time, date time or other date time value of the creation of this FLUX report document."
                },
                {
                    "@id": "cefact:ValidationResult_Document.Creation.DateTime",
                    "@type": "unece:BasicBIE",
                    "unece:cefactUNId": "UN01010752",
                    "unece:cefactBieDomainClass": "cefact:ValidationResult_Document.Details",
                    "rdfs:comment": "The date, time, date time or other date time value of a creation of this validation result document."
                }
            ]
        },
        {
            "@id": "fisheries:currencyCode",
            "@type": "rdf:Property",
            "schema:rangeIncludes": {
                "@id": "xsd:token"
            },
            "schema:domainIncludes": {
                "@id": "fisheries:Document"
            },
            "rdfs:comment": "The code specifying the currency for the sales in this sales document.",
            "rdfs:label": "currencyCode",
            "unece:cefactElementMetadata": [
                {
                    "@id": "cefact:Sales_Document.Currency.Code",
                    "@type": "unece:BasicBIE",
                    "unece:TDED": "6345",
                    "unece:cefactUNId": "UN01010911",
                    "unece:cefactBieDomainClass": "cefact:Sales_Document.Details",
                    "rdfs:comment": "The code specifying the currency for the sales in this sales document."
                }
            ]
        },
        {
            "@id": "fisheries:decisionDateTime",
            "@type": "rdf:Property",
            "schema:rangeIncludes": {
                "@id": "xsd:dateTime"
            },
            "schema:domainIncludes": {
                "@id": "fisheries:Document"
            },
            "rdfs:comment": "The decision date, time, date time or other date time value for this FLAP document.",
            "rdfs:label": "decisionDateTime",
            "unece:cefactElementMetadata": [
                {
                    "@id": "cefact:FLAP_Document.Decision.DateTime",
                    "@type": "unece:BasicBIE",
                    "unece:cefactUNId": "UN01010852",
                    "unece:cefactBieDomainClass": "cefact:FLAP_Document.Details",
                    "rdfs:comment": "The decision date, time, date time or other date time value for this FLAP document."
                }
            ]
        },
        {
            "@id": "fisheries:departureSpecifiedLocation",
            "@type": "rdf:Property",
            "schema:rangeIncludes": {
                "@id": "fisheries:Location"
            },
            "schema:domainIncludes": {
                "@id": "fisheries:Document"
            },
            "rdfs:comment": "The departure Fisheries Language for Universal eXchange (FLUX) location specified in this sales document.",
            "rdfs:label": "departureSpecifiedLocation",
            "unece:cefactElementMetadata": [
                {
                    "@id": "cefact:Sales_Document.Departure_Specified.FLUX_Location",
                    "@type": "unece:AssociationBIE",
                    "unece:cefactUNId": "UN01012117",
                    "unece:cefactBieDomainClass": "cefact:Sales_Document.Details",
                    "rdfs:comment": "The departure Fisheries Language for Universal eXchange (FLUX) location specified in this sales document."
                }
            ]
        },
        {
            "@id": "fisheries:dependentReport",
            "@type": "rdf:Property",
            "schema:rangeIncludes": {
                "@id": "fisheries:Report"
            },
            "schema:domainIncludes": {
                "@id": "fisheries:Report"
            },
            "rdfs:comment": "A report dependent on this IS report.",
            "rdfs:label": "dependentReport",
            "unece:cefactElementMetadata": [
                {
                    "@id": "cefact:IS_Report.Dependent.IS_Report",
                    "@type": "unece:AssociationBIE",
                    "unece:cefactUNId": "UN01012597",
                    "unece:cefactBieDomainClass": "cefact:IS_Report.Details",
                    "rdfs:comment": "A report dependent on this IS report."
                }
            ]
        },
        {
            "@id": "fisheries:description",
            "@type": "rdf:Property",
            "schema:rangeIncludes": {
                "@id": "xsd:string"
            },
            "schema:domainIncludes": [
                {
                    "@id": "fisheries:BinaryFile"
                },
                {
                    "@id": "fisheries:Characteristic"
                },
                {
                    "@id": "fisheries:DataSet"
                },
                {
                    "@id": "fisheries:Event"
                },
                {
                    "@id": "fisheries:Picture"
                },
                {
                    "@id": "fisheries:QualityAnalysis"
                }
            ],
            "rdfs:comment": [
                "A description, expressed as text, of this gear characteristic.",
                "A textual description of this FLUX characteristic.",
                "A textual description of this IS event.",
                "A textual description of this ISR item characteristic.",
                "A textual description of this gear inspection event.",
                "A textual description of this historical characteristic of a vessel.",
                "A textual description of this vessel administrative characteristic.",
                "A textual description of this vessel equipment characteristic.",
                "A textual description of this vessel event.",
                "A textual description of this vessel technical characteristic.",
                "The textual description for this MDR data set.",
                "The textual description of this FLUX binary file.",
                "The textual description of this FLUX picture.",
                "The textual description of this quality analysis of a validation process."
            ],
            "rdfs:label": "description",
            "unece:cefactElementMetadata": [
                {
                    "@id": "cefact:FLUX_BinaryFile.Description.Text",
                    "@type": "unece:BasicBIE",
                    "unece:cefactUNId": "UN01010802",
                    "unece:cefactBieDomainClass": "cefact:FLUX_BinaryFile.Details",
                    "rdfs:comment": "The textual description of this FLUX binary file."
                },
                {
                    "@id": "cefact:MDR_DataSet.Description.Text",
                    "@type": "unece:BasicBIE",
                    "unece:cefactUNId": "UN01010584",
                    "unece:cefactBieDomainClass": "cefact:MDR_DataSet.Details",
                    "rdfs:comment": "The textual description for this MDR data set."
                },
                {
                    "@id": "cefact:VesselTechnical_Characteristic.Description.Text",
                    "@type": "unece:BasicBIE",
                    "unece:TDED": "7036",
                    "unece:cefactUNId": "UN01010791",
                    "unece:cefactBieDomainClass": "cefact:VesselTechnical_Characteristic.Details",
                    "rdfs:comment": "A textual description of this vessel technical characteristic."
                },
                {
                    "@id": "cefact:Validation_QualityAnalysis.Description.Text",
                    "@type": "unece:BasicBIE",
                    "unece:cefactUNId": "UN01010766",
                    "unece:cefactBieDomainClass": "cefact:Validation_QualityAnalysis.Details",
                    "rdfs:comment": "The textual description of this quality analysis of a validation process."
                },
                {
                    "@id": "cefact:Vessel_Event.Description.Text",
                    "@type": "unece:BasicBIE",
                    "unece:cefactUNId": "UN01010661",
                    "unece:cefactBieDomainClass": "cefact:Vessel_Event.Details",
                    "rdfs:comment": "A textual description of this vessel event."
                },
                {
                    "@id": "cefact:IS_Event.Description.Text",
                    "@type": "unece:BasicBIE",
                    "unece:cefactUNId": "UN01012615",
                    "unece:cefactBieDomainClass": "cefact:IS_Event.Details",
                    "rdfs:comment": "A textual description of this IS event."
                },
                {
                    "@id": "cefact:GearInspection_Event.Description.Text",
                    "@type": "unece:BasicBIE",
                    "unece:cefactUNId": "UN01012625",
                    "unece:cefactBieDomainClass": "cefact:GearInspection_Event.Details",
                    "rdfs:comment": "A textual description of this gear inspection event."
                },
                {
                    "@id": "cefact:ISRItem_Characteristic.Description.Text",
                    "@type": "unece:BasicBIE",
                    "unece:cefactUNId": "UN01012604",
                    "unece:cefactBieDomainClass": "cefact:ISRItem_Characteristic.Details",
                    "rdfs:comment": "A textual description of this ISR item characteristic."
                },
                {
                    "@id": "cefact:Gear_Characteristic.Description.Text",
                    "@type": "unece:BasicBIE",
                    "unece:TDED": "7036",
                    "unece:cefactUNId": "UN01010821",
                    "unece:cefactBieDomainClass": "cefact:Gear_Characteristic.Details",
                    "rdfs:comment": "A description, expressed as text, of this gear characteristic."
                },
                {
                    "@id": "cefact:VesselAdministrative_Characteristic.Description.Text",
                    "@type": "unece:BasicBIE",
                    "unece:TDED": "7036",
                    "unece:cefactUNId": "UN01010702",
                    "unece:cefactBieDomainClass": "cefact:VesselAdministrative_Characteristic.Details",
                    "rdfs:comment": "A textual description of this vessel administrative characteristic."
                },
                {
                    "@id": "cefact:FLUX_Characteristic.Description.Text",
                    "@type": "unece:BasicBIE",
                    "unece:TDED": "7036",
                    "unece:cefactUNId": "UN01010867",
                    "unece:cefactBieDomainClass": "cefact:FLUX_Characteristic.Details",
                    "rdfs:comment": "A textual description of this FLUX characteristic."
                },
                {
                    "@id": "cefact:VesselEquipment_Characteristic.Description.Text",
                    "@type": "unece:BasicBIE",
                    "unece:TDED": "7036",
                    "unece:cefactUNId": "UN01010694",
                    "unece:cefactBieDomainClass": "cefact:VesselEquipment_Characteristic.Details",
                    "rdfs:comment": "A textual description of this vessel equipment characteristic."
                },
                {
                    "@id": "cefact:VesselHistorical_Characteristic.Description.Text",
                    "@type": "unece:BasicBIE",
                    "unece:TDED": "7036",
                    "unece:cefactUNId": "UN01010652",
                    "unece:cefactBieDomainClass": "cefact:VesselHistorical_Characteristic.Details",
                    "rdfs:comment": "A textual description of this historical characteristic of a vessel."
                },
                {
                    "@id": "cefact:FLUX_Picture.Description.Text",
                    "@type": "unece:BasicBIE",
                    "unece:cefactUNId": "UN01010734",
                    "unece:cefactBieDomainClass": "cefact:FLUX_Picture.Details",
                    "rdfs:comment": "The textual description of this FLUX picture."
                }
            ]
        },
        {
            "@id": "fisheries:descriptionCode",
            "@type": "rdf:Property",
            "schema:rangeIncludes": {
                "@id": "xsd:token"
            },
            "schema:domainIncludes": {
                "@id": "fisheries:Characteristic"
            },
            "rdfs:comment": "A code specifying a description of this fish catch characteristic.",
            "rdfs:label": "descriptionCode",
            "unece:cefactElementMetadata": [
                {
                    "@id": "cefact:FishCatch_Characteristic.Description.Code",
                    "@type": "unece:BasicBIE",
                    "unece:TDED": "7037",
                    "unece:cefactUNId": "UN01011286",
                    "unece:cefactBieDomainClass": "cefact:FishCatch_Characteristic.Details",
                    "rdfs:comment": "A code specifying a description of this fish catch characteristic."
                }
            ]
        },
        {
            "@id": "fisheries:destinationCharacteristic",
            "@type": "rdf:Property",
            "schema:rangeIncludes": {
                "@id": "fisheries:Characteristic"
            },
            "schema:domainIncludes": {
                "@id": "fisheries:Activity"
            },
            "rdfs:comment": "The characteristic of a vessel storage used as a destination for this fishing activity.",
            "rdfs:label": "destinationCharacteristic",
            "unece:cefactElementMetadata": [
                {
                    "@id": "cefact:Fishing_Activity.Destination.VesselStorage_Characteristic",
                    "@type": "unece:AssociationBIE",
                    "unece:cefactUNId": "UN01011184",
                    "unece:cefactBieDomainClass": "cefact:Fishing_Activity.Details",
                    "rdfs:comment": "The characteristic of a vessel storage used as a destination for this fishing activity."
                }
            ]
        },
        {
            "@id": "fisheries:destinationLocation",
            "@type": "rdf:Property",
            "schema:rangeIncludes": {
                "@id": "fisheries:Location"
            },
            "schema:domainIncludes": {
                "@id": "fisheries:Catch"
            },
            "rdfs:comment": "A Fisheries Language for Universal eXchange (FLUX) destination location for this FA catch.",
            "rdfs:label": "destinationLocation",
            "unece:cefactElementMetadata": [
                {
                    "@id": "cefact:FA_Catch.Destination.FLUX_Location",
                    "@type": "unece:AssociationBIE",
                    "unece:cefactUNId": "UN01011230",
                    "unece:cefactBieDomainClass": "cefact:FA_Catch.Details",
                    "rdfs:comment": "A Fisheries Language for Universal eXchange (FLUX) destination location for this FA catch."
                }
            ]
        },
        {
            "@id": "fisheries:digitalImageBinaryObject",
            "@type": "rdf:Property",
            "schema:rangeIncludes": {
                "@id": "xsd:base64Binary"
            },
            "schema:domainIncludes": {
                "@id": "fisheries:Picture"
            },
            "rdfs:comment": "Binary object data that is the actual digital image for this FLUX picture.",
            "rdfs:label": "digitalImageBinaryObject",
            "unece:cefactElementMetadata": [
                {
                    "@id": "cefact:FLUX_Picture.DigitalImage.BinaryObject",
                    "@type": "unece:BasicBIE",
                    "unece:cefactUNId": "UN01010735",
                    "unece:cefactBieDomainClass": "cefact:FLUX_Picture.Details",
                    "rdfs:comment": "Binary object data that is the actual digital image for this FLUX picture."
                }
            ]
        },
        {
            "@id": "fisheries:discretePeriod",
            "@type": "rdf:Property",
            "schema:rangeIncludes": {
                "@id": "fisheries:Period"
            },
            "schema:domainIncludes": {
                "@id": "fisheries:Event"
            },
            "rdfs:comment": "The discrete delimited period for this vessel event.",
            "rdfs:label": "discretePeriod",
            "unece:cefactElementMetadata": [
                {
                    "@id": "cefact:Vessel_Event.Discrete.Delimited_Period",
                    "@type": "unece:AssociationBIE",
                    "unece:cefactUNId": "UN01010663",
                    "unece:cefactBieDomainClass": "cefact:Vessel_Event.Details",
                    "rdfs:comment": "The discrete delimited period for this vessel event."
                }
            ]
        },
        {
            "@id": "fisheries:draughtMeasure",
            "@type": "rdf:Property",
            "schema:rangeIncludes": {
                "@id": "xsd:decimal"
            },
            "schema:domainIncludes": {
                "@id": "fisheries:TransportMeans"
            },
            "rdfs:comment": "The measure of the draught for this transport means vessel.",
            "rdfs:label": "draughtMeasure",
            "unece:cefactElementMetadata": [
                {
                    "@id": "cefact:Vessel_TransportMeans.Draught.Measure",
                    "@type": "unece:BasicBIE",
                    "unece:cefactUNId": "UN01010640",
                    "unece:cefactBieDomainClass": "cefact:Vessel_TransportMeans.Details",
                    "rdfs:comment": "The measure of the draught for this transport means vessel."
                }
            ]
        },
        {
            "@id": "fisheries:effectivePeriod",
            "@type": "rdf:Property",
            "schema:rangeIncludes": {
                "@id": "fisheries:Period"
            },
            "schema:domainIncludes": [
                {
                    "@id": "fisheries:DataNode"
                },
                {
                    "@id": "fisheries:Document"
                }
            ],
            "rdfs:comment": [
                "The delimited period within which this MDR data node is effective.",
                "The delimited period within which this aggregated catch report document is effective."
            ],
            "rdfs:label": "effectivePeriod",
            "unece:cefactElementMetadata": [
                {
                    "@id": "cefact:AggregatedCatchReport_Document.Effective.Delimited_Period",
                    "@type": "unece:AssociationBIE",
                    "unece:cefactUNId": "UN01010256",
                    "unece:cefactBieDomainClass": "cefact:AggregatedCatchReport_Document.Details",
                    "rdfs:comment": "The delimited period within which this aggregated catch report document is effective."
                },
                {
                    "@id": "cefact:MDR_DataNode.Effective.Delimited_Period",
                    "@type": "unece:AssociationBIE",
                    "unece:cefactUNId": "UN01010593",
                    "unece:cefactBieDomainClass": "cefact:MDR_DataNode.Details",
                    "rdfs:comment": "The delimited period within which this MDR data node is effective."
                }
            ]
        },
        {
            "@id": "fisheries:entryIntoForcePeriod",
            "@type": "rdf:Property",
            "schema:rangeIncludes": {
                "@id": "fisheries:Period"
            },
            "schema:domainIncludes": {
                "@id": "fisheries:Document"
            },
            "rdfs:comment": "The delimited period when this FLAP document enters into force.",
            "rdfs:label": "entryIntoForcePeriod",
            "unece:cefactElementMetadata": [
                {
                    "@id": "cefact:FLAP_Document.EntryIntoForce.Delimited_Period",
                    "@type": "unece:AssociationBIE",
                    "unece:cefactUNId": "UN01010856",
                    "unece:cefactBieDomainClass": "cefact:FLAP_Document.Details",
                    "rdfs:comment": "The delimited period when this FLAP document enters into force."
                }
            ]
        },
        {
            "@id": "fisheries:fADATypeCode",
            "@type": "rdf:Property",
            "schema:rangeIncludes": {
                "@id": "xsd:token"
            },
            "schema:domainIncludes": {
                "@id": "fisheries:Identity"
            },
            "rdfs:comment": "The code specifying the Fishing Authorization Delivering Authority (FADA) type for FLAP identity.",
            "rdfs:label": "fADATypeCode",
            "unece:cefactElementMetadata": [
                {
                    "@id": "cefact:FLAP_Identity.FADA_Type.Code",
                    "@type": "unece:BasicBIE",
                    "unece:cefactUNId": "UN01010897",
                    "unece:cefactBieDomainClass": "cefact:FLAP_Identity.Details",
                    "rdfs:comment": "The code specifying the Fishing Authorization Delivering Authority (FADA) type for FLAP identity."
                }
            ]
        },
        {
            "@id": "fisheries:fAOFishingGearCode",
            "@type": "rdf:Property",
            "schema:rangeIncludes": {
                "@id": "xsd:token"
            },
            "schema:domainIncludes": {
                "@id": "fisheries:ACDRReport"
            },
            "rdfs:comment": "The Food and Agriculture Organization (FAO) code specifying the fishing gear covered by this FLUX ACDR report.",
            "rdfs:label": "fAOFishingGearCode",
            "unece:cefactElementMetadata": [
                {
                    "@id": "cefact:FLUX_ACDRReport.FAO_FishingGear.Code",
                    "@type": "unece:BasicBIE",
                    "unece:cefactUNId": "UN01010273",
                    "unece:cefactBieDomainClass": "cefact:FLUX_ACDRReport.Details",
                    "rdfs:comment": "The Food and Agriculture Organization (FAO) code specifying the fishing gear covered by this FLUX ACDR report."
                }
            ]
        },
        {
            "@id": "fisheries:fAOIdentificationCode",
            "@type": "rdf:Property",
            "schema:rangeIncludes": {
                "@id": "xsd:token"
            },
            "schema:domainIncludes": {
                "@id": "fisheries:ReportedArea"
            },
            "rdfs:comment": "The Food and Agriculture Organization (FAO) code identifying this ACDR reported area.",
            "rdfs:label": "fAOIdentificationCode",
            "unece:cefactElementMetadata": [
                {
                    "@id": "cefact:ACDR_ReportedArea.FAO_Identification.Code",
                    "@type": "unece:BasicBIE",
                    "unece:cefactUNId": "UN01010259",
                    "unece:cefactBieDomainClass": "cefact:ACDR_ReportedArea.Details",
                    "rdfs:comment": "The Food and Agriculture Organization (FAO) code identifying this ACDR reported area."
                }
            ]
        },
        {
            "@id": "fisheries:fAOSpeciesCode",
            "@type": "rdf:Property",
            "schema:rangeIncludes": {
                "@id": "xsd:token"
            },
            "schema:domainIncludes": {
                "@id": "fisheries:Catch"
            },
            "rdfs:comment": "The Food and Agriculture Organisation (FAO) species code for this ACDR catch.",
            "rdfs:label": "fAOSpeciesCode",
            "unece:cefactElementMetadata": [
                {
                    "@id": "cefact:ACDR_Catch.FAO_Species.Code",
                    "@type": "unece:BasicBIE",
                    "unece:cefactUNId": "UN01010265",
                    "unece:cefactBieDomainClass": "cefact:ACDR_Catch.Details",
                    "rdfs:comment": "The Food and Agriculture Organisation (FAO) species code for this ACDR catch."
                }
            ]
        },
        {
            "@id": "fisheries:fAReportDocumentTypeCode",
            "@type": "rdf:Property",
            "schema:rangeIncludes": {
                "@id": "unece:UNECECL1001Code"
            },
            "schema:domainIncludes": {
                "@id": "fisheries:Document"
            },
            "rdfs:comment": "The code specifying a type of FA report document, such as a declaration or notification.",
            "rdfs:label": "fAReportDocumentTypeCode",
            "unece:cefactElementMetadata": [
                {
                    "@id": "cefact:FAReport_Document.Type.Code",
                    "@type": "unece:BasicBIE",
                    "unece:TDED": "1001",
                    "unece:cefactUNId": "UN01011157",
                    "unece:cefactBieDomainClass": "cefact:FAReport_Document.Details",
                    "rdfs:comment": "The code specifying a type of FA report document, such as a declaration or notification."
                }
            ]
        },
        {
            "@id": "fisheries:fCTypeCode",
            "@type": "rdf:Property",
            "schema:rangeIncludes": {
                "@id": "xsd:token"
            },
            "schema:domainIncludes": {
                "@id": "fisheries:Identity"
            },
            "rdfs:comment": "The code specifying the type of Fishing Category (FC) of FLAP identity.",
            "rdfs:label": "fCTypeCode",
            "unece:cefactElementMetadata": [
                {
                    "@id": "cefact:FLAP_Identity.FC_Type.Code",
                    "@type": "unece:BasicBIE",
                    "unece:cefactUNId": "UN01010898",
                    "unece:cefactBieDomainClass": "cefact:FLAP_Identity.Details",
                    "rdfs:comment": "The code specifying the type of Fishing Category (FC) of FLAP identity."
                }
            ]
        },
        {
            "@id": "fisheries:fLAPDocumentTypeCode",
            "@type": "rdf:Property",
            "schema:rangeIncludes": {
                "@id": "unece:UNECECL1001Code"
            },
            "schema:domainIncludes": {
                "@id": "fisheries:Document"
            },
            "rdfs:comment": "The code specifying the type of FLAP document.",
            "rdfs:label": "fLAPDocumentTypeCode",
            "unece:cefactElementMetadata": [
                {
                    "@id": "cefact:FLAP_Document.Type.Code",
                    "@type": "unece:BasicBIE",
                    "unece:TDED": "1001",
                    "unece:cefactUNId": "UN01011005",
                    "unece:cefactBieDomainClass": "cefact:FLAP_Document.Details",
                    "rdfs:comment": "The code specifying the type of FLAP document."
                }
            ]
        },
        {
            "@id": "fisheries:fLAPRequestDocumentFADATypeCode",
            "@type": "rdf:Property",
            "schema:rangeIncludes": {
                "@id": "unece:UNECECL1001Code"
            },
            "schema:domainIncludes": {
                "@id": "fisheries:Document"
            },
            "rdfs:comment": "The code specifying a type of Fishing Authorization Delivering Authority (FADA) for this FLAP request document.",
            "rdfs:label": "fLAPRequestDocumentFADATypeCode",
            "unece:cefactElementMetadata": [
                {
                    "@id": "cefact:FLAPRequest_Document.FADA_Type.Code",
                    "@type": "unece:BasicBIE",
                    "unece:TDED": "1001",
                    "unece:cefactUNId": "UN01010832",
                    "unece:cefactBieDomainClass": "cefact:FLAPRequest_Document.Details",
                    "rdfs:comment": "The code specifying a type of Fishing Authorization Delivering Authority (FADA) for this FLAP request document."
                }
            ]
        },
        {
            "@id": "fisheries:fLAPRequestDocumentPurposeCode",
            "@type": "rdf:Property",
            "schema:rangeIncludes": {
                "@id": "unece:UNECECL1225Code"
            },
            "schema:domainIncludes": {
                "@id": "fisheries:Document"
            },
            "rdfs:comment": "The code specifying the purpose for this FLAP request document, such as withdrawal or termination.",
            "rdfs:label": "fLAPRequestDocumentPurposeCode",
            "unece:cefactElementMetadata": [
                {
                    "@id": "cefact:FLAPRequest_Document.Purpose.Code",
                    "@type": "unece:BasicBIE",
                    "unece:TDED": "1225",
                    "unece:cefactUNId": "UN01010833",
                    "unece:cefactBieDomainClass": "cefact:FLAPRequest_Document.Details",
                    "rdfs:comment": "The code specifying the purpose for this FLAP request document, such as withdrawal or termination."
                }
            ]
        },
        {
            "@id": "fisheries:fLAPRequestDocumentTypeCode",
            "@type": "rdf:Property",
            "schema:rangeIncludes": {
                "@id": "unece:UNECECL1001Code"
            },
            "schema:domainIncludes": {
                "@id": "fisheries:Document"
            },
            "rdfs:comment": "The code specifying a type of FLAP request document.",
            "rdfs:label": "fLAPRequestDocumentTypeCode",
            "unece:cefactElementMetadata": [
                {
                    "@id": "cefact:FLAPRequest_Document.Type.Code",
                    "@type": "unece:BasicBIE",
                    "unece:TDED": "1001",
                    "unece:cefactUNId": "UN01010831",
                    "unece:cefactBieDomainClass": "cefact:FLAPRequest_Document.Details",
                    "rdfs:comment": "The code specifying a type of FLAP request document."
                }
            ]
        },
        {
            "@id": "fisheries:fLUXCharacteristicValueCode",
            "@type": "rdf:Property",
            "schema:rangeIncludes": {
                "@id": "unece:UNECECL7111Code"
            },
            "schema:domainIncludes": {
                "@id": "fisheries:Characteristic"
            },
            "rdfs:comment": "The code specifying a value of this FLUX characteristic.",
            "rdfs:label": "fLUXCharacteristicValueCode",
            "unece:cefactElementMetadata": [
                {
                    "@id": "cefact:FLUX_Characteristic.Value.Code",
                    "@type": "unece:BasicBIE",
                    "unece:TDED": "7111",
                    "unece:cefactUNId": "UN01010871",
                    "unece:cefactBieDomainClass": "cefact:FLUX_Characteristic.Details",
                    "rdfs:comment": "The code specifying a value of this FLUX characteristic."
                }
            ]
        },
        {
            "@id": "fisheries:fLUXLocationTypeCode",
            "@type": "rdf:Property",
            "schema:rangeIncludes": {
                "@id": "unece:UNECECL3227Code"
            },
            "schema:domainIncludes": {
                "@id": "fisheries:Location"
            },
            "rdfs:comment": "The code specifying the type of FLUX location.",
            "rdfs:label": "fLUXLocationTypeCode",
            "unece:cefactElementMetadata": [
                {
                    "@id": "cefact:FLUX_Location.Type.Code",
                    "@type": "unece:BasicBIE",
                    "unece:TDED": "3227",
                    "unece:cefactUNId": "UN01010960",
                    "unece:cefactBieDomainClass": "cefact:FLUX_Location.Details",
                    "rdfs:comment": "The code specifying the type of FLUX location."
                }
            ]
        },
        {
            "@id": "fisheries:fLUXReportDocumentPurposeCode",
            "@type": "rdf:Property",
            "schema:rangeIncludes": {
                "@id": "unece:UNECECL1225Code"
            },
            "schema:domainIncludes": {
                "@id": "fisheries:Document"
            },
            "rdfs:comment": "The code specifying the purpose of this FLUX report document, such as original, cancellation or replace.",
            "rdfs:label": "fLUXReportDocumentPurposeCode",
            "unece:cefactElementMetadata": [
                {
                    "@id": "cefact:FLUXReport_Document.Purpose.Code",
                    "@type": "unece:BasicBIE",
                    "unece:TDED": "1225",
                    "unece:cefactUNId": "UN01010242",
                    "unece:cefactBieDomainClass": "cefact:FLUXReport_Document.Details",
                    "rdfs:comment": "The code specifying the purpose of this FLUX report document, such as original, cancellation or replace."
                }
            ]
        },
        {
            "@id": "fisheries:fLUXReportDocumentTypeCode",
            "@type": "rdf:Property",
            "schema:rangeIncludes": {
                "@id": "unece:UNECECL1001Code"
            },
            "schema:domainIncludes": {
                "@id": "fisheries:Document"
            },
            "rdfs:comment": "The code specifying the type of this FLUX report document.",
            "rdfs:label": "fLUXReportDocumentTypeCode",
            "unece:cefactElementMetadata": [
                {
                    "@id": "cefact:FLUXReport_Document.Type.Code",
                    "@type": "unece:BasicBIE",
                    "unece:TDED": "1001",
                    "unece:cefactUNId": "UN01010760",
                    "unece:cefactBieDomainClass": "cefact:FLUXReport_Document.Details",
                    "rdfs:comment": "The code specifying the type of this FLUX report document."
                }
            ]
        },
        {
            "@id": "fisheries:fLUXResponseDocumentTypeCode",
            "@type": "rdf:Property",
            "schema:rangeIncludes": {
                "@id": "unece:UNECECL1001Code"
            },
            "schema:domainIncludes": {
                "@id": "fisheries:Document"
            },
            "rdfs:comment": "The code specifying the type of this FLUX response document.",
            "rdfs:label": "fLUXResponseDocumentTypeCode",
            "unece:cefactElementMetadata": [
                {
                    "@id": "cefact:FLUXResponse_Document.Type.Code",
                    "@type": "unece:BasicBIE",
                    "unece:TDED": "1001",
                    "unece:cefactUNId": "UN01010761",
                    "unece:cefactBieDomainClass": "cefact:FLUXResponse_Document.Details",
                    "rdfs:comment": "The code specifying the type of this FLUX response document."
                }
            ]
        },
        {
            "@id": "fisheries:fMCMarkerCode",
            "@type": "rdf:Property",
            "schema:rangeIncludes": {
                "@id": "xsd:token"
            },
            "schema:domainIncludes": {
                "@id": "fisheries:Document"
            },
            "rdfs:comment": "The code specifying a marker set by a Fishing Monitoring Centre (FMC) in this FA report document, such as original or modified by FMC.",
            "rdfs:label": "fMCMarkerCode",
            "unece:cefactElementMetadata": [
                {
                    "@id": "cefact:FAReport_Document.FMC_Marker.Code",
                    "@type": "unece:BasicBIE",
                    "unece:cefactUNId": "UN01011158",
                    "unece:cefactBieDomainClass": "cefact:FAReport_Document.Details",
                    "rdfs:comment": "The code specifying a marker set by a Fishing Monitoring Centre (FMC) in this FA report document, such as original or modified by FMC."
                }
            ]
        },
        {
            "@id": "fisheries:faxCommunication",
            "@type": "rdf:Property",
            "schema:rangeIncludes": {
                "@id": "fisheries:Communication"
            },
            "schema:domainIncludes": {
                "@id": "fisheries:Party"
            },
            "rdfs:comment": "Facsimile (FAX) communication information for this contact party.",
            "rdfs:label": "faxCommunication",
            "unece:cefactElementMetadata": [
                {
                    "@id": "cefact:Contact_Party.Fax.Telecommunication_Communication",
                    "@type": "unece:AssociationBIE",
                    "unece:cefactUNId": "UN01010787",
                    "unece:cefactBieDomainClass": "cefact:Contact_Party.Details",
                    "rdfs:comment": "Facsimile (FAX) communication information for this contact party."
                }
            ]
        },
        {
            "@id": "fisheries:firstApplicationIndicator",
            "@type": "rdf:Property",
            "schema:rangeIncludes": {
                "@id": "xsd:boolean"
            },
            "schema:domainIncludes": {
                "@id": "fisheries:Document"
            },
            "rdfs:comment": "The indication of whether or not this is the first application for this FLAP document.",
            "rdfs:label": "firstApplicationIndicator",
            "unece:cefactElementMetadata": [
                {
                    "@id": "cefact:FLAP_Document.First_Application.Indicator",
                    "@type": "unece:BasicBIE",
                    "unece:cefactUNId": "UN01010850",
                    "unece:cefactBieDomainClass": "cefact:FLAP_Document.Details",
                    "rdfs:comment": "The indication of whether or not this is the first application for this FLAP document."
                }
            ]
        },
        {
            "@id": "fisheries:fisheryTypeCode",
            "@type": "rdf:Property",
            "schema:rangeIncludes": {
                "@id": "xsd:token"
            },
            "schema:domainIncludes": {
                "@id": "fisheries:Activity"
            },
            "rdfs:comment": "The code specifying a type of fishery for this fishing activity, such as pelagic fisheries.",
            "rdfs:label": "fisheryTypeCode",
            "unece:cefactElementMetadata": [
                {
                    "@id": "cefact:Fishing_Activity.Fishery_Type.Code",
                    "@type": "unece:BasicBIE",
                    "unece:cefactUNId": "UN01011174",
                    "unece:cefactBieDomainClass": "cefact:Fishing_Activity.Details",
                    "rdfs:comment": "The code specifying a type of fishery for this fishing activity, such as pelagic fisheries."
                }
            ]
        },
        {
            "@id": "fisheries:fishingArea",
            "@type": "rdf:Property",
            "schema:rangeIncludes": {
                "@id": "xsd:string"
            },
            "schema:domainIncludes": {
                "@id": "fisheries:Category"
            },
            "rdfs:comment": "A fishing area, expressed as text, for this fishing category.",
            "rdfs:label": "fishingArea",
            "unece:cefactElementMetadata": [
                {
                    "@id": "cefact:Fishing_Category.Fishing_Area.Text",
                    "@type": "unece:BasicBIE",
                    "unece:cefactUNId": "UN01010842",
                    "unece:cefactBieDomainClass": "cefact:Fishing_Category.Details",
                    "rdfs:comment": "A fishing area, expressed as text, for this fishing category."
                }
            ]
        },
        {
            "@id": "fisheries:fishingAreaCode",
            "@type": "rdf:Property",
            "schema:rangeIncludes": {
                "@id": "xsd:token"
            },
            "schema:domainIncludes": {
                "@id": "fisheries:Category"
            },
            "rdfs:comment": "A code, such as a Food & Agriculture Organization (FAO) area code, specifying the fishing area for this fishing category.",
            "rdfs:label": "fishingAreaCode",
            "unece:cefactElementMetadata": [
                {
                    "@id": "cefact:Fishing_Category.Fishing_Area.Code",
                    "@type": "unece:BasicBIE",
                    "unece:cefactUNId": "UN01010841",
                    "unece:cefactBieDomainClass": "cefact:Fishing_Category.Details",
                    "rdfs:comment": "A code, such as a Food & Agriculture Organization (FAO) area code, specifying the fishing area for this fishing category."
                }
            ]
        },
        {
            "@id": "fisheries:fishingCategoryCode",
            "@type": "rdf:Property",
            "schema:rangeIncludes": {
                "@id": "xsd:token"
            },
            "schema:domainIncludes": {
                "@id": "fisheries:ACDRReport"
            },
            "rdfs:comment": "The code specifying a fishing category, such as the type of vessel, the type of fishing activity or the fishing gear deployed, in this FLUX ACDR report.",
            "rdfs:label": "fishingCategoryCode",
            "unece:cefactElementMetadata": [
                {
                    "@id": "cefact:FLUX_ACDRReport.FishingCategory.Code",
                    "@type": "unece:BasicBIE",
                    "unece:cefactUNId": "UN01010272",
                    "unece:cefactBieDomainClass": "cefact:FLUX_ACDRReport.Details",
                    "rdfs:comment": "The code specifying a fishing category, such as the type of vessel, the type of fishing activity or the fishing gear deployed, in this FLUX ACDR report."
                }
            ]
        },
        {
            "@id": "fisheries:fishingDurationMeasure",
            "@type": "rdf:Property",
            "schema:rangeIncludes": {
                "@id": "xsd:decimal"
            },
            "schema:domainIncludes": {
                "@id": "fisheries:Activity"
            },
            "rdfs:comment": "The measure of a duration for this fishing activity.",
            "rdfs:label": "fishingDurationMeasure",
            "unece:cefactElementMetadata": [
                {
                    "@id": "cefact:Fishing_Activity.Fishing_Duration.Measure",
                    "@type": "unece:BasicBIE",
                    "unece:cefactUNId": "UN01011177",
                    "unece:cefactBieDomainClass": "cefact:Fishing_Activity.Details",
                    "rdfs:comment": "The measure of a duration for this fishing activity."
                }
            ]
        },
        {
            "@id": "fisheries:fishingMethod",
            "@type": "rdf:Property",
            "schema:rangeIncludes": {
                "@id": "xsd:string"
            },
            "schema:domainIncludes": {
                "@id": "fisheries:Category"
            },
            "rdfs:comment": "A fishing method, expressed as text, for this fishing category.",
            "rdfs:label": "fishingMethod",
            "unece:cefactElementMetadata": [
                {
                    "@id": "cefact:Fishing_Category.Fishing_Method.Text",
                    "@type": "unece:BasicBIE",
                    "unece:cefactUNId": "UN01010840",
                    "unece:cefactBieDomainClass": "cefact:Fishing_Category.Details",
                    "rdfs:comment": "A fishing method, expressed as text, for this fishing category."
                }
            ]
        },
        {
            "@id": "fisheries:fishingMethodCode",
            "@type": "rdf:Property",
            "schema:rangeIncludes": {
                "@id": "xsd:token"
            },
            "schema:domainIncludes": {
                "@id": "fisheries:Category"
            },
            "rdfs:comment": "A code specifying the type of fishing method for this fishing category.",
            "rdfs:label": "fishingMethodCode",
            "unece:cefactElementMetadata": [
                {
                    "@id": "cefact:Fishing_Category.Fishing_Method.Code",
                    "@type": "unece:BasicBIE",
                    "unece:cefactUNId": "UN01010839",
                    "unece:cefactBieDomainClass": "cefact:Fishing_Category.Details",
                    "rdfs:comment": "A code specifying the type of fishing method for this fishing category."
                }
            ]
        },
        {
            "@id": "fisheries:gearCharacteristicValueCode",
            "@type": "rdf:Property",
            "schema:rangeIncludes": {
                "@id": "unece:UNECECL7111Code"
            },
            "schema:domainIncludes": {
                "@id": "fisheries:Characteristic"
            },
            "rdfs:comment": "The code specifying a value of this gear characteristic.",
            "rdfs:label": "gearCharacteristicValueCode",
            "unece:cefactElementMetadata": [
                {
                    "@id": "cefact:Gear_Characteristic.Value.Code",
                    "@type": "unece:BasicBIE",
                    "unece:TDED": "7111",
                    "unece:cefactUNId": "UN01010825",
                    "unece:cefactBieDomainClass": "cefact:Gear_Characteristic.Details",
                    "rdfs:comment": "The code specifying a value of this gear characteristic."
                }
            ]
        },
        {
            "@id": "fisheries:geopoliticalRegionCode",
            "@type": "rdf:Property",
            "schema:rangeIncludes": {
                "@id": "xsd:token"
            },
            "schema:domainIncludes": {
                "@id": "fisheries:Location"
            },
            "rdfs:comment": "The code specifying the geopolitical region for this FLUX location.",
            "rdfs:label": "geopoliticalRegionCode",
            "unece:cefactElementMetadata": [
                {
                    "@id": "cefact:FLUX_Location.GeopoliticalRegion.Code",
                    "@type": "unece:BasicBIE",
                    "unece:cefactUNId": "UN01010963",
                    "unece:cefactBieDomainClass": "cefact:FLUX_Location.Details",
                    "rdfs:comment": "The code specifying the geopolitical region for this FLUX location."
                }
            ]
        },
        {
            "@id": "fisheries:grantedDocument",
            "@type": "rdf:Property",
            "schema:rangeIncludes": {
                "@id": "fisheries:Document"
            },
            "schema:domainIncludes": {
                "@id": "fisheries:TransportMeans"
            },
            "rdfs:comment": "A Fishing Licence, Authorization, Permit (FLAP) document granted to this vessel transport means.",
            "rdfs:label": "grantedDocument",
            "unece:cefactElementMetadata": [
                {
                    "@id": "cefact:Vessel_TransportMeans.Granted.FLAP_Document",
                    "@type": "unece:AssociationBIE",
                    "unece:cefactUNId": "UN01011214",
                    "unece:cefactBieDomainClass": "cefact:Vessel_TransportMeans.Details",
                    "rdfs:comment": "A Fishing Licence, Authorization, Permit (FLAP) document granted to this vessel transport means."
                }
            ]
        },
        {
            "@id": "fisheries:hierarchicalLevelNumeric",
            "@type": "rdf:Property",
            "schema:rangeIncludes": {
                "@id": "xsd:decimal"
            },
            "schema:domainIncludes": {
                "@id": "fisheries:DataNode"
            },
            "rdfs:comment": "The number (integer) representing how deeply nested within the hierarchical tree structure the MDR data node lies.  For example, level 1 may mean it is a top level node, and level 4 may mean that there are three levels of nodes above this node in the tree.",
            "rdfs:label": "hierarchicalLevelNumeric",
            "unece:cefactElementMetadata": [
                {
                    "@id": "cefact:MDR_DataNode.HierarchicalLevel.Numeric",
                    "@type": "unece:BasicBIE",
                    "unece:cefactUNId": "UN01010592",
                    "unece:cefactBieDomainClass": "cefact:MDR_DataNode.Details",
                    "rdfs:comment": "The number (integer) representing how deeply nested within the hierarchical tree structure the MDR data node lies.  For example, level 1 may mean it is a top level node, and level 4 may mean that there are three levels of nodes above this node in the tree."
                }
            ]
        },
        {
            "@id": "fisheries:hullMaterialCode",
            "@type": "rdf:Property",
            "schema:rangeIncludes": {
                "@id": "xsd:token"
            },
            "schema:domainIncludes": {
                "@id": "fisheries:TransportMeans"
            },
            "rdfs:comment": "The code indicating the material of the hull for this vessel transport means.",
            "rdfs:label": "hullMaterialCode",
            "unece:cefactElementMetadata": [
                {
                    "@id": "cefact:Vessel_TransportMeans.HullMaterial.Code",
                    "@type": "unece:BasicBIE",
                    "unece:cefactUNId": "UN01010639",
                    "unece:cefactBieDomainClass": "cefact:Vessel_TransportMeans.Details",
                    "rdfs:comment": "The code indicating the material of the hull for this vessel transport means."
                }
            ]
        },
        {
            "@id": "fisheries:id",
            "@type": "rdf:Property",
            "schema:rangeIncludes": {
                "@id": "xsd:token"
            },
            "schema:domainIncludes": [
                {
                    "@id": "fisheries:Activity"
                },
                {
                    "@id": "fisheries:Batch"
                },
                {
                    "@id": "fisheries:Characteristic"
                },
                {
                    "@id": "fisheries:Country"
                },
                {
                    "@id": "fisheries:DataNode"
                },
                {
                    "@id": "fisheries:DataSet"
                },
                {
                    "@id": "fisheries:Document"
                },
                {
                    "@id": "fisheries:Event"
                },
                {
                    "@id": "fisheries:Identity"
                },
                {
                    "@id": "fisheries:Location"
                },
                {
                    "@id": "fisheries:Means"
                },
                {
                    "@id": "fisheries:Party"
                },
                {
                    "@id": "fisheries:Picture"
                },
                {
                    "@id": "fisheries:QualityAnalysis"
                },
                {
                    "@id": "fisheries:Query"
                },
                {
                    "@id": "fisheries:Report"
                },
                {
                    "@id": "fisheries:Stock"
                },
                {
                    "@id": "fisheries:TransportMeans"
                },
                {
                    "@id": "fisheries:Trip"
                },
                {
                    "@id": "fisheries:Version"
                }
            ],
            "rdfs:comment": [
                "An identification, such as RFC4122 Universally Unique IDentifier (UUID) or a human readable identifier, of this FLUX report document.",
                "An identification, such as RFC4122 Universally Unique IDentifier (UUID) or a human readable identifier, of this FLUX response document.",
                "An identifier for this IS report.",
                "An identifier for this MDR data set.",
                "An identifier for this fish catch characteristic.",
                "An identifier for this fishing activity.",
                "An identifier for this gear inspection event.",
                "An identifier for this sales batch.",
                "An identifier for this sales document.",
                "An identifier for this transport means vessel, such as an identifier defined by the Food and Agriculture Organisation (FAO), the radio call sign, or an external marking.",
                "An identifier for this vessel event.",
                "An identifier of this FLUX party.",
                "An identifier, such as International Radio Call Sign (IRCS) or a Regional Fisheries Management Organization (RFMO) reference, for this surveillance means.",
                "An identifier, such as an RFC 4122 Universally Unique IDentifier (UUID), for this fishing trip.",
                "The identification of this quality analysis of a validation process.",
                "The identifier for this AAP stock.",
                "The identifier for this FA query.",
                "The identifier for this FLAP document.",
                "The identifier for this FLAP identity.",
                "The identifier for this FLAP request document.",
                "The identifier for this FLUX location, such as a United Nations Location Code (UNLOCODE).",
                "The identifier for this IS event.",
                "The identifier for this ISR query.",
                "The identifier for this MDR data node.",
                "The identifier for this MDR query identity.",
                "The identifier for this MDR query.",
                "The identifier for this data set version.",
                "The identifier for this gear equipment inspection event.",
                "The identifier for this sales party.",
                "The identifier for this sales query.",
                "The identifier for this sales report.",
                "The identifier for this vessel country.",
                "The identifier for this vessel position query.",
                "The identifier for this vessel query.",
                "The identifier for this vessel storage characteristic.",
                "The identifier of this FLUX picture.",
                "The identifier of this vehicle transport means."
            ],
            "rdfs:label": "id",
            "unece:cefactElementMetadata": [
                {
                    "@id": "cefact:Sales_Batch.Identification.Identifier",
                    "@type": "unece:BasicBIE",
                    "unece:cefactUNId": "UN01010930",
                    "unece:cefactBieDomainClass": "cefact:Sales_Batch.Details",
                    "rdfs:comment": "An identifier for this sales batch."
                },
                {
                    "@id": "cefact:VesselStorage_Characteristic.Identification.Identifier",
                    "@type": "unece:BasicBIE",
                    "unece:cefactUNId": "UN01011215",
                    "unece:cefactBieDomainClass": "cefact:VesselStorage_Characteristic.Details",
                    "rdfs:comment": "The identifier for this vessel storage characteristic."
                },
                {
                    "@id": "cefact:Vessel_TransportMeans.Identification.Identifier",
                    "@type": "unece:BasicBIE",
                    "unece:TDED": "8213",
                    "unece:cefactUNId": "UN01010228",
                    "unece:cefactBieDomainClass": "cefact:Vessel_TransportMeans.Details",
                    "rdfs:comment": "An identifier for this transport means vessel, such as an identifier defined by the Food and Agriculture Organisation (FAO), the radio call sign, or an external marking."
                },
                {
                    "@id": "cefact:DataSet_Version.Identification.Identifier",
                    "@type": "unece:BasicBIE",
                    "unece:cefactUNId": "UN01010599",
                    "unece:cefactBieDomainClass": "cefact:DataSet_Version.Details",
                    "rdfs:comment": "The identifier for this data set version."
                },
                {
                    "@id": "cefact:FLUX_Picture.Identification.Identifier",
                    "@type": "unece:BasicBIE",
                    "unece:cefactUNId": "UN01010730",
                    "unece:cefactBieDomainClass": "cefact:FLUX_Picture.Details",
                    "rdfs:comment": "The identifier of this FLUX picture."
                },
                {
                    "@id": "cefact:Vessel_Query.Identification.Identifier",
                    "@type": "unece:BasicBIE",
                    "unece:cefactUNId": "UN01010759",
                    "unece:cefactBieDomainClass": "cefact:Vessel_Query.Details",
                    "rdfs:comment": "The identifier for this vessel query."
                },
                {
                    "@id": "cefact:Fishing_Activity.Identification.Identifier",
                    "@type": "unece:BasicBIE",
                    "unece:cefactUNId": "UN01011169",
                    "unece:cefactBieDomainClass": "cefact:Fishing_Activity.Details",
                    "rdfs:comment": "An identifier for this fishing activity."
                },
                {
                    "@id": "cefact:MDR_DataSet.Identification.Identifier",
                    "@type": "unece:BasicBIE",
                    "unece:cefactUNId": "UN01010583",
                    "unece:cefactBieDomainClass": "cefact:MDR_DataSet.Details",
                    "rdfs:comment": "An identifier for this MDR data set."
                },
                {
                    "@id": "cefact:Fishing_Trip.Identification.Identifier",
                    "@type": "unece:BasicBIE",
                    "unece:cefactUNId": "UN01011165",
                    "unece:cefactBieDomainClass": "cefact:Fishing_Trip.Details",
                    "rdfs:comment": "An identifier, such as an RFC 4122 Universally Unique IDentifier (UUID), for this fishing trip."
                },
                {
                    "@id": "cefact:ISR_Query.Identification.Identifier",
                    "@type": "unece:BasicBIE",
                    "unece:cefactUNId": "UN01012635",
                    "unece:cefactBieDomainClass": "cefact:ISR_Query.Details",
                    "rdfs:comment": "The identifier for this ISR query."
                },
                {
                    "@id": "cefact:Sales_Document.Identification.Identifier",
                    "@type": "unece:BasicBIE",
                    "unece:TDED": "1004",
                    "unece:cefactUNId": "UN01010910",
                    "unece:cefactBieDomainClass": "cefact:Sales_Document.Details",
                    "rdfs:comment": "An identifier for this sales document."
                },
                {
                    "@id": "cefact:FLAPRequest_Document.Identification.Identifier",
                    "@type": "unece:BasicBIE",
                    "unece:TDED": "1004",
                    "unece:cefactUNId": "UN01010830",
                    "unece:cefactBieDomainClass": "cefact:FLAPRequest_Document.Details",
                    "rdfs:comment": "The identifier for this FLAP request document."
                },
                {
                    "@id": "cefact:Vessel_Event.Identification.Identifier",
                    "@type": "unece:BasicBIE",
                    "unece:TDED": "1007",
                    "unece:cefactUNId": "UN01013076",
                    "unece:cefactBieDomainClass": "cefact:Vessel_Event.Details",
                    "rdfs:comment": "An identifier for this vessel event."
                },
                {
                    "@id": "cefact:FLUXReport_Document.Identification.Identifier",
                    "@type": "unece:BasicBIE",
                    "unece:TDED": "1004",
                    "unece:cefactUNId": "UN01010239",
                    "unece:cefactBieDomainClass": "cefact:FLUXReport_Document.Details",
                    "rdfs:comment": "An identification, such as RFC4122 Universally Unique IDentifier (UUID) or a human readable identifier, of this FLUX report document."
                },
                {
                    "@id": "cefact:IS_Event.Identification.Identifier",
                    "@type": "unece:BasicBIE",
                    "unece:cefactUNId": "UN01012614",
                    "unece:cefactBieDomainClass": "cefact:IS_Event.Details",
                    "rdfs:comment": "The identifier for this IS event."
                },
                {
                    "@id": "cefact:FLUXResponse_Document.Identification.Identifier",
                    "@type": "unece:BasicBIE",
                    "unece:TDED": "1004",
                    "unece:cefactUNId": "UN01010249",
                    "unece:cefactBieDomainClass": "cefact:FLUXResponse_Document.Details",
                    "rdfs:comment": "An identification, such as RFC4122 Universally Unique IDentifier (UUID) or a human readable identifier, of this FLUX response document."
                },
                {
                    "@id": "cefact:Surveillance_Means.Identification.Identifier",
                    "@type": "unece:BasicBIE",
                    "unece:cefactUNId": "UN01012630",
                    "unece:cefactBieDomainClass": "cefact:Surveillance_Means.Details",
                    "rdfs:comment": "An identifier, such as International Radio Call Sign (IRCS) or a Regional Fisheries Management Organization (RFMO) reference, for this surveillance means."
                },
                {
                    "@id": "cefact:Validation_QualityAnalysis.Identification.Identifier",
                    "@type": "unece:BasicBIE",
                    "unece:cefactUNId": "UN01010765",
                    "unece:cefactBieDomainClass": "cefact:Validation_QualityAnalysis.Details",
                    "rdfs:comment": "The identification of this quality analysis of a validation process."
                },
                {
                    "@id": "cefact:FishCatch_Characteristic.Identification.Identifier",
                    "@type": "unece:BasicBIE",
                    "unece:cefactUNId": "UN01011283",
                    "unece:cefactBieDomainClass": "cefact:FishCatch_Characteristic.Details",
                    "rdfs:comment": "An identifier for this fish catch characteristic."
                },
                {
                    "@id": "cefact:MDRQuery_Identity.Identification.Identifier",
                    "@type": "unece:BasicBIE",
                    "unece:cefactUNId": "UN01010578",
                    "unece:cefactBieDomainClass": "cefact:MDRQuery_Identity.Details",
                    "rdfs:comment": "The identifier for this MDR query identity."
                },
                {
                    "@id": "cefact:Sales_Party.Identification.Identifier",
                    "@type": "unece:BasicBIE",
                    "unece:TDED": "3039",
                    "unece:cefactUNId": "UN01010923",
                    "unece:cefactBieDomainClass": "cefact:Sales_Party.Details",
                    "rdfs:comment": "The identifier for this sales party."
                },
                {
                    "@id": "cefact:AAP_Stock.Identification.Identifier",
                    "@type": "unece:BasicBIE",
                    "unece:cefactUNId": "UN01011200",
                    "unece:cefactBieDomainClass": "cefact:AAP_Stock.Details",
                    "rdfs:comment": "The identifier for this AAP stock."
                },
                {
                    "@id": "cefact:MDR_DataNode.Identification.Identifier",
                    "@type": "unece:BasicBIE",
                    "unece:cefactUNId": "UN01010590",
                    "unece:cefactBieDomainClass": "cefact:MDR_DataNode.Details",
                    "rdfs:comment": "The identifier for this MDR data node."
                },
                {
                    "@id": "cefact:Sales_Query.Identification.Identifier",
                    "@type": "unece:BasicBIE",
                    "unece:cefactUNId": "UN01010994",
                    "unece:cefactBieDomainClass": "cefact:Sales_Query.Details",
                    "rdfs:comment": "The identifier for this sales query."
                },
                {
                    "@id": "cefact:FLUX_Party.Identification.Identifier",
                    "@type": "unece:BasicBIE",
                    "unece:TDED": "3039",
                    "unece:cefactUNId": "UN01010246",
                    "unece:cefactBieDomainClass": "cefact:FLUX_Party.Details",
                    "rdfs:comment": "An identifier of this FLUX party."
                },
                {
                    "@id": "cefact:GearInspection_Event.Identification.Identifier",
                    "@type": "unece:BasicBIE",
                    "unece:cefactUNId": "UN01012624",
                    "unece:cefactBieDomainClass": "cefact:GearInspection_Event.Details",
                    "rdfs:comment": "An identifier for this gear inspection event."
                },
                {
                    "@id": "cefact:FLUX_Location.Identification.Identifier",
                    "@type": "unece:BasicBIE",
                    "unece:TDED": "3225",
                    "unece:cefactUNId": "UN01010962",
                    "unece:cefactBieDomainClass": "cefact:FLUX_Location.Details",
                    "rdfs:comment": "The identifier for this FLUX location, such as a United Nations Location Code (UNLOCODE)."
                },
                {
                    "@id": "cefact:FLAP_Identity.Identification.Identifier",
                    "@type": "unece:BasicBIE",
                    "unece:cefactUNId": "UN01010895",
                    "unece:cefactBieDomainClass": "cefact:FLAP_Identity.Details",
                    "rdfs:comment": "The identifier for this FLAP identity."
                },
                {
                    "@id": "cefact:GearEquipmentInspection_Event.Identification.Identifier",
                    "@type": "unece:BasicBIE",
                    "unece:TDED": "1007",
                    "unece:cefactUNId": "UN01013330",
                    "unece:cefactBieDomainClass": "cefact:GearEquipmentInspection_Event.Details",
                    "rdfs:comment": "The identifier for this gear equipment inspection event."
                },
                {
                    "@id": "cefact:IS_Report.Identification.Identifier",
                    "@type": "unece:BasicBIE",
                    "unece:cefactUNId": "UN01013339",
                    "unece:cefactBieDomainClass": "cefact:IS_Report.Details",
                    "rdfs:comment": "An identifier for this IS report."
                },
                {
                    "@id": "cefact:FA_Query.Identification.Identifier",
                    "@type": "unece:BasicBIE",
                    "unece:cefactUNId": "UN01011218",
                    "unece:cefactBieDomainClass": "cefact:FA_Query.Details",
                    "rdfs:comment": "The identifier for this FA query."
                },
                {
                    "@id": "cefact:FLAP_Document.Identification.Identifier",
                    "@type": "unece:BasicBIE",
                    "unece:TDED": "1004",
                    "unece:cefactUNId": "UN01010846",
                    "unece:cefactBieDomainClass": "cefact:FLAP_Document.Details",
                    "rdfs:comment": "The identifier for this FLAP document."
                },
                {
                    "@id": "cefact:VesselPosition_Query.Identification.Identifier",
                    "@type": "unece:BasicBIE",
                    "unece:cefactUNId": "UN01012647",
                    "unece:cefactBieDomainClass": "cefact:VesselPosition_Query.Details",
                    "rdfs:comment": "The identifier for this vessel position query."
                },
                {
                    "@id": "cefact:MDR_Query.Identification.Identifier",
                    "@type": "unece:BasicBIE",
                    "unece:cefactUNId": "UN01010571",
                    "unece:cefactBieDomainClass": "cefact:MDR_Query.Details",
                    "rdfs:comment": "The identifier for this MDR query."
                },
                {
                    "@id": "cefact:Sales_Report.Identification.Identifier",
                    "@type": "unece:BasicBIE",
                    "unece:cefactUNId": "UN01010905",
                    "unece:cefactBieDomainClass": "cefact:Sales_Report.Details",
                    "rdfs:comment": "The identifier for this sales report."
                },
                {
                    "@id": "cefact:Vessel_Country.Identification.Identifier",
                    "@type": "unece:BasicBIE",
                    "unece:TDED": "3207",
                    "unece:cefactUNId": "UN01010232",
                    "unece:cefactBieDomainClass": "cefact:Vessel_Country.Details",
                    "rdfs:comment": "The identifier for this vessel country."
                },
                {
                    "@id": "cefact:Vehicle_TransportMeans.Identification.Identifier",
                    "@type": "unece:BasicBIE",
                    "unece:TDED": "8213",
                    "unece:cefactUNId": "UN01010988",
                    "unece:cefactBieDomainClass": "cefact:Vehicle_TransportMeans.Details",
                    "rdfs:comment": "The identifier of this vehicle transport means."
                }
            ]
        },
        {
            "@id": "fisheries:illustratePicture",
            "@type": "rdf:Property",
            "schema:rangeIncludes": {
                "@id": "fisheries:Picture"
            },
            "schema:domainIncludes": [
                {
                    "@id": "fisheries:Engine"
                },
                {
                    "@id": "fisheries:Gear"
                },
                {
                    "@id": "fisheries:TransportMeans"
                }
            ],
            "rdfs:comment": [
                "A Fisheries Language for Universal eXchange (FLUX) picture illustrating this fishing gear.",
                "A Fisheries Language for Universal eXchange (FLUX) picture illustrating this transport means vessel.",
                "A Fisheries Language for Universal eXchange (FLUX) picture illustrating this vessel engine."
            ],
            "rdfs:label": "illustratePicture",
            "unece:cefactElementMetadata": [
                {
                    "@id": "cefact:Vessel_TransportMeans.Illustrate.FLUX_Picture",
                    "@type": "unece:AssociationBIE",
                    "unece:cefactUNId": "UN01010648",
                    "unece:cefactBieDomainClass": "cefact:Vessel_TransportMeans.Details",
                    "rdfs:comment": "A Fisheries Language for Universal eXchange (FLUX) picture illustrating this transport means vessel."
                },
                {
                    "@id": "cefact:Fishing_Gear.Illustrate.FLUX_Picture",
                    "@type": "unece:AssociationBIE",
                    "unece:cefactUNId": "UN01010779",
                    "unece:cefactBieDomainClass": "cefact:Fishing_Gear.Details",
                    "rdfs:comment": "A Fisheries Language for Universal eXchange (FLUX) picture illustrating this fishing gear."
                },
                {
                    "@id": "cefact:Vessel_Engine.Illustrate.FLUX_Picture",
                    "@type": "unece:AssociationBIE",
                    "unece:cefactUNId": "UN01010778",
                    "unece:cefactBieDomainClass": "cefact:Vessel_Engine.Details",
                    "rdfs:comment": "A Fisheries Language for Universal eXchange (FLUX) picture illustrating this vessel engine."
                }
            ]
        },
        {
            "@id": "fisheries:includedBinaryObject",
            "@type": "rdf:Property",
            "schema:rangeIncludes": {
                "@id": "xsd:base64Binary"
            },
            "schema:domainIncludes": {
                "@id": "fisheries:BinaryFile"
            },
            "rdfs:comment": "The included binary object for this FLUX binary file.",
            "rdfs:label": "includedBinaryObject",
            "unece:cefactElementMetadata": [
                {
                    "@id": "cefact:FLUX_BinaryFile.Included.BinaryObject",
                    "@type": "unece:BasicBIE",
                    "unece:cefactUNId": "UN01010801",
                    "unece:cefactBieDomainClass": "cefact:FLUX_BinaryFile.Details",
                    "rdfs:comment": "The included binary object for this FLUX binary file."
                }
            ]
        },
        {
            "@id": "fisheries:includedDocument",
            "@type": "rdf:Property",
            "schema:rangeIncludes": {
                "@id": "fisheries:Document"
            },
            "schema:domainIncludes": {
                "@id": "fisheries:Report"
            },
            "rdfs:comment": [
                "A result document of a validation process for this sales report.",
                "A sales document included in this report.",
                "The Fisheries Language Universal eXchange (FLUX) report document included in this IS report."
            ],
            "rdfs:label": "includedDocument",
            "unece:cefactElementMetadata": [
                {
                    "@id": "cefact:Sales_Report.Included.Sales_Document",
                    "@type": "unece:AssociationBIE",
                    "unece:cefactUNId": "UN01010907",
                    "unece:cefactBieDomainClass": "cefact:Sales_Report.Details",
                    "rdfs:comment": "A sales document included in this report."
                },
                {
                    "@id": "cefact:Sales_Report.Included.ValidationResult_Document",
                    "@type": "unece:AssociationBIE",
                    "unece:cefactUNId": "UN01010908",
                    "unece:cefactBieDomainClass": "cefact:Sales_Report.Details",
                    "rdfs:comment": "A result document of a validation process for this sales report."
                },
                {
                    "@id": "cefact:IS_Report.Included.FLUXReport_Document",
                    "@type": "unece:AssociationBIE",
                    "unece:cefactUNId": "UN01012591",
                    "unece:cefactBieDomainClass": "cefact:IS_Report.Details",
                    "rdfs:comment": "The Fisheries Language Universal eXchange (FLUX) report document included in this IS report."
                }
            ]
        },
        {
            "@id": "fisheries:itemTypeCode",
            "@type": "rdf:Property",
            "schema:rangeIncludes": {
                "@id": "xsd:token"
            },
            "schema:domainIncludes": {
                "@id": "fisheries:Report"
            },
            "rdfs:comment": "The code specifying the type of the item in this sales report.",
            "rdfs:label": "itemTypeCode",
            "unece:cefactElementMetadata": [
                {
                    "@id": "cefact:Sales_Report.Item_Type.Code",
                    "@type": "unece:BasicBIE",
                    "unece:cefactUNId": "UN01010906",
                    "unece:cefactBieDomainClass": "cefact:Sales_Report.Details",
                    "rdfs:comment": "The code specifying the type of the item in this sales report."
                }
            ]
        },
        {
            "@id": "fisheries:joinedVesselId",
            "@type": "rdf:Property",
            "schema:rangeIncludes": {
                "@id": "xsd:token"
            },
            "schema:domainIncludes": {
                "@id": "fisheries:Document"
            },
            "rdfs:comment": "An identifier for a joined vessel for this FLAP document.",
            "rdfs:label": "joinedVesselId",
            "unece:cefactElementMetadata": [
                {
                    "@id": "cefact:FLAP_Document.JoinedVessel_Identification.Identifier",
                    "@type": "unece:BasicBIE",
                    "unece:TDED": "8313",
                    "unece:cefactUNId": "UN01010848",
                    "unece:cefactBieDomainClass": "cefact:FLAP_Document.Details",
                    "rdfs:comment": "An identifier for a joined vessel for this FLAP document."
                }
            ]
        },
        {
            "@id": "fisheries:jurisdictionCountryId",
            "@type": "rdf:Property",
            "schema:rangeIncludes": {
                "@id": "xsd:token"
            },
            "schema:domainIncludes": {
                "@id": "fisheries:Location"
            },
            "rdfs:comment": "The identifier of the country having jurisdiction over this FLUX location.",
            "rdfs:label": "jurisdictionCountryId",
            "unece:cefactElementMetadata": [
                {
                    "@id": "cefact:FLUX_Location.Jurisdiction_Country.Identifier",
                    "@type": "unece:BasicBIE",
                    "unece:cefactUNId": "UN01011202",
                    "unece:cefactBieDomainClass": "cefact:FLUX_Location.Details",
                    "rdfs:comment": "The identifier of the country having jurisdiction over this FLUX location."
                }
            ]
        },
        {
            "@id": "fisheries:landingCountryCode",
            "@type": "rdf:Property",
            "schema:rangeIncludes": {
                "@id": "xsd:token"
            },
            "schema:domainIncludes": {
                "@id": "fisheries:ReportedArea"
            },
            "rdfs:comment": "The code specifying a landing country for this ACDR reported area.",
            "rdfs:label": "landingCountryCode",
            "unece:cefactElementMetadata": [
                {
                    "@id": "cefact:ACDR_ReportedArea.LandingCountry.Code",
                    "@type": "unece:BasicBIE",
                    "unece:cefactUNId": "UN01010261",
                    "unece:cefactBieDomainClass": "cefact:ACDR_ReportedArea.Details",
                    "rdfs:comment": "The code specifying a landing country for this ACDR reported area."
                }
            ]
        },
        {
            "@id": "fisheries:latitudeMeasure",
            "@type": "rdf:Property",
            "schema:rangeIncludes": {
                "@id": "xsd:decimal"
            },
            "schema:domainIncludes": {
                "@id": "fisheries:GeographicalCoordinate"
            },
            "rdfs:comment": [
                "The measure of the latitude as an angular distance north or south from the Equator meridian to the meridian of a specific place for this vessel geographical coordinate.",
                "The measure of the latitude of this FLUX geographical coordinate."
            ],
            "rdfs:label": "latitudeMeasure",
            "unece:cefactElementMetadata": [
                {
                    "@id": "cefact:FLUX_GeographicalCoordinate.Latitude.Measure",
                    "@type": "unece:BasicBIE",
                    "unece:TDED": "6000",
                    "unece:cefactUNId": "UN01010968",
                    "unece:cefactBieDomainClass": "cefact:FLUX_GeographicalCoordinate.Details",
                    "rdfs:comment": "The measure of the latitude of this FLUX geographical coordinate."
                },
                {
                    "@id": "cefact:Vessel_GeographicalCoordinate.Latitude.Measure",
                    "@type": "unece:BasicBIE",
                    "unece:TDED": "6000",
                    "unece:cefactUNId": "UN01010223",
                    "unece:cefactBieDomainClass": "cefact:Vessel_GeographicalCoordinate.Details",
                    "rdfs:comment": "The measure of the latitude as an angular distance north or south from the Equator meridian to the meridian of a specific place for this vessel geographical coordinate."
                }
            ]
        },
        {
            "@id": "fisheries:legalReference",
            "@type": "rdf:Property",
            "schema:rangeIncludes": {
                "@id": "xsd:string"
            },
            "schema:domainIncludes": {
                "@id": "fisheries:Suspicion"
            },
            "rdfs:comment": "The legal reference, expressed as text, for this ISR infringement suspicion.",
            "rdfs:label": "legalReference",
            "unece:cefactElementMetadata": [
                {
                    "@id": "cefact:ISRInfringement_Suspicion.Legal_Reference.Text",
                    "@type": "unece:BasicBIE",
                    "unece:cefactUNId": "UN01013325",
                    "unece:cefactBieDomainClass": "cefact:ISRInfringement_Suspicion.Details",
                    "rdfs:comment": "The legal reference, expressed as text, for this ISR infringement suspicion."
                }
            ]
        },
        {
            "@id": "fisheries:levelCode",
            "@type": "rdf:Property",
            "schema:rangeIncludes": {
                "@id": "xsd:token"
            },
            "schema:domainIncludes": {
                "@id": "fisheries:QualityAnalysis"
            },
            "rdfs:comment": "The code specifying the level of this quality analysis of a validation process.",
            "rdfs:label": "levelCode",
            "unece:cefactElementMetadata": [
                {
                    "@id": "cefact:Validation_QualityAnalysis.Level.Code",
                    "@type": "unece:BasicBIE",
                    "unece:cefactUNId": "UN01010755",
                    "unece:cefactBieDomainClass": "cefact:Validation_QualityAnalysis.Details",
                    "rdfs:comment": "The code specifying the level of this quality analysis of a validation process."
                }
            ]
        },
        {
            "@id": "fisheries:longitudeMeasure",
            "@type": "rdf:Property",
            "schema:rangeIncludes": {
                "@id": "xsd:decimal"
            },
            "schema:domainIncludes": {
                "@id": "fisheries:GeographicalCoordinate"
            },
            "rdfs:comment": [
                "The measure of the longitude as an angular distance east or west from the Greenwich meridian to the meridian of a specific place for this vessel geographical coordinate.",
                "The measure of the longitude of this FLUX geographical coordinate."
            ],
            "rdfs:label": "longitudeMeasure",
            "unece:cefactElementMetadata": [
                {
                    "@id": "cefact:FLUX_GeographicalCoordinate.Longitude.Measure",
                    "@type": "unece:BasicBIE",
                    "unece:TDED": "6002",
                    "unece:cefactUNId": "UN01010967",
                    "unece:cefactBieDomainClass": "cefact:FLUX_GeographicalCoordinate.Details",
                    "rdfs:comment": "The measure of the longitude of this FLUX geographical coordinate."
                },
                {
                    "@id": "cefact:Vessel_GeographicalCoordinate.Longitude.Measure",
                    "@type": "unece:BasicBIE",
                    "unece:TDED": "6002",
                    "unece:cefactUNId": "UN01010224",
                    "unece:cefactBieDomainClass": "cefact:Vessel_GeographicalCoordinate.Details",
                    "rdfs:comment": "The measure of the longitude as an angular distance east or west from the Greenwich meridian to the meridian of a specific place for this vessel geographical coordinate."
                }
            ]
        },
        {
            "@id": "fisheries:manufacturer",
            "@type": "rdf:Property",
            "schema:rangeIncludes": {
                "@id": "xsd:string"
            },
            "schema:domainIncludes": {
                "@id": "fisheries:Engine"
            },
            "rdfs:comment": "The manufacturer, expressed as text, of this vessel engine.",
            "rdfs:label": "manufacturer",
            "unece:cefactElementMetadata": [
                {
                    "@id": "cefact:Vessel_Engine.Manufacturer.Text",
                    "@type": "unece:BasicBIE",
                    "unece:cefactUNId": "UN01010777",
                    "unece:cefactBieDomainClass": "cefact:Vessel_Engine.Details",
                    "rdfs:comment": "The manufacturer, expressed as text, of this vessel engine."
                }
            ]
        },
        {
            "@id": "fisheries:manufacturerCode",
            "@type": "rdf:Property",
            "schema:rangeIncludes": {
                "@id": "xsd:token"
            },
            "schema:domainIncludes": {
                "@id": "fisheries:Engine"
            },
            "rdfs:comment": "The code specifying the manufacturer of this vessel engine.",
            "rdfs:label": "manufacturerCode",
            "unece:cefactElementMetadata": [
                {
                    "@id": "cefact:Vessel_Engine.Manufacturer.Code",
                    "@type": "unece:BasicBIE",
                    "unece:cefactUNId": "UN01010724",
                    "unece:cefactBieDomainClass": "cefact:Vessel_Engine.Details",
                    "rdfs:comment": "The code specifying the manufacturer of this vessel engine."
                }
            ]
        },
        {
            "@id": "fisheries:maximumSizeQuantity",
            "@type": "rdf:Property",
            "schema:rangeIncludes": {
                "@id": "xsd:decimal"
            },
            "schema:domainIncludes": {
                "@id": "fisheries:Crew"
            },
            "rdfs:comment": "The maximum size, expressed as a quantity, of this vessel crew.",
            "rdfs:label": "maximumSizeQuantity",
            "unece:cefactElementMetadata": [
                {
                    "@id": "cefact:Vessel_Crew.Maximum_Size.Quantity",
                    "@type": "unece:BasicBIE",
                    "unece:cefactUNId": "UN01010816",
                    "unece:cefactBieDomainClass": "cefact:Vessel_Crew.Details",
                    "rdfs:comment": "The maximum size, expressed as a quantity, of this vessel crew."
                }
            ]
        },
        {
            "@id": "fisheries:memberQuantity",
            "@type": "rdf:Property",
            "schema:rangeIncludes": {
                "@id": "xsd:decimal"
            },
            "schema:domainIncludes": {
                "@id": "fisheries:Crew"
            },
            "rdfs:comment": "The number of members in this vessel crew.",
            "rdfs:label": "memberQuantity",
            "unece:cefactElementMetadata": [
                {
                    "@id": "cefact:Vessel_Crew.Member.Quantity",
                    "@type": "unece:BasicBIE",
                    "unece:cefactUNId": "UN01010814",
                    "unece:cefactBieDomainClass": "cefact:Vessel_Crew.Details",
                    "rdfs:comment": "The number of members in this vessel crew."
                }
            ]
        },
        {
            "@id": "fisheries:methodTypeCode",
            "@type": "rdf:Property",
            "schema:rangeIncludes": {
                "@id": "xsd:token"
            },
            "schema:domainIncludes": {
                "@id": "fisheries:Characteristic"
            },
            "rdfs:comment": "The code specifying a method type of this vessel storage characteristic.",
            "rdfs:label": "methodTypeCode",
            "unece:cefactElementMetadata": [
                {
                    "@id": "cefact:VesselStorage_Characteristic.Method_Type.Code",
                    "@type": "unece:BasicBIE",
                    "unece:cefactUNId": "UN01010808",
                    "unece:cefactBieDomainClass": "cefact:VesselStorage_Characteristic.Details",
                    "rdfs:comment": "The code specifying a method type of this vessel storage characteristic."
                }
            ]
        },
        {
            "@id": "fisheries:minimumSizeQuantity",
            "@type": "rdf:Property",
            "schema:rangeIncludes": {
                "@id": "xsd:decimal"
            },
            "schema:domainIncludes": {
                "@id": "fisheries:Crew"
            },
            "rdfs:comment": "The minimum size, expressed as a quantity, of this vessel crew.",
            "rdfs:label": "minimumSizeQuantity",
            "unece:cefactElementMetadata": [
                {
                    "@id": "cefact:Vessel_Crew.Minimum_Size.Quantity",
                    "@type": "unece:BasicBIE",
                    "unece:cefactUNId": "UN01010815",
                    "unece:cefactBieDomainClass": "cefact:Vessel_Crew.Details",
                    "rdfs:comment": "The minimum size, expressed as a quantity, of this vessel crew."
                }
            ]
        },
        {
            "@id": "fisheries:model",
            "@type": "rdf:Property",
            "schema:rangeIncludes": {
                "@id": "xsd:string"
            },
            "schema:domainIncludes": {
                "@id": "fisheries:Engine"
            },
            "rdfs:comment": "The model, expressed as a text, of this vessel engine.",
            "rdfs:label": "model",
            "unece:cefactElementMetadata": [
                {
                    "@id": "cefact:Vessel_Engine.Model.Text",
                    "@type": "unece:BasicBIE",
                    "unece:cefactUNId": "UN01010725",
                    "unece:cefactBieDomainClass": "cefact:Vessel_Engine.Details",
                    "rdfs:comment": "The model, expressed as a text, of this vessel engine."
                }
            ]
        },
        {
            "@id": "fisheries:name",
            "@type": "rdf:Property",
            "schema:rangeIncludes": {
                "@id": "xsd:string"
            },
            "schema:domainIncludes": [
                {
                    "@id": "fisheries:BinaryFile"
                },
                {
                    "@id": "fisheries:DataNode"
                },
                {
                    "@id": "fisheries:DataSet"
                },
                {
                    "@id": "fisheries:Document"
                },
                {
                    "@id": "fisheries:Location"
                },
                {
                    "@id": "fisheries:Organization"
                },
                {
                    "@id": "fisheries:Party"
                },
                {
                    "@id": "fisheries:TransportMeans"
                },
                {
                    "@id": "fisheries:Version"
                }
            ],
            "rdfs:comment": [
                "A name, expressed as text, of this FLUX location.",
                "A name, expressed as text, of this party.",
                "A name, expressed as text, of this transport means vessel.",
                "The name, expressed as text, of this FLAP document.",
                "The name, expressed as text, of this FLUX binary file.",
                "The name, expressed as text, of this FLUX organization.",
                "The name, expressed as text, of this MDR data set.",
                "The name, expressed as text, of this MDR element data node.",
                "The name, expressed as text, of this data set version.",
                "The name, expressed as text, of this sales party.",
                "The name, expressed as text, of this vehicle transport means."
            ],
            "rdfs:label": "name",
            "unece:cefactElementMetadata": [
                {
                    "@id": "cefact:FLUX_BinaryFile.Name.Text",
                    "@type": "unece:BasicBIE",
                    "unece:TDED": "1508",
                    "unece:cefactUNId": "UN01010805",
                    "unece:cefactBieDomainClass": "cefact:FLUX_BinaryFile.Details",
                    "rdfs:comment": "The name, expressed as text, of this FLUX binary file."
                },
                {
                    "@id": "cefact:Vehicle_TransportMeans.Name.Text",
                    "@type": "unece:BasicBIE",
                    "unece:TDED": "8212",
                    "unece:cefactUNId": "UN01010990",
                    "unece:cefactBieDomainClass": "cefact:Vehicle_TransportMeans.Details",
                    "rdfs:comment": "The name, expressed as text, of this vehicle transport means."
                },
                {
                    "@id": "cefact:Vessel_TransportMeans.Name.Text",
                    "@type": "unece:BasicBIE",
                    "unece:TDED": "8212",
                    "unece:cefactUNId": "UN01010635",
                    "unece:cefactBieDomainClass": "cefact:Vessel_TransportMeans.Details",
                    "rdfs:comment": "A name, expressed as text, of this transport means vessel."
                },
                {
                    "@id": "cefact:FLAP_Document.Name.Text",
                    "@type": "unece:BasicBIE",
                    "unece:TDED": "1000",
                    "unece:cefactUNId": "UN01010849",
                    "unece:cefactBieDomainClass": "cefact:FLAP_Document.Details",
                    "rdfs:comment": "The name, expressed as text, of this FLAP document."
                },
                {
                    "@id": "cefact:MDRElement_DataNode.Name.Text",
                    "@type": "unece:BasicBIE",
                    "unece:cefactUNId": "UN01010596",
                    "unece:cefactBieDomainClass": "cefact:MDRElement_DataNode.Details",
                    "rdfs:comment": "The name, expressed as text, of this MDR element data node."
                },
                {
                    "@id": "cefact:Sales_Party.Name.Text",
                    "@type": "unece:BasicBIE",
                    "unece:TDED": "3036",
                    "unece:cefactUNId": "UN01010924",
                    "unece:cefactBieDomainClass": "cefact:Sales_Party.Details",
                    "rdfs:comment": "The name, expressed as text, of this sales party."
                },
                {
                    "@id": "cefact:DataSet_Version.Name.Text",
                    "@type": "unece:BasicBIE",
                    "unece:cefactUNId": "UN01010600",
                    "unece:cefactBieDomainClass": "cefact:DataSet_Version.Details",
                    "rdfs:comment": "The name, expressed as text, of this data set version."
                },
                {
                    "@id": "cefact:MDR_DataSet.Name.Text",
                    "@type": "unece:BasicBIE",
                    "unece:cefactUNId": "UN01010586",
                    "unece:cefactBieDomainClass": "cefact:MDR_DataSet.Details",
                    "rdfs:comment": "The name, expressed as text, of this MDR data set."
                },
                {
                    "@id": "cefact:FLUX_Location.Name.Text",
                    "@type": "unece:BasicBIE",
                    "unece:TDED": "3224",
                    "unece:cefactUNId": "UN01010885",
                    "unece:cefactBieDomainClass": "cefact:FLUX_Location.Details",
                    "rdfs:comment": "A name, expressed as text, of this FLUX location."
                },
                {
                    "@id": "cefact:FLUX_Party.Name.Text",
                    "@type": "unece:BasicBIE",
                    "unece:TDED": "3036",
                    "unece:cefactUNId": "UN01010247",
                    "unece:cefactBieDomainClass": "cefact:FLUX_Party.Details",
                    "rdfs:comment": "A name, expressed as text, of this party."
                },
                {
                    "@id": "cefact:FLUX_Organization.Name.Text",
                    "@type": "unece:BasicBIE",
                    "unece:cefactUNId": "UN01010985",
                    "unece:cefactBieDomainClass": "cefact:FLUX_Organization.Details",
                    "rdfs:comment": "The name, expressed as text, of this FLUX organization."
                }
            ]
        },
        {
            "@id": "fisheries:objectCode",
            "@type": "rdf:Property",
            "schema:rangeIncludes": {
                "@id": "xsd:token"
            },
            "schema:domainIncludes": {
                "@id": "fisheries:Quota"
            },
            "rdfs:comment": "The code specifying an object to which this targeted quota is applied.",
            "rdfs:label": "objectCode",
            "unece:cefactElementMetadata": [
                {
                    "@id": "cefact:Targeted_Quota.Object.Code",
                    "@type": "unece:BasicBIE",
                    "unece:cefactUNId": "UN01010880",
                    "unece:cefactBieDomainClass": "cefact:Targeted_Quota.Details",
                    "rdfs:comment": "The code specifying an object to which this targeted quota is applied."
                }
            ]
        },
        {
            "@id": "fisheries:observation",
            "@type": "rdf:Property",
            "schema:rangeIncludes": {
                "@id": "xsd:string"
            },
            "schema:domainIncludes": {
                "@id": "fisheries:Suspicion"
            },
            "rdfs:comment": "The observation, expressed as text, about this ISR infringement suspicion.",
            "rdfs:label": "observation",
            "unece:cefactElementMetadata": [
                {
                    "@id": "cefact:ISRInfringement_Suspicion.Observation.Text",
                    "@type": "unece:BasicBIE",
                    "unece:cefactUNId": "UN01013326",
                    "unece:cefactBieDomainClass": "cefact:ISRInfringement_Suspicion.Details",
                    "rdfs:comment": "The observation, expressed as text, about this ISR infringement suspicion."
                }
            ]
        },
        {
            "@id": "fisheries:obtainedOccurrenceDateTime",
            "@type": "rdf:Property",
            "schema:rangeIncludes": {
                "@id": "xsd:dateTime"
            },
            "schema:domainIncludes": {
                "@id": "fisheries:Event"
            },
            "rdfs:comment": "The date and time when the position of the vessel was taken by the vessel's navigation equipment.",
            "rdfs:label": "obtainedOccurrenceDateTime",
            "unece:cefactElementMetadata": [
                {
                    "@id": "cefact:VesselPosition_Event.Obtained_Occurrence.DateTime",
                    "@type": "unece:BasicBIE",
                    "unece:TDED": "2193",
                    "unece:cefactUNId": "UN01010234",
                    "unece:cefactBieDomainClass": "cefact:VesselPosition_Event.Details",
                    "rdfs:comment": "The date and time when the position of the vessel was taken by the vessel's navigation equipment."
                }
            ]
        },
        {
            "@id": "fisheries:occurrenceDateTime",
            "@type": "rdf:Property",
            "schema:rangeIncludes": {
                "@id": "xsd:dateTime"
            },
            "schema:domainIncludes": [
                {
                    "@id": "fisheries:Activity"
                },
                {
                    "@id": "fisheries:Event"
                }
            ],
            "rdfs:comment": [
                "The date, time, date time, or other date time value of an occurrence of this sales event.",
                "The date, time, date time, or other date time value of an occurrence of this vessel event.",
                "The date, time, date time, or other date time value of the occurrence of this IS event.",
                "The date, time, date time, or other date time value of the occurrence of this gear inspection event.",
                "The date, time, date time, or other date time value, of the occurrence of this fishing activity.",
                "The occurrence date, time, date time or other date time value for this gear equipment inspection event."
            ],
            "rdfs:label": "occurrenceDateTime",
            "unece:cefactElementMetadata": [
                {
                    "@id": "cefact:IS_Event.Occurrence.DateTime",
                    "@type": "unece:BasicBIE",
                    "unece:cefactUNId": "UN01012616",
                    "unece:cefactBieDomainClass": "cefact:IS_Event.Details",
                    "rdfs:comment": "The date, time, date time, or other date time value of the occurrence of this IS event."
                },
                {
                    "@id": "cefact:Fishing_Activity.Occurrence.DateTime",
                    "@type": "unece:BasicBIE",
                    "unece:cefactUNId": "UN01011171",
                    "unece:cefactBieDomainClass": "cefact:Fishing_Activity.Details",
                    "rdfs:comment": "The date, time, date time, or other date time value, of the occurrence of this fishing activity."
                },
                {
                    "@id": "cefact:GearInspection_Event.Occurrence.DateTime",
                    "@type": "unece:BasicBIE",
                    "unece:cefactUNId": "UN01012626",
                    "unece:cefactBieDomainClass": "cefact:GearInspection_Event.Details",
                    "rdfs:comment": "The date, time, date time, or other date time value of the occurrence of this gear inspection event."
                },
                {
                    "@id": "cefact:Vessel_Event.Occurrence.DateTime",
                    "@type": "unece:BasicBIE",
                    "unece:TDED": "2193",
                    "unece:cefactUNId": "UN01010662",
                    "unece:cefactBieDomainClass": "cefact:Vessel_Event.Details",
                    "rdfs:comment": "The date, time, date time, or other date time value of an occurrence of this vessel event."
                },
                {
                    "@id": "cefact:GearEquipmentInspection_Event.Occurrence.DateTime",
                    "@type": "unece:BasicBIE",
                    "unece:TDED": "2193",
                    "unece:cefactUNId": "UN01013331",
                    "unece:cefactBieDomainClass": "cefact:GearEquipmentInspection_Event.Details",
                    "rdfs:comment": "The occurrence date, time, date time or other date time value for this gear equipment inspection event."
                },
                {
                    "@id": "cefact:Sales_Event.Occurrence.DateTime",
                    "@type": "unece:BasicBIE",
                    "unece:TDED": "2193",
                    "unece:cefactUNId": "UN01010948",
                    "unece:cefactBieDomainClass": "cefact:Sales_Event.Details",
                    "rdfs:comment": "The date, time, date time, or other date time value of an occurrence of this sales event."
                }
            ]
        },
        {
            "@id": "fisheries:occurrencePeriod",
            "@type": "rdf:Property",
            "schema:rangeIncludes": {
                "@id": "fisheries:Period"
            },
            "schema:domainIncludes": {
                "@id": "fisheries:Event"
            },
            "rdfs:comment": [
                "The delimited period of time during which this IS event occurs.",
                "The delimited period of time during which this gear inspection event occurs."
            ],
            "rdfs:label": "occurrencePeriod",
            "unece:cefactElementMetadata": [
                {
                    "@id": "cefact:GearInspection_Event.Occurrence.Delimited_Period",
                    "@type": "unece:AssociationBIE",
                    "unece:cefactUNId": "UN01012627",
                    "unece:cefactBieDomainClass": "cefact:GearInspection_Event.Details",
                    "rdfs:comment": "The delimited period of time during which this gear inspection event occurs."
                },
                {
                    "@id": "cefact:IS_Event.Occurrence.Delimited_Period",
                    "@type": "unece:AssociationBIE",
                    "unece:cefactUNId": "UN01012618",
                    "unece:cefactBieDomainClass": "cefact:IS_Event.Details",
                    "rdfs:comment": "The delimited period of time during which this IS event occurs."
                }
            ]
        },
        {
            "@id": "fisheries:onBoardGear",
            "@type": "rdf:Property",
            "schema:rangeIncludes": {
                "@id": "fisheries:Gear"
            },
            "schema:domainIncludes": {
                "@id": "fisheries:TransportMeans"
            },
            "rdfs:comment": "Fishing gear which is on board this transport means vessel.",
            "rdfs:label": "onBoardGear",
            "unece:cefactElementMetadata": [
                {
                    "@id": "cefact:Vessel_TransportMeans.OnBoard.Fishing_Gear",
                    "@type": "unece:AssociationBIE",
                    "unece:cefactUNId": "UN01010645",
                    "unece:cefactBieDomainClass": "cefact:Vessel_TransportMeans.Details",
                    "rdfs:comment": "Fishing gear which is on board this transport means vessel."
                }
            ]
        },
        {
            "@id": "fisheries:onDeckSizeQuantity",
            "@type": "rdf:Property",
            "schema:rangeIncludes": {
                "@id": "xsd:decimal"
            },
            "schema:domainIncludes": {
                "@id": "fisheries:Crew"
            },
            "rdfs:comment": "The size, expressed as a quantity, of this vessel crew working on the deck.",
            "rdfs:label": "onDeckSizeQuantity",
            "unece:cefactElementMetadata": [
                {
                    "@id": "cefact:Vessel_Crew.OnDeck_Size.Quantity",
                    "@type": "unece:BasicBIE",
                    "unece:cefactUNId": "UN01010817",
                    "unece:cefactBieDomainClass": "cefact:Vessel_Crew.Details",
                    "rdfs:comment": "The size, expressed as a quantity, of this vessel crew working on the deck."
                }
            ]
        },
        {
            "@id": "fisheries:operationalStatusCode",
            "@type": "rdf:Property",
            "schema:rangeIncludes": {
                "@id": "xsd:token"
            },
            "schema:domainIncludes": {
                "@id": "fisheries:TransportMeans"
            },
            "rdfs:comment": "The code indicating the operational status for this vessel transport means, such as in service/commission, broken up, total loss, continued existence in doubt, laid-up.",
            "rdfs:label": "operationalStatusCode",
            "unece:cefactElementMetadata": [
                {
                    "@id": "cefact:Vessel_TransportMeans.OperationalStatus.Code",
                    "@type": "unece:BasicBIE",
                    "unece:cefactUNId": "UN01010638",
                    "unece:cefactBieDomainClass": "cefact:Vessel_TransportMeans.Details",
                    "rdfs:comment": "The code indicating the operational status for this vessel transport means, such as in service/commission, broken up, total loss, continued existence in doubt, laid-up."
                }
            ]
        },
        {
            "@id": "fisheries:operationsQuantity",
            "@type": "rdf:Property",
            "schema:rangeIncludes": {
                "@id": "xsd:decimal"
            },
            "schema:domainIncludes": {
                "@id": "fisheries:Activity"
            },
            "rdfs:comment": "The number of operations for this fishing activity.",
            "rdfs:label": "operationsQuantity",
            "unece:cefactElementMetadata": [
                {
                    "@id": "cefact:Fishing_Activity.Operations.Quantity",
                    "@type": "unece:BasicBIE",
                    "unece:cefactUNId": "UN01011176",
                    "unece:cefactBieDomainClass": "cefact:Fishing_Activity.Details",
                    "rdfs:comment": "The number of operations for this fishing activity."
                }
            ]
        },
        {
            "@id": "fisheries:origin",
            "@type": "rdf:Property",
            "schema:rangeIncludes": {
                "@id": "xsd:string"
            },
            "schema:domainIncludes": {
                "@id": "fisheries:DataSet"
            },
            "rdfs:comment": "The origin, expressed as text, of this MDR data set.",
            "rdfs:label": "origin",
            "unece:cefactElementMetadata": [
                {
                    "@id": "cefact:MDR_DataSet.Origin.Text",
                    "@type": "unece:BasicBIE",
                    "unece:cefactUNId": "UN01010585",
                    "unece:cefactBieDomainClass": "cefact:MDR_DataSet.Details",
                    "rdfs:comment": "The origin, expressed as text, of this MDR data set."
                }
            ]
        },
        {
            "@id": "fisheries:originActivity",
            "@type": "rdf:Property",
            "schema:rangeIncludes": {
                "@id": "fisheries:Activity"
            },
            "schema:domainIncludes": {
                "@id": "fisheries:Product"
            },
            "rdfs:comment": "The fishing activity from which this AAP product originates.",
            "rdfs:label": "originActivity",
            "unece:cefactElementMetadata": [
                {
                    "@id": "cefact:AAP_Product.Origin.Fishing_Activity",
                    "@type": "unece:AssociationBIE",
                    "unece:cefactUNId": "UN01011148",
                    "unece:cefactBieDomainClass": "cefact:AAP_Product.Details",
                    "rdfs:comment": "The fishing activity from which this AAP product originates."
                }
            ]
        },
        {
            "@id": "fisheries:originLocation",
            "@type": "rdf:Property",
            "schema:rangeIncludes": {
                "@id": "fisheries:Location"
            },
            "schema:domainIncludes": {
                "@id": "fisheries:Product"
            },
            "rdfs:comment": "A Fisheries Language for Universal eXchange (FLUX) location from which this AAP product originates.",
            "rdfs:label": "originLocation",
            "unece:cefactElementMetadata": [
                {
                    "@id": "cefact:AAP_Product.Origin.FLUX_Location",
                    "@type": "unece:AssociationBIE",
                    "unece:cefactUNId": "UN01011147",
                    "unece:cefactBieDomainClass": "cefact:AAP_Product.Details",
                    "rdfs:comment": "A Fisheries Language for Universal eXchange (FLUX) location from which this AAP product originates."
                }
            ]
        },
        {
            "@id": "fisheries:ownerParty",
            "@type": "rdf:Property",
            "schema:rangeIncludes": {
                "@id": "fisheries:Party"
            },
            "schema:domainIncludes": [
                {
                    "@id": "fisheries:Document"
                },
                {
                    "@id": "fisheries:TransportMeans"
                }
            ],
            "rdfs:comment": [
                "The Fisheries Language for Universal eXchange (FLUX) party that owns this aggregated catch report document.",
                "The party that owns this FLUX report document.",
                "The sales party owning this vehicle transport means."
            ],
            "rdfs:label": "ownerParty",
            "unece:cefactElementMetadata": [
                {
                    "@id": "cefact:AggregatedCatchReport_Document.Owner.FLUX_Party",
                    "@type": "unece:AssociationBIE",
                    "unece:cefactUNId": "UN01010257",
                    "unece:cefactBieDomainClass": "cefact:AggregatedCatchReport_Document.Details",
                    "rdfs:comment": "The Fisheries Language for Universal eXchange (FLUX) party that owns this aggregated catch report document."
                },
                {
                    "@id": "cefact:FLUXReport_Document.Owner.FLUX_Party",
                    "@type": "unece:AssociationBIE",
                    "unece:cefactUNId": "UN01010244",
                    "unece:cefactBieDomainClass": "cefact:FLUXReport_Document.Details",
                    "rdfs:comment": "The party that owns this FLUX report document."
                },
                {
                    "@id": "cefact:Vehicle_TransportMeans.Owner.Sales_Party",
                    "@type": "unece:AssociationBIE",
                    "unece:cefactUNId": "UN01010992",
                    "unece:cefactBieDomainClass": "cefact:Vehicle_TransportMeans.Details",
                    "rdfs:comment": "The sales party owning this vehicle transport means."
                }
            ]
        },
        {
            "@id": "fisheries:packagingTypeCode",
            "@type": "rdf:Property",
            "schema:rangeIncludes": {
                "@id": "xsd:token"
            },
            "schema:domainIncludes": {
                "@id": "fisheries:Product"
            },
            "rdfs:comment": "The code specifying the type of packaging for this AAP product.",
            "rdfs:label": "packagingTypeCode",
            "unece:cefactElementMetadata": [
                {
                    "@id": "cefact:AAP_Product.Packaging_Type.Code",
                    "@type": "unece:BasicBIE",
                    "unece:cefactUNId": "UN01011143",
                    "unece:cefactBieDomainClass": "cefact:AAP_Product.Details",
                    "rdfs:comment": "The code specifying the type of packaging for this AAP product."
                }
            ]
        },
        {
            "@id": "fisheries:packagingUnitAverageWeightMeasure",
            "@type": "rdf:Property",
            "schema:rangeIncludes": {
                "@id": "xsd:decimal"
            },
            "schema:domainIncludes": {
                "@id": "fisheries:Product"
            },
            "rdfs:comment": "The measure of the average weight of a packaging unit for this AAP product.",
            "rdfs:label": "packagingUnitAverageWeightMeasure",
            "unece:cefactElementMetadata": [
                {
                    "@id": "cefact:AAP_Product.PackagingUnitAverage_Weight.Measure",
                    "@type": "unece:BasicBIE",
                    "unece:cefactUNId": "UN01011144",
                    "unece:cefactBieDomainClass": "cefact:AAP_Product.Details",
                    "rdfs:comment": "The measure of the average weight of a packaging unit for this AAP product."
                }
            ]
        },
        {
            "@id": "fisheries:packagingUnitQuantity",
            "@type": "rdf:Property",
            "schema:rangeIncludes": {
                "@id": "xsd:decimal"
            },
            "schema:domainIncludes": {
                "@id": "fisheries:Product"
            },
            "rdfs:comment": "The quantity of packaging units for this AAP product.",
            "rdfs:label": "packagingUnitQuantity",
            "unece:cefactElementMetadata": [
                {
                    "@id": "cefact:AAP_Product.Packaging_Unit.Quantity",
                    "@type": "unece:BasicBIE",
                    "unece:cefactUNId": "UN01011145",
                    "unece:cefactBieDomainClass": "cefact:AAP_Product.Details",
                    "rdfs:comment": "The quantity of packaging units for this AAP product."
                }
            ]
        },
        {
            "@id": "fisheries:parentId",
            "@type": "rdf:Property",
            "schema:rangeIncludes": {
                "@id": "xsd:token"
            },
            "schema:domainIncludes": {
                "@id": "fisheries:DataNode"
            },
            "rdfs:comment": "The identifier of the parent for this MDR data node.",
            "rdfs:label": "parentId",
            "unece:cefactElementMetadata": [
                {
                    "@id": "cefact:MDR_DataNode.Parent_Identification.Identifier",
                    "@type": "unece:BasicBIE",
                    "unece:cefactUNId": "UN01010591",
                    "unece:cefactBieDomainClass": "cefact:MDR_DataNode.Details",
                    "rdfs:comment": "The identifier of the parent for this MDR data node."
                }
            ]
        },
        {
            "@id": "fisheries:physicalAddress",
            "@type": "rdf:Property",
            "schema:rangeIncludes": {
                "@id": "fisheries:Address"
            },
            "schema:domainIncludes": {
                "@id": "fisheries:Location"
            },
            "rdfs:comment": [
                "The physical structured address of this registration location.",
                "The structured physical address information for this FLUX location."
            ],
            "rdfs:label": "physicalAddress",
            "unece:cefactElementMetadata": [
                {
                    "@id": "cefact:FLUX_Location.Physical.Structured_Address",
                    "@type": "unece:AssociationBIE",
                    "unece:cefactUNId": "UN01011204",
                    "unece:cefactBieDomainClass": "cefact:FLUX_Location.Details",
                    "rdfs:comment": "The structured physical address information for this FLUX location."
                },
                {
                    "@id": "cefact:Registration_Location.Physical.Structured_Address",
                    "@type": "unece:AssociationBIE",
                    "unece:cefactUNId": "UN01010774",
                    "unece:cefactBieDomainClass": "cefact:Registration_Location.Details",
                    "rdfs:comment": "The physical structured address of this registration location."
                }
            ]
        },
        {
            "@id": "fisheries:postalAddress",
            "@type": "rdf:Property",
            "schema:rangeIncludes": {
                "@id": "fisheries:Address"
            },
            "schema:domainIncludes": [
                {
                    "@id": "fisheries:Location"
                },
                {
                    "@id": "fisheries:Organization"
                }
            ],
            "rdfs:comment": [
                "Structured postal address information for this FLUX location.",
                "Structured postal address information for this FLUX organization."
            ],
            "rdfs:label": "postalAddress",
            "unece:cefactElementMetadata": [
                {
                    "@id": "cefact:FLUX_Location.Postal.Structured_Address",
                    "@type": "unece:AssociationBIE",
                    "unece:cefactUNId": "UN01010965",
                    "unece:cefactBieDomainClass": "cefact:FLUX_Location.Details",
                    "rdfs:comment": "Structured postal address information for this FLUX location."
                },
                {
                    "@id": "cefact:FLUX_Organization.Postal.Structured_Address",
                    "@type": "unece:AssociationBIE",
                    "unece:cefactUNId": "UN01010986",
                    "unece:cefactBieDomainClass": "cefact:FLUX_Organization.Details",
                    "rdfs:comment": "Structured postal address information for this FLUX organization."
                }
            ]
        },
        {
            "@id": "fisheries:powerMeasure",
            "@type": "rdf:Property",
            "schema:rangeIncludes": {
                "@id": "xsd:decimal"
            },
            "schema:domainIncludes": {
                "@id": "fisheries:Engine"
            },
            "rdfs:comment": "A measure of the power produced by this vessel engine, expressed in a unit such as horsepower.",
            "rdfs:label": "powerMeasure",
            "unece:cefactElementMetadata": [
                {
                    "@id": "cefact:Vessel_Engine.Power.Measure",
                    "@type": "unece:BasicBIE",
                    "unece:cefactUNId": "UN01010722",
                    "unece:cefactBieDomainClass": "cefact:Vessel_Engine.Details",
                    "rdfs:comment": "A measure of the power produced by this vessel engine, expressed in a unit such as horsepower."
                }
            ]
        },
        {
            "@id": "fisheries:powerMeasurementMethodCode",
            "@type": "rdf:Property",
            "schema:rangeIncludes": {
                "@id": "xsd:token"
            },
            "schema:domainIncludes": {
                "@id": "fisheries:Engine"
            },
            "rdfs:comment": "The code specifying the measurement method used for measuring the power of this vessel engine.",
            "rdfs:label": "powerMeasurementMethodCode",
            "unece:cefactElementMetadata": [
                {
                    "@id": "cefact:Vessel_Engine.PowerMeasurementMethod.Code",
                    "@type": "unece:BasicBIE",
                    "unece:cefactUNId": "UN01010723",
                    "unece:cefactBieDomainClass": "cefact:Vessel_Engine.Details",
                    "rdfs:comment": "The code specifying the measurement method used for measuring the power of this vessel engine."
                }
            ]
        },
        {
            "@id": "fisheries:propulsionTypeCode",
            "@type": "rdf:Property",
            "schema:rangeIncludes": {
                "@id": "xsd:token"
            },
            "schema:domainIncludes": {
                "@id": "fisheries:Engine"
            },
            "rdfs:comment": "The code specifying the type of propulsion for this vessel engine.",
            "rdfs:label": "propulsionTypeCode",
            "unece:cefactElementMetadata": [
                {
                    "@id": "cefact:Vessel_Engine.Propulsion_Type.Code",
                    "@type": "unece:BasicBIE",
                    "unece:cefactUNId": "UN01010721",
                    "unece:cefactBieDomainClass": "cefact:Vessel_Engine.Details",
                    "rdfs:comment": "The code specifying the type of propulsion for this vessel engine."
                }
            ]
        },
        {
            "@id": "fisheries:purpose",
            "@type": "rdf:Property",
            "schema:rangeIncludes": {
                "@id": "xsd:string"
            },
            "schema:domainIncludes": {
                "@id": "fisheries:Document"
            },
            "rdfs:comment": [
                "The purpose, expressed as text, for this FLAP request document.",
                "The purpose, expressed as text, of this FLUX report document."
            ],
            "rdfs:label": "purpose",
            "unece:cefactElementMetadata": [
                {
                    "@id": "cefact:FLUXReport_Document.Purpose.Text",
                    "@type": "unece:BasicBIE",
                    "unece:TDED": "1160",
                    "unece:cefactUNId": "UN01010243",
                    "unece:cefactBieDomainClass": "cefact:FLUXReport_Document.Details",
                    "rdfs:comment": "The purpose, expressed as text, of this FLUX report document."
                },
                {
                    "@id": "cefact:FLAPRequest_Document.Purpose.Text",
                    "@type": "unece:BasicBIE",
                    "unece:TDED": "1160",
                    "unece:cefactUNId": "UN01010834",
                    "unece:cefactBieDomainClass": "cefact:FLAPRequest_Document.Details",
                    "rdfs:comment": "The purpose, expressed as text, for this FLAP request document."
                }
            ]
        },
        {
            "@id": "fisheries:reasonCode",
            "@type": "rdf:Property",
            "schema:rangeIncludes": {
                "@id": "xsd:token"
            },
            "schema:domainIncludes": {
                "@id": "fisheries:Activity"
            },
            "rdfs:comment": "The code specifying a reason for this fishing activity, such as returning to port with the intention of unloading catches.",
            "rdfs:label": "reasonCode",
            "unece:cefactElementMetadata": [
                {
                    "@id": "cefact:Fishing_Activity.Reason.Code",
                    "@type": "unece:BasicBIE",
                    "unece:cefactUNId": "UN01011172",
                    "unece:cefactBieDomainClass": "cefact:Fishing_Activity.Details",
                    "rdfs:comment": "The code specifying a reason for this fishing activity, such as returning to port with the intention of unloading catches."
                }
            ]
        },
        {
            "@id": "fisheries:recoveryMeasureCode",
            "@type": "rdf:Property",
            "schema:rangeIncludes": {
                "@id": "xsd:token"
            },
            "schema:domainIncludes": {
                "@id": "fisheries:Problem"
            },
            "rdfs:comment": "A code specifying a measure for recovering this gear problem.",
            "rdfs:label": "recoveryMeasureCode",
            "unece:cefactElementMetadata": [
                {
                    "@id": "cefact:Gear_Problem.RecoveryMeasure.Code",
                    "@type": "unece:BasicBIE",
                    "unece:cefactUNId": "UN01011211",
                    "unece:cefactBieDomainClass": "cefact:Gear_Problem.Details",
                    "rdfs:comment": "A code specifying a measure for recovering this gear problem."
                }
            ]
        },
        {
            "@id": "fisheries:referenceDateTime",
            "@type": "rdf:Property",
            "schema:rangeIncludes": {
                "@id": "xsd:dateTime"
            },
            "schema:domainIncludes": {
                "@id": "fisheries:Report"
            },
            "rdfs:comment": "The reference date, time, date time or other data time value for this IS report.",
            "rdfs:label": "referenceDateTime",
            "unece:cefactElementMetadata": [
                {
                    "@id": "cefact:IS_Report.Reference.DateTime",
                    "@type": "unece:BasicBIE",
                    "unece:cefactUNId": "UN01013320",
                    "unece:cefactBieDomainClass": "cefact:IS_Report.Details",
                    "rdfs:comment": "The reference date, time, date time or other data time value for this IS report."
                }
            ]
        },
        {
            "@id": "fisheries:referencedId",
            "@type": "rdf:Property",
            "schema:rangeIncludes": {
                "@id": "xsd:token"
            },
            "schema:domainIncludes": {
                "@id": "fisheries:Document"
            },
            "rdfs:comment": [
                "The identifier of a referenced FLUX report document.",
                "The identifier of the referenced document to which this FLUX document responds."
            ],
            "rdfs:label": "referencedId",
            "unece:cefactElementMetadata": [
                {
                    "@id": "cefact:FLUXResponse_Document.Referenced_Identification.Identifier",
                    "@type": "unece:BasicBIE",
                    "unece:TDED": "1004",
                    "unece:cefactUNId": "UN01010250",
                    "unece:cefactBieDomainClass": "cefact:FLUXResponse_Document.Details",
                    "rdfs:comment": "The identifier of the referenced document to which this FLUX document responds."
                },
                {
                    "@id": "cefact:FLUXReport_Document.Referenced_Identification.Identifier",
                    "@type": "unece:BasicBIE",
                    "unece:TDED": "1004",
                    "unece:cefactUNId": "UN01010240",
                    "unece:cefactBieDomainClass": "cefact:FLUXReport_Document.Details",
                    "rdfs:comment": "The identifier of a referenced FLUX report document."
                }
            ]
        },
        {
            "@id": "fisheries:referencedItem",
            "@type": "rdf:Property",
            "schema:rangeIncludes": {
                "@id": "xsd:string"
            },
            "schema:domainIncludes": {
                "@id": "fisheries:QualityAnalysis"
            },
            "rdfs:comment": "A referenced item, expressed as text, for this quality analysis of a validation process.",
            "rdfs:label": "referencedItem",
            "unece:cefactElementMetadata": [
                {
                    "@id": "cefact:Validation_QualityAnalysis.Referenced_Item.Text",
                    "@type": "unece:BasicBIE",
                    "unece:cefactUNId": "UN01010767",
                    "unece:cefactBieDomainClass": "cefact:Validation_QualityAnalysis.Details",
                    "rdfs:comment": "A referenced item, expressed as text, for this quality analysis of a validation process."
                }
            ]
        },
        {
            "@id": "fisheries:regimeManagementCode",
            "@type": "rdf:Property",
            "schema:rangeIncludes": {
                "@id": "xsd:token"
            },
            "schema:domainIncludes": {
                "@id": "fisheries:Status"
            },
            "rdfs:comment": "The management regime code specified for this inspected vessel status.",
            "rdfs:label": "regimeManagementCode",
            "unece:cefactElementMetadata": [
                {
                    "@id": "cefact:InspectedVessel_Status.Regime_Management.Code",
                    "@type": "unece:BasicBIE",
                    "unece:cefactUNId": "UN01013335",
                    "unece:cefactBieDomainClass": "cefact:InspectedVessel_Status.Details",
                    "rdfs:comment": "The management regime code specified for this inspected vessel status."
                }
            ]
        },
        {
            "@id": "fisheries:regionalAreaCode",
            "@type": "rdf:Property",
            "schema:rangeIncludes": {
                "@id": "xsd:token"
            },
            "schema:domainIncludes": {
                "@id": "fisheries:ACDRReport"
            },
            "rdfs:comment": "The code, as defined by a regional body, specifying an area for this FLUX ACDR report.",
            "rdfs:label": "regionalAreaCode",
            "unece:cefactElementMetadata": [
                {
                    "@id": "cefact:FLUX_ACDRReport.RegionalArea.Code",
                    "@type": "unece:BasicBIE",
                    "unece:cefactUNId": "UN01010270",
                    "unece:cefactBieDomainClass": "cefact:FLUX_ACDRReport.Details",
                    "rdfs:comment": "The code, as defined by a regional body, specifying an area for this FLUX ACDR report."
                }
            ]
        },
        {
            "@id": "fisheries:regionalFisheriesManagementOrganizationCode",
            "@type": "rdf:Property",
            "schema:rangeIncludes": {
                "@id": "xsd:token"
            },
            "schema:domainIncludes": {
                "@id": "fisheries:Location"
            },
            "rdfs:comment": "The code specifying the organization managing the regional fisheries at this FLUX location.",
            "rdfs:label": "regionalFisheriesManagementOrganizationCode",
            "unece:cefactElementMetadata": [
                {
                    "@id": "cefact:FLUX_Location.RegionalFisheries_ManagementOrganization.Code",
                    "@type": "unece:BasicBIE",
                    "unece:cefactUNId": "UN01011203",
                    "unece:cefactBieDomainClass": "cefact:FLUX_Location.Details",
                    "rdfs:comment": "The code specifying the organization managing the regional fisheries at this FLUX location."
                }
            ]
        },
        {
            "@id": "fisheries:regionalSpeciesCode",
            "@type": "rdf:Property",
            "schema:rangeIncludes": {
                "@id": "xsd:token"
            },
            "schema:domainIncludes": {
                "@id": "fisheries:ACDRReport"
            },
            "rdfs:comment": "The code, as defined by a regional body, specifying a species covered by this FLUX ACDR report.",
            "rdfs:label": "regionalSpeciesCode",
            "unece:cefactElementMetadata": [
                {
                    "@id": "cefact:FLUX_ACDRReport.RegionalSpecies.Code",
                    "@type": "unece:BasicBIE",
                    "unece:cefactUNId": "UN01010271",
                    "unece:cefactBieDomainClass": "cefact:FLUX_ACDRReport.Details",
                    "rdfs:comment": "The code, as defined by a regional body, specifying a species covered by this FLUX ACDR report."
                }
            ]
        },
        {
            "@id": "fisheries:registrationCountry",
            "@type": "rdf:Property",
            "schema:rangeIncludes": {
                "@id": "fisheries:Country"
            },
            "schema:domainIncludes": {
                "@id": "fisheries:TransportMeans"
            },
            "rdfs:comment": "The country of registration of this transport means vessel.",
            "rdfs:label": "registrationCountry",
            "unece:cefactElementMetadata": [
                {
                    "@id": "cefact:Vessel_TransportMeans.Registration.Vessel_Country",
                    "@type": "unece:AssociationBIE",
                    "unece:cefactUNId": "UN01010229",
                    "unece:cefactBieDomainClass": "cefact:Vessel_TransportMeans.Details",
                    "rdfs:comment": "The country of registration of this transport means vessel."
                }
            ]
        },
        {
            "@id": "fisheries:registrationCountryId",
            "@type": "rdf:Property",
            "schema:rangeIncludes": {
                "@id": "xsd:token"
            },
            "schema:domainIncludes": {
                "@id": "fisheries:TransportMeans"
            },
            "rdfs:comment": "The identifier of the country of registration for this vehicle transport means.",
            "rdfs:label": "registrationCountryId",
            "unece:cefactElementMetadata": [
                {
                    "@id": "cefact:Vehicle_TransportMeans.RegistrationCountry_Identification.Identifier",
                    "@type": "unece:BasicBIE",
                    "unece:TDED": "8213",
                    "unece:cefactUNId": "UN01010989",
                    "unece:cefactBieDomainClass": "cefact:Vehicle_TransportMeans.Details",
                    "rdfs:comment": "The identifier of the country of registration for this vehicle transport means."
                }
            ]
        },
        {
            "@id": "fisheries:rejectionReason",
            "@type": "rdf:Property",
            "schema:rangeIncludes": {
                "@id": "xsd:string"
            },
            "schema:domainIncludes": {
                "@id": "fisheries:Document"
            },
            "rdfs:comment": "The rejection reason, expressed as text, in this FLUX response document.",
            "rdfs:label": "rejectionReason",
            "unece:cefactElementMetadata": [
                {
                    "@id": "cefact:FLUXResponse_Document.RejectionReason.Text",
                    "@type": "unece:BasicBIE",
                    "unece:TDED": "4308",
                    "unece:cefactUNId": "UN01010254",
                    "unece:cefactBieDomainClass": "cefact:FLUXResponse_Document.Details",
                    "rdfs:comment": "The rejection reason, expressed as text, in this FLUX response document."
                }
            ]
        },
        {
            "@id": "fisheries:relatedActivity",
            "@type": "rdf:Property",
            "schema:rangeIncludes": {
                "@id": "fisheries:Activity"
            },
            "schema:domainIncludes": {
                "@id": "fisheries:Activity"
            },
            "rdfs:comment": "A fishing activity related to this fishing activity.",
            "rdfs:label": "relatedActivity",
            "unece:cefactElementMetadata": [
                {
                    "@id": "cefact:Fishing_Activity.Related.Fishing_Activity",
                    "@type": "unece:AssociationBIE",
                    "unece:cefactUNId": "UN01011185",
                    "unece:cefactBieDomainClass": "cefact:Fishing_Activity.Details",
                    "rdfs:comment": "A fishing activity related to this fishing activity."
                }
            ]
        },
        {
            "@id": "fisheries:relatedBatch",
            "@type": "rdf:Property",
            "schema:rangeIncludes": {
                "@id": "fisheries:Batch"
            },
            "schema:domainIncludes": [
                {
                    "@id": "fisheries:Catch"
                },
                {
                    "@id": "fisheries:Event"
                }
            ],
            "rdfs:comment": [
                "A batch related to this sales event.",
                "A sales batch related to this FA catch."
            ],
            "rdfs:label": "relatedBatch",
            "unece:cefactElementMetadata": [
                {
                    "@id": "cefact:FA_Catch.Related.Sales_Batch",
                    "@type": "unece:AssociationBIE",
                    "unece:cefactUNId": "UN01011195",
                    "unece:cefactBieDomainClass": "cefact:FA_Catch.Details",
                    "rdfs:comment": "A sales batch related to this FA catch."
                },
                {
                    "@id": "cefact:Sales_Event.Related.Sales_Batch",
                    "@type": "unece:AssociationBIE",
                    "unece:cefactUNId": "UN01010951",
                    "unece:cefactBieDomainClass": "cefact:Sales_Event.Details",
                    "rdfs:comment": "A batch related to this sales event."
                }
            ]
        },
        {
            "@id": "fisheries:relatedCatch",
            "@type": "rdf:Property",
            "schema:rangeIncludes": {
                "@id": "fisheries:Catch"
            },
            "schema:domainIncludes": {
                "@id": "fisheries:Report"
            },
            "rdfs:comment": "A Fishing Activity (FA) catch related to this IS report.",
            "rdfs:label": "relatedCatch",
            "unece:cefactElementMetadata": [
                {
                    "@id": "cefact:IS_Report.Related.FA_Catch",
                    "@type": "unece:AssociationBIE",
                    "unece:cefactUNId": "UN01012600",
                    "unece:cefactBieDomainClass": "cefact:IS_Report.Details",
                    "rdfs:comment": "A Fishing Activity (FA) catch related to this IS report."
                }
            ]
        },
        {
            "@id": "fisheries:relatedCategory",
            "@type": "rdf:Property",
            "schema:rangeIncludes": {
                "@id": "fisheries:Category"
            },
            "schema:domainIncludes": {
                "@id": "fisheries:Document"
            },
            "rdfs:comment": "The fishing category related to this FLAP request document.",
            "rdfs:label": "relatedCategory",
            "unece:cefactElementMetadata": [
                {
                    "@id": "cefact:FLAPRequest_Document.Related.Fishing_Category",
                    "@type": "unece:AssociationBIE",
                    "unece:cefactUNId": "UN01010835",
                    "unece:cefactBieDomainClass": "cefact:FLAPRequest_Document.Details",
                    "rdfs:comment": "The fishing category related to this FLAP request document."
                }
            ]
        },
        {
            "@id": "fisheries:relatedCharacteristic",
            "@type": "rdf:Property",
            "schema:rangeIncludes": {
                "@id": "fisheries:Characteristic"
            },
            "schema:domainIncludes": [
                {
                    "@id": "fisheries:Event"
                },
                {
                    "@id": "fisheries:Report"
                }
            ],
            "rdfs:comment": [
                "A characteristic of a gear related to this gear inspection event.",
                "A vessel historical characteristic related to this event.",
                "An Inspection or Surveillance Report (ISR) item characteristic related to this IS report."
            ],
            "rdfs:label": "relatedCharacteristic",
            "unece:cefactElementMetadata": [
                {
                    "@id": "cefact:IS_Report.Related.ISRItem_Characteristic",
                    "@type": "unece:AssociationBIE",
                    "unece:cefactUNId": "UN01012596",
                    "unece:cefactBieDomainClass": "cefact:IS_Report.Details",
                    "rdfs:comment": "An Inspection or Surveillance Report (ISR) item characteristic related to this IS report."
                },
                {
                    "@id": "cefact:GearInspection_Event.Related.Gear_Characteristic",
                    "@type": "unece:AssociationBIE",
                    "unece:cefactUNId": "UN01012628",
                    "unece:cefactBieDomainClass": "cefact:GearInspection_Event.Details",
                    "rdfs:comment": "A characteristic of a gear related to this gear inspection event."
                },
                {
                    "@id": "cefact:Vessel_Event.Related.VesselHistorical_Characteristic",
                    "@type": "unece:AssociationBIE",
                    "unece:cefactUNId": "UN01010666",
                    "unece:cefactBieDomainClass": "cefact:Vessel_Event.Details",
                    "rdfs:comment": "A vessel historical characteristic related to this event."
                }
            ]
        },
        {
            "@id": "fisheries:relatedDocument",
            "@type": "rdf:Property",
            "schema:rangeIncludes": {
                "@id": "fisheries:Document"
            },
            "schema:domainIncludes": [
                {
                    "@id": "fisheries:Characteristic"
                },
                {
                    "@id": "fisheries:Document"
                },
                {
                    "@id": "fisheries:Event"
                }
            ],
            "rdfs:comment": [
                "A Fishing Licence, Authorization or Permit (FLAP) document related to this FLUX characteristic.",
                "A request document related to this FLAP document.",
                "A result document of a validation process related to this FLAP document.",
                "A result document of a validation process related to this FLAP request document.",
                "A result document of a validation process related to this sales document.",
                "A validation result document related to this FLUX response document.",
                "The Fisheries Language for Universal eXchange (FLUX) report document related to this FA report document.",
                "The validation result document related to this vessel event."
            ],
            "rdfs:label": "relatedDocument",
            "unece:cefactElementMetadata": [
                {
                    "@id": "cefact:FLAPRequest_Document.Related.ValidationResult_Document",
                    "@type": "unece:AssociationBIE",
                    "unece:cefactUNId": "UN01010836",
                    "unece:cefactBieDomainClass": "cefact:FLAPRequest_Document.Details",
                    "rdfs:comment": "A result document of a validation process related to this FLAP request document."
                },
                {
                    "@id": "cefact:FLAP_Document.Related.FLAPRequest_Document",
                    "@type": "unece:AssociationBIE",
                    "unece:cefactUNId": "UN01010863",
                    "unece:cefactBieDomainClass": "cefact:FLAP_Document.Details",
                    "rdfs:comment": "A request document related to this FLAP document."
                },
                {
                    "@id": "cefact:FLUXResponse_Document.Related.ValidationResult_Document",
                    "@type": "unece:AssociationBIE",
                    "unece:cefactUNId": "UN01010762",
                    "unece:cefactBieDomainClass": "cefact:FLUXResponse_Document.Details",
                    "rdfs:comment": "A validation result document related to this FLUX response document."
                },
                {
                    "@id": "cefact:FLAP_Document.Related.ValidationResult_Document",
                    "@type": "unece:AssociationBIE",
                    "unece:cefactUNId": "UN01010862",
                    "unece:cefactBieDomainClass": "cefact:FLAP_Document.Details",
                    "rdfs:comment": "A result document of a validation process related to this FLAP document."
                },
                {
                    "@id": "cefact:FLUX_Characteristic.Related.FLAP_Document",
                    "@type": "unece:AssociationBIE",
                    "unece:cefactUNId": "UN01012122",
                    "unece:cefactBieDomainClass": "cefact:FLUX_Characteristic.Details",
                    "rdfs:comment": "A Fishing Licence, Authorization or Permit (FLAP) document related to this FLUX characteristic."
                },
                {
                    "@id": "cefact:Vessel_Event.Related.ValidationResult_Document",
                    "@type": "unece:AssociationBIE",
                    "unece:cefactUNId": "UN01010665",
                    "unece:cefactBieDomainClass": "cefact:Vessel_Event.Details",
                    "rdfs:comment": "The validation result document related to this vessel event."
                },
                {
                    "@id": "cefact:FAReport_Document.Related.FLUXReport_Document",
                    "@type": "unece:AssociationBIE",
                    "unece:cefactUNId": "UN01011161",
                    "unece:cefactBieDomainClass": "cefact:FAReport_Document.Details",
                    "rdfs:comment": "The Fisheries Language for Universal eXchange (FLUX) report document related to this FA report document."
                },
                {
                    "@id": "cefact:Sales_Document.Related.ValidationResult_Document",
                    "@type": "unece:AssociationBIE",
                    "unece:cefactUNId": "UN01010921",
                    "unece:cefactBieDomainClass": "cefact:Sales_Document.Details",
                    "rdfs:comment": "A result document of a validation process related to this sales document."
                }
            ]
        },
        {
            "@id": "fisheries:relatedEvent",
            "@type": "rdf:Property",
            "schema:rangeIncludes": {
                "@id": "fisheries:Event"
            },
            "schema:domainIncludes": [
                {
                    "@id": "fisheries:Equipment"
                },
                {
                    "@id": "fisheries:Gear"
                }
            ],
            "rdfs:comment": [
                "A gear equipment inspection event related to this fishing gear equipment.",
                "A gear inspection event related to this fishing gear."
            ],
            "rdfs:label": "relatedEvent",
            "unece:cefactElementMetadata": [
                {
                    "@id": "cefact:FishingGear_Equipment.Related.GearEquipmentInspection_Event",
                    "@type": "unece:AssociationBIE",
                    "unece:cefactUNId": "UN01013333",
                    "unece:cefactBieDomainClass": "cefact:FishingGear_Equipment.Details",
                    "rdfs:comment": "A gear equipment inspection event related to this fishing gear equipment."
                },
                {
                    "@id": "cefact:Fishing_Gear.Related.GearInspection_Event",
                    "@type": "unece:AssociationBIE",
                    "unece:cefactUNId": "UN01012622",
                    "unece:cefactBieDomainClass": "cefact:Fishing_Gear.Details",
                    "rdfs:comment": "A gear inspection event related to this fishing gear."
                }
            ]
        },
        {
            "@id": "fisheries:relatedGear",
            "@type": "rdf:Property",
            "schema:rangeIncludes": {
                "@id": "fisheries:Gear"
            },
            "schema:domainIncludes": {
                "@id": "fisheries:Problem"
            },
            "rdfs:comment": "A fishing gear related to this gear problem.",
            "rdfs:label": "relatedGear",
            "unece:cefactElementMetadata": [
                {
                    "@id": "cefact:Gear_Problem.Related.Fishing_Gear",
                    "@type": "unece:AssociationBIE",
                    "unece:cefactUNId": "UN01011213",
                    "unece:cefactBieDomainClass": "cefact:Gear_Problem.Details",
                    "rdfs:comment": "A fishing gear related to this gear problem."
                }
            ]
        },
        {
            "@id": "fisheries:relatedLocation",
            "@type": "rdf:Property",
            "schema:rangeIncludes": {
                "@id": "fisheries:Location"
            },
            "schema:domainIncludes": {
                "@id": "fisheries:Activity"
            },
            "rdfs:comment": "A Fisheries Language for Universal eXchange (FLUX) location related to this fishing activity.",
            "rdfs:label": "relatedLocation",
            "unece:cefactElementMetadata": [
                {
                    "@id": "cefact:Fishing_Activity.Related.FLUX_Location",
                    "@type": "unece:AssociationBIE",
                    "unece:cefactUNId": "UN01011179",
                    "unece:cefactBieDomainClass": "cefact:Fishing_Activity.Details",
                    "rdfs:comment": "A Fisheries Language for Universal eXchange (FLUX) location related to this fishing activity."
                }
            ]
        },
        {
            "@id": "fisheries:relatedQualityAnalysis",
            "@type": "rdf:Property",
            "schema:rangeIncludes": {
                "@id": "fisheries:QualityAnalysis"
            },
            "schema:domainIncludes": [
                {
                    "@id": "fisheries:Document"
                },
                {
                    "@id": "fisheries:Event"
                }
            ],
            "rdfs:comment": [
                "A validation quality analysis related to this vessel event.",
                "Quality analysis related to this validation result document."
            ],
            "rdfs:label": "relatedQualityAnalysis",
            "unece:cefactElementMetadata": [
                {
                    "@id": "cefact:Vessel_Event.Related.Validation_QualityAnalysis",
                    "@type": "unece:AssociationBIE",
                    "unece:cefactUNId": "UN01012121",
                    "unece:cefactBieDomainClass": "cefact:Vessel_Event.Details",
                    "rdfs:comment": "A validation quality analysis related to this vessel event."
                },
                {
                    "@id": "cefact:ValidationResult_Document.Related.Validation_QualityAnalysis",
                    "@type": "unece:AssociationBIE",
                    "unece:cefactUNId": "UN01010753",
                    "unece:cefactBieDomainClass": "cefact:ValidationResult_Document.Details",
                    "rdfs:comment": "Quality analysis related to this validation result document."
                }
            ]
        },
        {
            "@id": "fisheries:relatedReportId",
            "@type": "rdf:Property",
            "schema:rangeIncludes": {
                "@id": "xsd:token"
            },
            "schema:domainIncludes": {
                "@id": "fisheries:Document"
            },
            "rdfs:comment": "An identifier of a report related to this FA report document.",
            "rdfs:label": "relatedReportId",
            "unece:cefactElementMetadata": [
                {
                    "@id": "cefact:FAReport_Document.Related_Report.Identifier",
                    "@type": "unece:BasicBIE",
                    "unece:cefactUNId": "UN01011159",
                    "unece:cefactBieDomainClass": "cefact:FAReport_Document.Details",
                    "rdfs:comment": "An identifier of a report related to this FA report document."
                }
            ]
        },
        {
            "@id": "fisheries:relatedStock",
            "@type": "rdf:Property",
            "schema:rangeIncludes": {
                "@id": "fisheries:Stock"
            },
            "schema:domainIncludes": {
                "@id": "fisheries:Catch"
            },
            "rdfs:comment": "An Aquatic Animal or Plant (AAP) stock related to this FA catch.",
            "rdfs:label": "relatedStock",
            "unece:cefactElementMetadata": [
                {
                    "@id": "cefact:FA_Catch.Related.AAP_Stock",
                    "@type": "unece:AssociationBIE",
                    "unece:cefactUNId": "UN01011193",
                    "unece:cefactBieDomainClass": "cefact:FA_Catch.Details",
                    "rdfs:comment": "An Aquatic Animal or Plant (AAP) stock related to this FA catch."
                }
            ]
        },
        {
            "@id": "fisheries:relatedTransportMeans",
            "@type": "rdf:Property",
            "schema:rangeIncludes": {
                "@id": "fisheries:TransportMeans"
            },
            "schema:domainIncludes": [
                {
                    "@id": "fisheries:Activity"
                },
                {
                    "@id": "fisheries:Event"
                }
            ],
            "rdfs:comment": [
                "A vessel transport means related to this fishing activity.",
                "The vessel transport means related to this vessel event."
            ],
            "rdfs:label": "relatedTransportMeans",
            "unece:cefactElementMetadata": [
                {
                    "@id": "cefact:Fishing_Activity.Related.Vessel_TransportMeans",
                    "@type": "unece:AssociationBIE",
                    "unece:cefactUNId": "UN01011189",
                    "unece:cefactBieDomainClass": "cefact:Fishing_Activity.Details",
                    "rdfs:comment": "A vessel transport means related to this fishing activity."
                },
                {
                    "@id": "cefact:Vessel_Event.Related.Vessel_TransportMeans",
                    "@type": "unece:AssociationBIE",
                    "unece:cefactUNId": "UN01010664",
                    "unece:cefactBieDomainClass": "cefact:Vessel_Event.Details",
                    "rdfs:comment": "The vessel transport means related to this vessel event."
                }
            ]
        },
        {
            "@id": "fisheries:relatedTrip",
            "@type": "rdf:Property",
            "schema:rangeIncludes": {
                "@id": "fisheries:Trip"
            },
            "schema:domainIncludes": {
                "@id": "fisheries:Catch"
            },
            "rdfs:comment": "A fishing trip related to this FA catch.",
            "rdfs:label": "relatedTrip",
            "unece:cefactElementMetadata": [
                {
                    "@id": "cefact:FA_Catch.Related.Fishing_Trip",
                    "@type": "unece:AssociationBIE",
                    "unece:cefactUNId": "UN01011191",
                    "unece:cefactBieDomainClass": "cefact:FA_Catch.Details",
                    "rdfs:comment": "A fishing trip related to this FA catch."
                }
            ]
        },
        {
            "@id": "fisheries:remarks",
            "@type": "rdf:Property",
            "schema:rangeIncludes": {
                "@id": "xsd:string"
            },
            "schema:domainIncludes": {
                "@id": "fisheries:Document"
            },
            "rdfs:comment": [
                "Remarks, expressed as text, in this FLAP document.",
                "Remarks, expressed as text, in this FLUX response document."
            ],
            "rdfs:label": "remarks",
            "unece:cefactElementMetadata": [
                {
                    "@id": "cefact:FLAP_Document.Remarks.Text",
                    "@type": "unece:BasicBIE",
                    "unece:cefactUNId": "UN01010851",
                    "unece:cefactBieDomainClass": "cefact:FLAP_Document.Details",
                    "rdfs:comment": "Remarks, expressed as text, in this FLAP document."
                },
                {
                    "@id": "cefact:FLUXResponse_Document.Remarks.Text",
                    "@type": "unece:BasicBIE",
                    "unece:cefactUNId": "UN01010253",
                    "unece:cefactBieDomainClass": "cefact:FLUXResponse_Document.Details",
                    "rdfs:comment": "Remarks, expressed as text, in this FLUX response document."
                }
            ]
        },
        {
            "@id": "fisheries:requestId",
            "@type": "rdf:Property",
            "schema:rangeIncludes": {
                "@id": "xsd:token"
            },
            "schema:domainIncludes": {
                "@id": "fisheries:Identity"
            },
            "rdfs:comment": "The identifier of a request for this FLAP identity.",
            "rdfs:label": "requestId",
            "unece:cefactElementMetadata": [
                {
                    "@id": "cefact:FLAP_Identity.Request_Identification.Identifier",
                    "@type": "unece:BasicBIE",
                    "unece:cefactUNId": "UN01010896",
                    "unece:cefactBieDomainClass": "cefact:FLAP_Identity.Details",
                    "rdfs:comment": "The identifier of a request for this FLAP identity."
                }
            ]
        },
        {
            "@id": "fisheries:respondentParty",
            "@type": "rdf:Property",
            "schema:rangeIncludes": {
                "@id": "fisheries:Party"
            },
            "schema:domainIncludes": {
                "@id": "fisheries:Document"
            },
            "rdfs:comment": "The respondent party for this FLUX Response.",
            "rdfs:label": "respondentParty",
            "unece:cefactElementMetadata": [
                {
                    "@id": "cefact:FLUXResponse_Document.Respondent.FLUX_Party",
                    "@type": "unece:AssociationBIE",
                    "unece:cefactUNId": "UN01010763",
                    "unece:cefactBieDomainClass": "cefact:FLUXResponse_Document.Details",
                    "rdfs:comment": "The respondent party for this FLUX Response."
                }
            ]
        },
        {
            "@id": "fisheries:responseCode",
            "@type": "rdf:Property",
            "schema:rangeIncludes": {
                "@id": "xsd:token"
            },
            "schema:domainIncludes": {
                "@id": "fisheries:Document"
            },
            "rdfs:comment": "The code indicating the response in this FLUX response document.",
            "rdfs:label": "responseCode",
            "unece:cefactElementMetadata": [
                {
                    "@id": "cefact:FLUXResponse_Document.Response.Code",
                    "@type": "unece:BasicBIE",
                    "unece:cefactUNId": "UN01010252",
                    "unece:cefactBieDomainClass": "cefact:FLUXResponse_Document.Details",
                    "rdfs:comment": "The code indicating the response in this FLUX response document."
                }
            ]
        },
        {
            "@id": "fisheries:result",
            "@type": "rdf:Property",
            "schema:rangeIncludes": {
                "@id": "xsd:string"
            },
            "schema:domainIncludes": {
                "@id": "fisheries:QualityAnalysis"
            },
            "rdfs:comment": "A result, expressed as text, in this quality analysis of a validation process.",
            "rdfs:label": "result",
            "unece:cefactElementMetadata": [
                {
                    "@id": "cefact:Validation_QualityAnalysis.Result.Text",
                    "@type": "unece:BasicBIE",
                    "unece:cefactUNId": "UN01010757",
                    "unece:cefactBieDomainClass": "cefact:Validation_QualityAnalysis.Details",
                    "rdfs:comment": "A result, expressed as text, in this quality analysis of a validation process."
                }
            ]
        },
        {
            "@id": "fisheries:resultProduct",
            "@type": "rdf:Property",
            "schema:rangeIncludes": {
                "@id": "fisheries:Product"
            },
            "schema:domainIncludes": {
                "@id": "fisheries:Process"
            },
            "rdfs:comment": "An Aquatic Animal or Plant (AAP) product resulting from this process.",
            "rdfs:label": "resultProduct",
            "unece:cefactElementMetadata": [
                {
                    "@id": "cefact:AAP_Process.Result.AAP_Product",
                    "@type": "unece:AssociationBIE",
                    "unece:cefactUNId": "UN01011151",
                    "unece:cefactBieDomainClass": "cefact:AAP_Process.Details",
                    "rdfs:comment": "An Aquatic Animal or Plant (AAP) product resulting from this process."
                }
            ]
        },
        {
            "@id": "fisheries:roleCode",
            "@type": "rdf:Property",
            "schema:rangeIncludes": {
                "@id": "xsd:token"
            },
            "schema:domainIncludes": [
                {
                    "@id": "fisheries:Engine"
                },
                {
                    "@id": "fisheries:Gear"
                },
                {
                    "@id": "fisheries:TransportMeans"
                }
            ],
            "rdfs:comment": [
                "A code specifying the role of this fishing gear, such as main gear, subsidiary gear.",
                "The code specifying the role of this vehicle transport means.",
                "The code specifying the role of this vessel engine, such as main or secondary.",
                "The code specifying the role of this vessel transport means."
            ],
            "rdfs:label": "roleCode",
            "unece:cefactElementMetadata": [
                {
                    "@id": "cefact:Vehicle_TransportMeans.Role.Code",
                    "@type": "unece:BasicBIE",
                    "unece:cefactUNId": "UN01013337",
                    "unece:cefactBieDomainClass": "cefact:Vehicle_TransportMeans.Details",
                    "rdfs:comment": "The code specifying the role of this vehicle transport means."
                },
                {
                    "@id": "cefact:Vessel_Engine.Role.Code",
                    "@type": "unece:BasicBIE",
                    "unece:cefactUNId": "UN01010720",
                    "unece:cefactBieDomainClass": "cefact:Vessel_Engine.Details",
                    "rdfs:comment": "The code specifying the role of this vessel engine, such as main or secondary."
                },
                {
                    "@id": "cefact:Vessel_TransportMeans.Role.Code",
                    "@type": "unece:BasicBIE",
                    "unece:cefactUNId": "UN01011229",
                    "unece:cefactBieDomainClass": "cefact:Vessel_TransportMeans.Details",
                    "rdfs:comment": "The code specifying the role of this vessel transport means."
                },
                {
                    "@id": "cefact:Fishing_Gear.Role.Code",
                    "@type": "unece:BasicBIE",
                    "unece:cefactUNId": "UN01010728",
                    "unece:cefactBieDomainClass": "cefact:Fishing_Gear.Details",
                    "rdfs:comment": "A code specifying the role of this fishing gear, such as main gear, subsidiary gear."
                }
            ]
        },
        {
            "@id": "fisheries:salesNoteId",
            "@type": "rdf:Property",
            "schema:rangeIncludes": {
                "@id": "xsd:token"
            },
            "schema:domainIncludes": {
                "@id": "fisheries:Document"
            },
            "rdfs:comment": "A sales note identifier for this sales document.",
            "rdfs:label": "salesNoteId",
            "unece:cefactElementMetadata": [
                {
                    "@id": "cefact:Sales_Document.SalesNote_Identification.Identifier",
                    "@type": "unece:BasicBIE",
                    "unece:TDED": "1004",
                    "unece:cefactUNId": "UN01010913",
                    "unece:cefactBieDomainClass": "cefact:Sales_Document.Details",
                    "rdfs:comment": "A sales note identifier for this sales document."
                }
            ]
        },
        {
            "@id": "fisheries:salesPartyRoleCode",
            "@type": "rdf:Property",
            "schema:rangeIncludes": {
                "@id": "unece:UNECECL3035Code"
            },
            "schema:domainIncludes": {
                "@id": "fisheries:Party"
            },
            "rdfs:comment": "A code specifying the role of this sales party.",
            "rdfs:label": "salesPartyRoleCode",
            "unece:cefactElementMetadata": [
                {
                    "@id": "cefact:Sales_Party.Role.Code",
                    "@type": "unece:BasicBIE",
                    "unece:TDED": "3035",
                    "unece:cefactUNId": "UN01010927",
                    "unece:cefactBieDomainClass": "cefact:Sales_Party.Details",
                    "rdfs:comment": "A code specifying the role of this sales party."
                }
            ]
        },
        {
            "@id": "fisheries:searchTypeCode",
            "@type": "rdf:Property",
            "schema:rangeIncludes": {
                "@id": "xsd:token"
            },
            "schema:domainIncludes": {
                "@id": "fisheries:QueryParameter"
            },
            "rdfs:comment": "The code specifying the type of search parameter for this vessel query, such as full or partial.",
            "rdfs:label": "searchTypeCode",
            "unece:cefactElementMetadata": [
                {
                    "@id": "cefact:Vessel_QueryParameter.Search_Type.Code",
                    "@type": "unece:BasicBIE",
                    "unece:cefactUNId": "UN01010749",
                    "unece:cefactBieDomainClass": "cefact:Vessel_QueryParameter.Details",
                    "rdfs:comment": "The code specifying the type of search parameter for this vessel query, such as full or partial."
                }
            ]
        },
        {
            "@id": "fisheries:sellerName",
            "@type": "rdf:Property",
            "schema:rangeIncludes": {
                "@id": "xsd:string"
            },
            "schema:domainIncludes": {
                "@id": "fisheries:Event"
            },
            "rdfs:comment": "The name of the seller, such as company name or name of an individual, expressed as text, for this sales event.",
            "rdfs:label": "sellerName",
            "unece:cefactElementMetadata": [
                {
                    "@id": "cefact:Sales_Event.Seller_Name.Text",
                    "@type": "unece:BasicBIE",
                    "unece:cefactUNId": "UN01010949",
                    "unece:cefactBieDomainClass": "cefact:Sales_Event.Details",
                    "rdfs:comment": "The name of the seller, such as company name or name of an individual, expressed as text, for this sales event."
                }
            ]
        },
        {
            "@id": "fisheries:serialNumberId",
            "@type": "rdf:Property",
            "schema:rangeIncludes": {
                "@id": "xsd:token"
            },
            "schema:domainIncludes": {
                "@id": "fisheries:Engine"
            },
            "rdfs:comment": "The serial number identifier of this vessel engine.",
            "rdfs:label": "serialNumberId",
            "unece:cefactElementMetadata": [
                {
                    "@id": "cefact:Vessel_Engine.SerialNumber.Identifier",
                    "@type": "unece:BasicBIE",
                    "unece:cefactUNId": "UN01010718",
                    "unece:cefactBieDomainClass": "cefact:Vessel_Engine.Details",
                    "rdfs:comment": "The serial number identifier of this vessel engine."
                }
            ]
        },
        {
            "@id": "fisheries:seriousViolationIndicator",
            "@type": "rdf:Property",
            "schema:rangeIncludes": {
                "@id": "xsd:boolean"
            },
            "schema:domainIncludes": {
                "@id": "fisheries:Suspicion"
            },
            "rdfs:comment": "The indication of whether or not this ISR infringement suspicion is a serious violation.",
            "rdfs:label": "seriousViolationIndicator",
            "unece:cefactElementMetadata": [
                {
                    "@id": "cefact:ISRInfringement_Suspicion.SeriousViolation.Indicator",
                    "@type": "unece:BasicBIE",
                    "unece:cefactUNId": "UN01013327",
                    "unece:cefactBieDomainClass": "cefact:ISRInfringement_Suspicion.Details",
                    "rdfs:comment": "The indication of whether or not this ISR infringement suspicion is a serious violation."
                }
            ]
        },
        {
            "@id": "fisheries:simpleQueryParameter",
            "@type": "rdf:Property",
            "schema:rangeIncludes": {
                "@id": "fisheries:QueryParameter"
            },
            "schema:domainIncludes": {
                "@id": "fisheries:Query"
            },
            "rdfs:comment": [
                "A simple query parameter for this FA query.",
                "A simple query parameter for this ISR query.",
                "A simple query parameter for this sales query.",
                "A simple vessel query parameter for this vessel query."
            ],
            "rdfs:label": "simpleQueryParameter",
            "unece:cefactElementMetadata": [
                {
                    "@id": "cefact:FA_Query.Simple.FA_QueryParameter",
                    "@type": "unece:AssociationBIE",
                    "unece:cefactUNId": "UN01011223",
                    "unece:cefactBieDomainClass": "cefact:FA_Query.Details",
                    "rdfs:comment": "A simple query parameter for this FA query."
                },
                {
                    "@id": "cefact:Sales_Query.Simple.Sales_QueryParameter",
                    "@type": "unece:AssociationBIE",
                    "unece:cefactUNId": "UN01010999",
                    "unece:cefactBieDomainClass": "cefact:Sales_Query.Details",
                    "rdfs:comment": "A simple query parameter for this sales query."
                },
                {
                    "@id": "cefact:Vessel_Query.Simple.Vessel_QueryParameter",
                    "@type": "unece:AssociationBIE",
                    "unece:cefactUNId": "UN01010740",
                    "unece:cefactBieDomainClass": "cefact:Vessel_Query.Details",
                    "rdfs:comment": "A simple vessel query parameter for this vessel query."
                },
                {
                    "@id": "cefact:ISR_Query.Simple.ISR_QueryParameter",
                    "@type": "unece:AssociationBIE",
                    "unece:cefactUNId": "UN01012640",
                    "unece:cefactBieDomainClass": "cefact:ISR_Query.Details",
                    "rdfs:comment": "A simple query parameter for this ISR query."
                }
            ]
        },
        {
            "@id": "fisheries:sizeMeasure",
            "@type": "rdf:Property",
            "schema:rangeIncludes": {
                "@id": "xsd:decimal"
            },
            "schema:domainIncludes": {
                "@id": "fisheries:BinaryFile"
            },
            "rdfs:comment": "The measure of the size of this FLUX binary file.",
            "rdfs:label": "sizeMeasure",
            "unece:cefactElementMetadata": [
                {
                    "@id": "cefact:FLUX_BinaryFile.Size.Measure",
                    "@type": "unece:BasicBIE",
                    "unece:cefactUNId": "UN01010803",
                    "unece:cefactBieDomainClass": "cefact:FLUX_BinaryFile.Details",
                    "rdfs:comment": "The measure of the size of this FLUX binary file."
                }
            ]
        },
        {
            "@id": "fisheries:sourceCharacteristic",
            "@type": "rdf:Property",
            "schema:rangeIncludes": {
                "@id": "fisheries:Characteristic"
            },
            "schema:domainIncludes": {
                "@id": "fisheries:Activity"
            },
            "rdfs:comment": "The characteristic of a vessel storage, such as a cage, used as a source for this fishing activity.",
            "rdfs:label": "sourceCharacteristic",
            "unece:cefactElementMetadata": [
                {
                    "@id": "cefact:Fishing_Activity.Source.VesselStorage_Characteristic",
                    "@type": "unece:AssociationBIE",
                    "unece:cefactUNId": "UN01011183",
                    "unece:cefactBieDomainClass": "cefact:Fishing_Activity.Details",
                    "rdfs:comment": "The characteristic of a vessel storage, such as a cage, used as a source for this fishing activity."
                }
            ]
        },
        {
            "@id": "fisheries:sovereignRightsCountryId",
            "@type": "rdf:Property",
            "schema:rangeIncludes": {
                "@id": "xsd:token"
            },
            "schema:domainIncludes": {
                "@id": "fisheries:Location"
            },
            "rdfs:comment": "The identifier of the country exercising sovereign rights over this FLUX location.",
            "rdfs:label": "sovereignRightsCountryId",
            "unece:cefactElementMetadata": [
                {
                    "@id": "cefact:FLUX_Location.SovereignRights_Country.Identifier",
                    "@type": "unece:BasicBIE",
                    "unece:cefactUNId": "UN01011201",
                    "unece:cefactBieDomainClass": "cefact:FLUX_Location.Details",
                    "rdfs:comment": "The identifier of the country exercising sovereign rights over this FLUX location."
                }
            ]
        },
        {
            "@id": "fisheries:sovereigntyWaterCode",
            "@type": "rdf:Property",
            "schema:rangeIncludes": {
                "@id": "xsd:token"
            },
            "schema:domainIncludes": {
                "@id": "fisheries:ReportedArea"
            },
            "rdfs:comment": "The sovereignty water code specified for this ACDR reported area.",
            "rdfs:label": "sovereigntyWaterCode",
            "unece:cefactElementMetadata": [
                {
                    "@id": "cefact:ACDR_ReportedArea.SovereigntyWater.Code",
                    "@type": "unece:BasicBIE",
                    "unece:cefactUNId": "UN01010260",
                    "unece:cefactBieDomainClass": "cefact:ACDR_ReportedArea.Details",
                    "rdfs:comment": "The sovereignty water code specified for this ACDR reported area."
                }
            ]
        },
        {
            "@id": "fisheries:specialCondition",
            "@type": "rdf:Property",
            "schema:rangeIncludes": {
                "@id": "xsd:string"
            },
            "schema:domainIncludes": {
                "@id": "fisheries:Category"
            },
            "rdfs:comment": "The special condition, expressed as text, for this fishing category.",
            "rdfs:label": "specialCondition",
            "unece:cefactElementMetadata": [
                {
                    "@id": "cefact:Fishing_Category.SpecialCondition.Text",
                    "@type": "unece:BasicBIE",
                    "unece:cefactUNId": "UN01010843",
                    "unece:cefactBieDomainClass": "cefact:Fishing_Category.Details",
                    "rdfs:comment": "The special condition, expressed as text, for this fishing category."
                }
            ]
        },
        {
            "@id": "fisheries:speciesCode",
            "@type": "rdf:Property",
            "schema:rangeIncludes": {
                "@id": "xsd:token"
            },
            "schema:domainIncludes": [
                {
                    "@id": "fisheries:Catch"
                },
                {
                    "@id": "fisheries:Product"
                }
            ],
            "rdfs:comment": [
                "The code specifying the species for this AAP product, such as the Food and Agriculture Organization (FAO) code.",
                "The code specifying the species of this FA catch, such as the Food and Agriculture Organization (FAO) code."
            ],
            "rdfs:label": "speciesCode",
            "unece:cefactElementMetadata": [
                {
                    "@id": "cefact:AAP_Product.Species.Code",
                    "@type": "unece:BasicBIE",
                    "unece:cefactUNId": "UN01010934",
                    "unece:cefactBieDomainClass": "cefact:AAP_Product.Details",
                    "rdfs:comment": "The code specifying the species for this AAP product, such as the Food and Agriculture Organization (FAO) code."
                },
                {
                    "@id": "cefact:FA_Catch.Species.Code",
                    "@type": "unece:BasicBIE",
                    "unece:cefactUNId": "UN01010972",
                    "unece:cefactBieDomainClass": "cefact:FA_Catch.Details",
                    "rdfs:comment": "The code specifying the species of this FA catch, such as the Food and Agriculture Organization (FAO) code."
                }
            ]
        },
        {
            "@id": "fisheries:speciesTargetCode",
            "@type": "rdf:Property",
            "schema:rangeIncludes": {
                "@id": "xsd:token"
            },
            "schema:domainIncludes": {
                "@id": "fisheries:Activity"
            },
            "rdfs:comment": "The code specifying a species targeted for this fishing activity, such as the Food and Agriculture Organization (FAO) species code.",
            "rdfs:label": "speciesTargetCode",
            "unece:cefactElementMetadata": [
                {
                    "@id": "cefact:Fishing_Activity.Species_Target.Code",
                    "@type": "unece:BasicBIE",
                    "unece:cefactUNId": "UN01011175",
                    "unece:cefactBieDomainClass": "cefact:Fishing_Activity.Details",
                    "rdfs:comment": "The code specifying a species targeted for this fishing activity, such as the Food and Agriculture Organization (FAO) species code."
                }
            ]
        },
        {
            "@id": "fisheries:specifiedActivity",
            "@type": "rdf:Property",
            "schema:rangeIncludes": {
                "@id": "fisheries:Activity"
            },
            "schema:domainIncludes": [
                {
                    "@id": "fisheries:Document"
                },
                {
                    "@id": "fisheries:Report"
                }
            ],
            "rdfs:comment": [
                "A Fishing Activity, such as a landing operation, specified for this sales document.",
                "A fishing activity specified in this FA report document.",
                "A fishing activity specified in this IS report."
            ],
            "rdfs:label": "specifiedActivity",
            "unece:cefactElementMetadata": [
                {
                    "@id": "cefact:FAReport_Document.Specified.Fishing_Activity",
                    "@type": "unece:AssociationBIE",
                    "unece:cefactUNId": "UN01011162",
                    "unece:cefactBieDomainClass": "cefact:FAReport_Document.Details",
                    "rdfs:comment": "A fishing activity specified in this FA report document."
                },
                {
                    "@id": "cefact:IS_Report.Specified.Fishing_Activity",
                    "@type": "unece:AssociationBIE",
                    "unece:cefactUNId": "UN01012598",
                    "unece:cefactBieDomainClass": "cefact:IS_Report.Details",
                    "rdfs:comment": "A fishing activity specified in this IS report."
                },
                {
                    "@id": "cefact:Sales_Document.Specified.Fishing_Activity",
                    "@type": "unece:AssociationBIE",
                    "unece:cefactUNId": "UN01010917",
                    "unece:cefactBieDomainClass": "cefact:Sales_Document.Details",
                    "rdfs:comment": "A Fishing Activity, such as a landing operation, specified for this sales document."
                }
            ]
        },
        {
            "@id": "fisheries:specifiedAddress",
            "@type": "rdf:Property",
            "schema:rangeIncludes": {
                "@id": "fisheries:Address"
            },
            "schema:domainIncludes": {
                "@id": "fisheries:Party"
            },
            "rdfs:comment": "A structured address specified for this sales party.",
            "rdfs:label": "specifiedAddress",
            "unece:cefactElementMetadata": [
                {
                    "@id": "cefact:Sales_Party.Specified.Structured_Address",
                    "@type": "unece:AssociationBIE",
                    "unece:cefactUNId": "UN01010928",
                    "unece:cefactBieDomainClass": "cefact:Sales_Party.Details",
                    "rdfs:comment": "A structured address specified for this sales party."
                }
            ]
        },
        {
            "@id": "fisheries:specifiedBatch",
            "@type": "rdf:Property",
            "schema:rangeIncludes": {
                "@id": "fisheries:Batch"
            },
            "schema:domainIncludes": {
                "@id": "fisheries:Document"
            },
            "rdfs:comment": "A batch specified for this sales document.",
            "rdfs:label": "specifiedBatch",
            "unece:cefactElementMetadata": [
                {
                    "@id": "cefact:Sales_Document.Specified.Sales_Batch",
                    "@type": "unece:AssociationBIE",
                    "unece:cefactUNId": "UN01010915",
                    "unece:cefactBieDomainClass": "cefact:Sales_Document.Details",
                    "rdfs:comment": "A batch specified for this sales document."
                }
            ]
        },
        {
            "@id": "fisheries:specifiedCatch",
            "@type": "rdf:Property",
            "schema:rangeIncludes": {
                "@id": "fisheries:Catch"
            },
            "schema:domainIncludes": [
                {
                    "@id": "fisheries:Activity"
                },
                {
                    "@id": "fisheries:ReportedArea"
                },
                {
                    "@id": "fisheries:TransportMeans"
                }
            ],
            "rdfs:comment": [
                "A Fishing Activity (FA) catch specified for this fishing activity.",
                "A Fishing Activity (FA) catch specified for this vessel transport means.",
                "A catch specified for this ACDR reported area."
            ],
            "rdfs:label": "specifiedCatch",
            "unece:cefactElementMetadata": [
                {
                    "@id": "cefact:Fishing_Activity.Specified.FA_Catch",
                    "@type": "unece:AssociationBIE",
                    "unece:cefactUNId": "UN01011178",
                    "unece:cefactBieDomainClass": "cefact:Fishing_Activity.Details",
                    "rdfs:comment": "A Fishing Activity (FA) catch specified for this fishing activity."
                },
                {
                    "@id": "cefact:ACDR_ReportedArea.Specified.ACDR_Catch",
                    "@type": "unece:AssociationBIE",
                    "unece:cefactUNId": "UN01010263",
                    "unece:cefactBieDomainClass": "cefact:ACDR_ReportedArea.Details",
                    "rdfs:comment": "A catch specified for this ACDR reported area."
                },
                {
                    "@id": "cefact:Vessel_TransportMeans.Specified.FA_Catch",
                    "@type": "unece:AssociationBIE",
                    "unece:cefactUNId": "UN01012621",
                    "unece:cefactBieDomainClass": "cefact:Vessel_TransportMeans.Details",
                    "rdfs:comment": "A Fishing Activity (FA) catch specified for this vessel transport means."
                }
            ]
        },
        {
            "@id": "fisheries:specifiedCharacteristic",
            "@type": "rdf:Property",
            "schema:rangeIncludes": {
                "@id": "fisheries:Characteristic"
            },
            "schema:domainIncludes": [
                {
                    "@id": "fisheries:Activity"
                },
                {
                    "@id": "fisheries:Document"
                },
                {
                    "@id": "fisheries:Status"
                }
            ],
            "rdfs:comment": [
                "A FLUX characteristic specified for this FA report document.",
                "A Fisheries Language for Universal eXchange (FLUX) characteristic specified for this FLAP document.",
                "A Fisheries Language for Universal eXchange (FLUX) characteristic specified for this fishing activity.",
                "An Inspection or Surveillance Report (ISR) item characteristic specified for this inspected vessel status."
            ],
            "rdfs:label": "specifiedCharacteristic",
            "unece:cefactElementMetadata": [
                {
                    "@id": "cefact:Fishing_Activity.Specified.FLUX_Characteristic",
                    "@type": "unece:AssociationBIE",
                    "unece:cefactUNId": "UN01011181",
                    "unece:cefactBieDomainClass": "cefact:Fishing_Activity.Details",
                    "rdfs:comment": "A Fisheries Language for Universal eXchange (FLUX) characteristic specified for this fishing activity."
                },
                {
                    "@id": "cefact:InspectedVessel_Status.Specified.ISRItem_Characteristic",
                    "@type": "unece:AssociationBIE",
                    "unece:cefactUNId": "UN01013336",
                    "unece:cefactBieDomainClass": "cefact:InspectedVessel_Status.Details",
                    "rdfs:comment": "An Inspection or Surveillance Report (ISR) item characteristic specified for this inspected vessel status."
                },
                {
                    "@id": "cefact:FLAP_Document.Specified.FLUX_Characteristic",
                    "@type": "unece:AssociationBIE",
                    "unece:cefactUNId": "UN01010853",
                    "unece:cefactBieDomainClass": "cefact:FLAP_Document.Details",
                    "rdfs:comment": "A Fisheries Language for Universal eXchange (FLUX) characteristic specified for this FLAP document."
                },
                {
                    "@id": "cefact:FAReport_Document.Specified.FLUX_Characteristic",
                    "@type": "unece:AssociationBIE",
                    "unece:cefactUNId": "UN01013078",
                    "unece:cefactBieDomainClass": "cefact:FAReport_Document.Details",
                    "rdfs:comment": "A FLUX characteristic specified for this FA report document."
                }
            ]
        },
        {
            "@id": "fisheries:specifiedCrew",
            "@type": "rdf:Property",
            "schema:rangeIncludes": {
                "@id": "fisheries:Crew"
            },
            "schema:domainIncludes": [
                {
                    "@id": "fisheries:Document"
                },
                {
                    "@id": "fisheries:TransportMeans"
                }
            ],
            "rdfs:comment": [
                "A vessel crew specified for this FLAP document.",
                "The crew specified for this transport means vessel."
            ],
            "rdfs:label": "specifiedCrew",
            "unece:cefactElementMetadata": [
                {
                    "@id": "cefact:Vessel_TransportMeans.Specified.Vessel_Crew",
                    "@type": "unece:AssociationBIE",
                    "unece:cefactUNId": "UN01010771",
                    "unece:cefactBieDomainClass": "cefact:Vessel_TransportMeans.Details",
                    "rdfs:comment": "The crew specified for this transport means vessel."
                },
                {
                    "@id": "cefact:FLAP_Document.Specified.Vessel_Crew",
                    "@type": "unece:AssociationBIE",
                    "unece:cefactUNId": "UN01010854",
                    "unece:cefactBieDomainClass": "cefact:FLAP_Document.Details",
                    "rdfs:comment": "A vessel crew specified for this FLAP document."
                }
            ]
        },
        {
            "@id": "fisheries:specifiedDimension",
            "@type": "rdf:Property",
            "schema:rangeIncludes": {
                "@id": "fisheries:Dimension"
            },
            "schema:domainIncludes": {
                "@id": "fisheries:TransportMeans"
            },
            "rdfs:comment": "A dimension specified for this transport means vessel.",
            "rdfs:label": "specifiedDimension",
            "unece:cefactElementMetadata": [
                {
                    "@id": "cefact:Vessel_TransportMeans.Specified.Vessel_Dimension",
                    "@type": "unece:AssociationBIE",
                    "unece:cefactUNId": "UN01010644",
                    "unece:cefactBieDomainClass": "cefact:Vessel_TransportMeans.Details",
                    "rdfs:comment": "A dimension specified for this transport means vessel."
                }
            ]
        },
        {
            "@id": "fisheries:specifiedDistribution",
            "@type": "rdf:Property",
            "schema:rangeIncludes": {
                "@id": "fisheries:Distribution"
            },
            "schema:domainIncludes": [
                {
                    "@id": "fisheries:Catch"
                },
                {
                    "@id": "fisheries:Product"
                }
            ],
            "rdfs:comment": [
                "The size distribution specified for this AAP product.",
                "The size distribution specified for this FA catch."
            ],
            "rdfs:label": "specifiedDistribution",
            "unece:cefactElementMetadata": [
                {
                    "@id": "cefact:AAP_Product.Specified.Size_Distribution",
                    "@type": "unece:AssociationBIE",
                    "unece:cefactUNId": "UN01011146",
                    "unece:cefactBieDomainClass": "cefact:AAP_Product.Details",
                    "rdfs:comment": "The size distribution specified for this AAP product."
                },
                {
                    "@id": "cefact:FA_Catch.Specified.Size_Distribution",
                    "@type": "unece:AssociationBIE",
                    "unece:cefactUNId": "UN01011192",
                    "unece:cefactBieDomainClass": "cefact:FA_Catch.Details",
                    "rdfs:comment": "The size distribution specified for this FA catch."
                }
            ]
        },
        {
            "@id": "fisheries:specifiedDocument",
            "@type": "rdf:Property",
            "schema:rangeIncludes": {
                "@id": "fisheries:Document"
            },
            "schema:domainIncludes": {
                "@id": "fisheries:Activity"
            },
            "rdfs:comment": "A Fishing Licence, Authorization or Permit (FLAP) document specified for this fishing activity.",
            "rdfs:label": "specifiedDocument",
            "unece:cefactElementMetadata": [
                {
                    "@id": "cefact:Fishing_Activity.Specified.FLAP_Document",
                    "@type": "unece:AssociationBIE",
                    "unece:cefactUNId": "UN01011186",
                    "unece:cefactBieDomainClass": "cefact:Fishing_Activity.Details",
                    "rdfs:comment": "A Fishing Licence, Authorization or Permit (FLAP) document specified for this fishing activity."
                }
            ]
        },
        {
            "@id": "fisheries:specifiedEvent",
            "@type": "rdf:Property",
            "schema:rangeIncludes": {
                "@id": "fisheries:Event"
            },
            "schema:domainIncludes": [
                {
                    "@id": "fisheries:Document"
                },
                {
                    "@id": "fisheries:Report"
                },
                {
                    "@id": "fisheries:TransportMeans"
                }
            ],
            "rdfs:comment": [
                "A position event specified for this vessel transport means.",
                "A registration event specified for this vessel transport means.",
                "An event specified for this sales document.",
                "The construction event specified for this vessel transport means.",
                "The inspection or surveillance event specified in this IS report."
            ],
            "rdfs:label": "specifiedEvent",
            "unece:cefactElementMetadata": [
                {
                    "@id": "cefact:Vessel_TransportMeans.Specified.Registration_Event",
                    "@type": "unece:AssociationBIE",
                    "unece:cefactUNId": "UN01010641",
                    "unece:cefactBieDomainClass": "cefact:Vessel_TransportMeans.Details",
                    "rdfs:comment": "A registration event specified for this vessel transport means."
                },
                {
                    "@id": "cefact:Vessel_TransportMeans.Specified.Construction_Event",
                    "@type": "unece:AssociationBIE",
                    "unece:cefactUNId": "UN01010642",
                    "unece:cefactBieDomainClass": "cefact:Vessel_TransportMeans.Details",
                    "rdfs:comment": "The construction event specified for this vessel transport means."
                },
                {
                    "@id": "cefact:IS_Report.Specified.IS_Event",
                    "@type": "unece:AssociationBIE",
                    "unece:cefactUNId": "UN01012592",
                    "unece:cefactBieDomainClass": "cefact:IS_Report.Details",
                    "rdfs:comment": "The inspection or surveillance event specified in this IS report."
                },
                {
                    "@id": "cefact:Vessel_TransportMeans.Specified.VesselPosition_Event",
                    "@type": "unece:AssociationBIE",
                    "unece:cefactUNId": "UN01010230",
                    "unece:cefactBieDomainClass": "cefact:Vessel_TransportMeans.Details",
                    "rdfs:comment": "A position event specified for this vessel transport means."
                },
                {
                    "@id": "cefact:Sales_Document.Specified.Sales_Event",
                    "@type": "unece:AssociationBIE",
                    "unece:cefactUNId": "UN01010916",
                    "unece:cefactBieDomainClass": "cefact:Sales_Document.Details",
                    "rdfs:comment": "An event specified for this sales document."
                }
            ]
        },
        {
            "@id": "fisheries:specifiedGear",
            "@type": "rdf:Property",
            "schema:rangeIncludes": {
                "@id": "fisheries:Gear"
            },
            "schema:domainIncludes": {
                "@id": "fisheries:Activity"
            },
            "rdfs:comment": "A fishing gear specified for this fishing activity.",
            "rdfs:label": "specifiedGear",
            "unece:cefactElementMetadata": [
                {
                    "@id": "cefact:Fishing_Activity.Specified.Fishing_Gear",
                    "@type": "unece:AssociationBIE",
                    "unece:cefactUNId": "UN01011182",
                    "unece:cefactBieDomainClass": "cefact:Fishing_Activity.Details",
                    "rdfs:comment": "A fishing gear specified for this fishing activity."
                }
            ]
        },
        {
            "@id": "fisheries:specifiedGeographicalCoordinate",
            "@type": "rdf:Property",
            "schema:rangeIncludes": {
                "@id": "fisheries:GeographicalCoordinate"
            },
            "schema:domainIncludes": [
                {
                    "@id": "fisheries:Event"
                },
                {
                    "@id": "fisheries:LinearRing"
                }
            ],
            "rdfs:comment": [
                "Geographical coordinate information specified for this linear ring.",
                "The set of geographical coordinates specified for this vessel position event."
            ],
            "rdfs:label": "specifiedGeographicalCoordinate",
            "unece:cefactElementMetadata": [
                {
                    "@id": "cefact:Specified_LinearRing.Specified.FLUX_GeographicalCoordinate",
                    "@type": "unece:AssociationBIE",
                    "unece:cefactUNId": "UN01011207",
                    "unece:cefactBieDomainClass": "cefact:Specified_LinearRing.Details",
                    "rdfs:comment": "Geographical coordinate information specified for this linear ring."
                },
                {
                    "@id": "cefact:VesselPosition_Event.Specified.Vessel_GeographicalCoordinate",
                    "@type": "unece:AssociationBIE",
                    "unece:cefactUNId": "UN01010226",
                    "unece:cefactBieDomainClass": "cefact:VesselPosition_Event.Details",
                    "rdfs:comment": "The set of geographical coordinates specified for this vessel position event."
                }
            ]
        },
        {
            "@id": "fisheries:specifiedLocation",
            "@type": "rdf:Property",
            "schema:rangeIncludes": {
                "@id": "fisheries:Location"
            },
            "schema:domainIncludes": [
                {
                    "@id": "fisheries:Catch"
                },
                {
                    "@id": "fisheries:Characteristic"
                },
                {
                    "@id": "fisheries:Document"
                },
                {
                    "@id": "fisheries:Means"
                },
                {
                    "@id": "fisheries:Problem"
                },
                {
                    "@id": "fisheries:Query"
                },
                {
                    "@id": "fisheries:Report"
                },
                {
                    "@id": "fisheries:TransportMeans"
                }
            ],
            "rdfs:comment": [
                "A FLUX location specified for this FLUX characteristic.",
                "A FLUX location specified for this gear characteristic.",
                "A Fisheries Language Universal eXchange (FLUX) location specified for this ISR item characteristic.",
                "A Fisheries Language Universal eXchange (FLUX) location specified for this surveillance means.",
                "A Fisheries Language Universal eXchange (FLUX) location specified for this vessel transport means.",
                "A Fisheries Language Universal eXchange (FLUX) location specified in this IS report.",
                "A Fisheries Language for Universal eXchange (FLUX) location specified for this FA catch.",
                "A Fisheries Language for Universal eXchange (FLUX) location specified for this FLAP document.",
                "A Fisheries Language for Universal eXchange (FLUX) location specified for this gear problem.",
                "A Fisheries Language for Universal eXchange (FLUX) location specified for this sales document.",
                "A Fisheries Language for Universal eXchange (FLUX) location specified in this vessel position query."
            ],
            "rdfs:label": "specifiedLocation",
            "unece:cefactElementMetadata": [
                {
                    "@id": "cefact:Surveillance_Means.Specified.FLUX_Location",
                    "@type": "unece:AssociationBIE",
                    "unece:cefactUNId": "UN01012632",
                    "unece:cefactBieDomainClass": "cefact:Surveillance_Means.Details",
                    "rdfs:comment": "A Fisheries Language Universal eXchange (FLUX) location specified for this surveillance means."
                },
                {
                    "@id": "cefact:Gear_Characteristic.Specified.FLUX_Location",
                    "@type": "unece:AssociationBIE",
                    "unece:cefactUNId": "UN01012112",
                    "unece:cefactBieDomainClass": "cefact:Gear_Characteristic.Details",
                    "rdfs:comment": "A FLUX location specified for this gear characteristic."
                },
                {
                    "@id": "cefact:IS_Report.Specified.FLUX_Location",
                    "@type": "unece:AssociationBIE",
                    "unece:cefactUNId": "UN01012599",
                    "unece:cefactBieDomainClass": "cefact:IS_Report.Details",
                    "rdfs:comment": "A Fisheries Language Universal eXchange (FLUX) location specified in this IS report."
                },
                {
                    "@id": "cefact:FLAP_Document.Specified.FLUX_Location",
                    "@type": "unece:AssociationBIE",
                    "unece:cefactUNId": "UN01010861",
                    "unece:cefactBieDomainClass": "cefact:FLAP_Document.Details",
                    "rdfs:comment": "A Fisheries Language for Universal eXchange (FLUX) location specified for this FLAP document."
                },
                {
                    "@id": "cefact:VesselPosition_Query.Specified.FLUX_Location",
                    "@type": "unece:AssociationBIE",
                    "unece:cefactUNId": "UN01012652",
                    "unece:cefactBieDomainClass": "cefact:VesselPosition_Query.Details",
                    "rdfs:comment": "A Fisheries Language for Universal eXchange (FLUX) location specified in this vessel position query."
                },
                {
                    "@id": "cefact:Vessel_TransportMeans.Specified.FLUX_Location",
                    "@type": "unece:AssociationBIE",
                    "unece:cefactUNId": "UN01012620",
                    "unece:cefactBieDomainClass": "cefact:Vessel_TransportMeans.Details",
                    "rdfs:comment": "A Fisheries Language Universal eXchange (FLUX) location specified for this vessel transport means."
                },
                {
                    "@id": "cefact:FA_Catch.Specified.FLUX_Location",
                    "@type": "unece:AssociationBIE",
                    "unece:cefactUNId": "UN01011196",
                    "unece:cefactBieDomainClass": "cefact:FA_Catch.Details",
                    "rdfs:comment": "A Fisheries Language for Universal eXchange (FLUX) location specified for this FA catch."
                },
                {
                    "@id": "cefact:ISRItem_Characteristic.Specified.FLUX_Location",
                    "@type": "unece:AssociationBIE",
                    "unece:cefactUNId": "UN01012612",
                    "unece:cefactBieDomainClass": "cefact:ISRItem_Characteristic.Details",
                    "rdfs:comment": "A Fisheries Language Universal eXchange (FLUX) location specified for this ISR item characteristic."
                },
                {
                    "@id": "cefact:Gear_Problem.Specified.FLUX_Location",
                    "@type": "unece:AssociationBIE",
                    "unece:cefactUNId": "UN01011212",
                    "unece:cefactBieDomainClass": "cefact:Gear_Problem.Details",
                    "rdfs:comment": "A Fisheries Language for Universal eXchange (FLUX) location specified for this gear problem."
                },
                {
                    "@id": "cefact:FLUX_Characteristic.Specified.FLUX_Location",
                    "@type": "unece:AssociationBIE",
                    "unece:cefactUNId": "UN01012111",
                    "unece:cefactBieDomainClass": "cefact:FLUX_Characteristic.Details",
                    "rdfs:comment": "A FLUX location specified for this FLUX characteristic."
                },
                {
                    "@id": "cefact:Sales_Document.Specified.FLUX_Location",
                    "@type": "unece:AssociationBIE",
                    "unece:cefactUNId": "UN01010918",
                    "unece:cefactBieDomainClass": "cefact:Sales_Document.Details",
                    "rdfs:comment": "A Fisheries Language for Universal eXchange (FLUX) location specified for this sales document."
                }
            ]
        },
        {
            "@id": "fisheries:specifiedMeans",
            "@type": "rdf:Property",
            "schema:rangeIncludes": {
                "@id": "fisheries:Means"
            },
            "schema:domainIncludes": {
                "@id": "fisheries:Report"
            },
            "rdfs:comment": "A means of surveillance specified in this IS report.",
            "rdfs:label": "specifiedMeans",
            "unece:cefactElementMetadata": [
                {
                    "@id": "cefact:IS_Report.Specified.Surveillance_Means",
                    "@type": "unece:AssociationBIE",
                    "unece:cefactUNId": "UN01012601",
                    "unece:cefactBieDomainClass": "cefact:IS_Report.Details",
                    "rdfs:comment": "A means of surveillance specified in this IS report."
                }
            ]
        },
        {
            "@id": "fisheries:specifiedOrganization",
            "@type": "rdf:Property",
            "schema:rangeIncludes": {
                "@id": "fisheries:Organization"
            },
            "schema:domainIncludes": {
                "@id": "fisheries:Party"
            },
            "rdfs:comment": "The Fisheries Language for Universal eXchange (FLUX) organization specified for this sales party.",
            "rdfs:label": "specifiedOrganization",
            "unece:cefactElementMetadata": [
                {
                    "@id": "cefact:Sales_Party.Specified.FLUX_Organization",
                    "@type": "unece:AssociationBIE",
                    "unece:cefactUNId": "UN01011155",
                    "unece:cefactBieDomainClass": "cefact:Sales_Party.Details",
                    "rdfs:comment": "The Fisheries Language for Universal eXchange (FLUX) organization specified for this sales party."
                }
            ]
        },
        {
            "@id": "fisheries:specifiedParty",
            "@type": "rdf:Property",
            "schema:rangeIncludes": {
                "@id": "fisheries:Party"
            },
            "schema:domainIncludes": [
                {
                    "@id": "fisheries:Document"
                },
                {
                    "@id": "fisheries:Report"
                },
                {
                    "@id": "fisheries:TransportCharter"
                },
                {
                    "@id": "fisheries:TransportMeans"
                }
            ],
            "rdfs:comment": [
                "A contact party specified for this FLAP document.",
                "A contact party specified for this transport means vessel.",
                "A contact party specified for this vehicle transport means.",
                "A contact party specified for this vessel transport charter.",
                "A contact party specified in this IS report.",
                "A sales party specified in this sales document."
            ],
            "rdfs:label": "specifiedParty",
            "unece:cefactElementMetadata": [
                {
                    "@id": "cefact:Vehicle_TransportMeans.Specified.Contact_Party",
                    "@type": "unece:AssociationBIE",
                    "unece:cefactUNId": "UN01012661",
                    "unece:cefactBieDomainClass": "cefact:Vehicle_TransportMeans.Details",
                    "rdfs:comment": "A contact party specified for this vehicle transport means."
                },
                {
                    "@id": "cefact:IS_Report.Specified.Contact_Party",
                    "@type": "unece:AssociationBIE",
                    "unece:cefactUNId": "UN01012595",
                    "unece:cefactBieDomainClass": "cefact:IS_Report.Details",
                    "rdfs:comment": "A contact party specified in this IS report."
                },
                {
                    "@id": "cefact:FLAP_Document.Specified.Contact_Party",
                    "@type": "unece:AssociationBIE",
                    "unece:cefactUNId": "UN01010858",
                    "unece:cefactBieDomainClass": "cefact:FLAP_Document.Details",
                    "rdfs:comment": "A contact party specified for this FLAP document."
                },
                {
                    "@id": "cefact:Vessel_TransportCharter.Specified.Contact_Party",
                    "@type": "unece:AssociationBIE",
                    "unece:cefactUNId": "UN01010877",
                    "unece:cefactBieDomainClass": "cefact:Vessel_TransportCharter.Details",
                    "rdfs:comment": "A contact party specified for this vessel transport charter."
                },
                {
                    "@id": "cefact:Vessel_TransportMeans.Specified.Contact_Party",
                    "@type": "unece:AssociationBIE",
                    "unece:cefactUNId": "UN01010649",
                    "unece:cefactBieDomainClass": "cefact:Vessel_TransportMeans.Details",
                    "rdfs:comment": "A contact party specified for this transport means vessel."
                },
                {
                    "@id": "cefact:Sales_Document.Specified.Sales_Party",
                    "@type": "unece:AssociationBIE",
                    "unece:cefactUNId": "UN01010919",
                    "unece:cefactBieDomainClass": "cefact:Sales_Document.Details",
                    "rdfs:comment": "A sales party specified in this sales document."
                }
            ]
        },
        {
            "@id": "fisheries:specifiedPeriod",
            "@type": "rdf:Property",
            "schema:rangeIncludes": {
                "@id": "fisheries:Period"
            },
            "schema:domainIncludes": [
                {
                    "@id": "fisheries:Activity"
                },
                {
                    "@id": "fisheries:Catch"
                },
                {
                    "@id": "fisheries:Query"
                },
                {
                    "@id": "fisheries:Trip"
                }
            ],
            "rdfs:comment": [
                "A delimited period specified for this FA catch.",
                "A delimited period specified for this fishing activity.",
                "A delimited period specified for this fishing trip.",
                "The delimited period specified for this FA query.",
                "The delimited period specified for this FLAP query.",
                "The delimited period specified for this ISR query.",
                "The delimited period specified for this sales query.",
                "The delimited period specified for this vessel position query.",
                "The delimited period specified for this vessel query."
            ],
            "rdfs:label": "specifiedPeriod",
            "unece:cefactElementMetadata": [
                {
                    "@id": "cefact:Fishing_Trip.Specified.Delimited_Period",
                    "@type": "unece:AssociationBIE",
                    "unece:cefactUNId": "UN01011167",
                    "unece:cefactBieDomainClass": "cefact:Fishing_Trip.Details",
                    "rdfs:comment": "A delimited period specified for this fishing trip."
                },
                {
                    "@id": "cefact:ISR_Query.Specified.Delimited_Period",
                    "@type": "unece:AssociationBIE",
                    "unece:cefactUNId": "UN01012639",
                    "unece:cefactBieDomainClass": "cefact:ISR_Query.Details",
                    "rdfs:comment": "The delimited period specified for this ISR query."
                },
                {
                    "@id": "cefact:FA_Query.Specified.Delimited_Period",
                    "@type": "unece:AssociationBIE",
                    "unece:cefactUNId": "UN01011221",
                    "unece:cefactBieDomainClass": "cefact:FA_Query.Details",
                    "rdfs:comment": "The delimited period specified for this FA query."
                },
                {
                    "@id": "cefact:Sales_Query.Specified.Delimited_Period",
                    "@type": "unece:AssociationBIE",
                    "unece:cefactUNId": "UN01010997",
                    "unece:cefactBieDomainClass": "cefact:Sales_Query.Details",
                    "rdfs:comment": "The delimited period specified for this sales query."
                },
                {
                    "@id": "cefact:FLAP_Query.Specified.Delimited_Period",
                    "@type": "unece:AssociationBIE",
                    "unece:cefactUNId": "UN01010890",
                    "unece:cefactBieDomainClass": "cefact:FLAP_Query.Details",
                    "rdfs:comment": "The delimited period specified for this FLAP query."
                },
                {
                    "@id": "cefact:FA_Catch.Specified.Delimited_Period",
                    "@type": "unece:AssociationBIE",
                    "unece:cefactUNId": "UN01012633",
                    "unece:cefactBieDomainClass": "cefact:FA_Catch.Details",
                    "rdfs:comment": "A delimited period specified for this FA catch."
                },
                {
                    "@id": "cefact:Vessel_Query.Specified.Delimited_Period",
                    "@type": "unece:AssociationBIE",
                    "unece:cefactUNId": "UN01010828",
                    "unece:cefactBieDomainClass": "cefact:Vessel_Query.Details",
                    "rdfs:comment": "The delimited period specified for this vessel query."
                },
                {
                    "@id": "cefact:Fishing_Activity.Specified.Delimited_Period",
                    "@type": "unece:AssociationBIE",
                    "unece:cefactUNId": "UN01011187",
                    "unece:cefactBieDomainClass": "cefact:Fishing_Activity.Details",
                    "rdfs:comment": "A delimited period specified for this fishing activity."
                },
                {
                    "@id": "cefact:VesselPosition_Query.Specified.Delimited_Period",
                    "@type": "unece:AssociationBIE",
                    "unece:cefactUNId": "UN01012651",
                    "unece:cefactBieDomainClass": "cefact:VesselPosition_Query.Details",
                    "rdfs:comment": "The delimited period specified for this vessel position query."
                }
            ]
        },
        {
            "@id": "fisheries:specifiedPerson",
            "@type": "rdf:Property",
            "schema:rangeIncludes": {
                "@id": "fisheries:Person"
            },
            "schema:domainIncludes": {
                "@id": "fisheries:Party"
            },
            "rdfs:comment": "A specified person for this contact party.",
            "rdfs:label": "specifiedPerson",
            "unece:cefactElementMetadata": [
                {
                    "@id": "cefact:Contact_Party.Specified.Contact_Person",
                    "@type": "unece:AssociationBIE",
                    "unece:cefactUNId": "UN01010785",
                    "unece:cefactBieDomainClass": "cefact:Contact_Party.Details",
                    "rdfs:comment": "A specified person for this contact party."
                }
            ]
        },
        {
            "@id": "fisheries:specifiedPhysicalGeographicalCoordinate",
            "@type": "rdf:Property",
            "schema:rangeIncludes": {
                "@id": "fisheries:GeographicalCoordinate"
            },
            "schema:domainIncludes": {
                "@id": "fisheries:Location"
            },
            "rdfs:comment": "Geographical coordinate information specified for this FLUX location.",
            "rdfs:label": "specifiedPhysicalGeographicalCoordinate",
            "unece:cefactElementMetadata": [
                {
                    "@id": "cefact:FLUX_Location.Specified_Physical.FLUX_GeographicalCoordinate",
                    "@type": "unece:AssociationBIE",
                    "unece:cefactUNId": "UN01010964",
                    "unece:cefactBieDomainClass": "cefact:FLUX_Location.Details",
                    "rdfs:comment": "Geographical coordinate information specified for this FLUX location."
                }
            ]
        },
        {
            "@id": "fisheries:specifiedProblem",
            "@type": "rdf:Property",
            "schema:rangeIncludes": {
                "@id": "fisheries:Problem"
            },
            "schema:domainIncludes": {
                "@id": "fisheries:Activity"
            },
            "rdfs:comment": "A gear problem specified for this fishing activity.",
            "rdfs:label": "specifiedProblem",
            "unece:cefactElementMetadata": [
                {
                    "@id": "cefact:Fishing_Activity.Specified.Gear_Problem",
                    "@type": "unece:AssociationBIE",
                    "unece:cefactUNId": "UN01011180",
                    "unece:cefactBieDomainClass": "cefact:Fishing_Activity.Details",
                    "rdfs:comment": "A gear problem specified for this fishing activity."
                }
            ]
        },
        {
            "@id": "fisheries:specifiedProduct",
            "@type": "rdf:Property",
            "schema:rangeIncludes": {
                "@id": "fisheries:Product"
            },
            "schema:domainIncludes": {
                "@id": "fisheries:Batch"
            },
            "rdfs:comment": "An Aquatic Animals & Plants (AAP) product specified for this sales batch.",
            "rdfs:label": "specifiedProduct",
            "unece:cefactElementMetadata": [
                {
                    "@id": "cefact:Sales_Batch.Specified.AAP_Product",
                    "@type": "unece:AssociationBIE",
                    "unece:cefactUNId": "UN01010931",
                    "unece:cefactBieDomainClass": "cefact:Sales_Batch.Details",
                    "rdfs:comment": "An Aquatic Animals & Plants (AAP) product specified for this sales batch."
                }
            ]
        },
        {
            "@id": "fisheries:specifiedQuantity",
            "@type": "rdf:Property",
            "schema:rangeIncludes": {
                "@id": "xsd:decimal"
            },
            "schema:domainIncludes": {
                "@id": "fisheries:Quota"
            },
            "rdfs:comment": "A specified quantity for this targeted quota.",
            "rdfs:label": "specifiedQuantity",
            "unece:cefactElementMetadata": [
                {
                    "@id": "cefact:Targeted_Quota.Specified.Quantity",
                    "@type": "unece:BasicBIE",
                    "unece:cefactUNId": "UN01010882",
                    "unece:cefactBieDomainClass": "cefact:Targeted_Quota.Details",
                    "rdfs:comment": "A specified quantity for this targeted quota."
                }
            ]
        },
        {
            "@id": "fisheries:specifiedQuota",
            "@type": "rdf:Property",
            "schema:rangeIncludes": {
                "@id": "fisheries:Quota"
            },
            "schema:domainIncludes": {
                "@id": "fisheries:Document"
            },
            "rdfs:comment": "A targeted quota specified in this FLAP document.",
            "rdfs:label": "specifiedQuota",
            "unece:cefactElementMetadata": [
                {
                    "@id": "cefact:FLAP_Document.Specified.Targeted_Quota",
                    "@type": "unece:AssociationBIE",
                    "unece:cefactUNId": "UN01010859",
                    "unece:cefactBieDomainClass": "cefact:FLAP_Document.Details",
                    "rdfs:comment": "A targeted quota specified in this FLAP document."
                }
            ]
        },
        {
            "@id": "fisheries:specifiedReportedArea",
            "@type": "rdf:Property",
            "schema:rangeIncludes": {
                "@id": "fisheries:ReportedArea"
            },
            "schema:domainIncludes": {
                "@id": "fisheries:ACDRReport"
            },
            "rdfs:comment": "A reported area specified in this FLUX ACDR report.",
            "rdfs:label": "specifiedReportedArea",
            "unece:cefactElementMetadata": [
                {
                    "@id": "cefact:FLUX_ACDRReport.Specified.ACDR_ReportedArea",
                    "@type": "unece:AssociationBIE",
                    "unece:cefactUNId": "UN01010275",
                    "unece:cefactBieDomainClass": "cefact:FLUX_ACDRReport.Details",
                    "rdfs:comment": "A reported area specified in this FLUX ACDR report."
                }
            ]
        },
        {
            "@id": "fisheries:specifiedStatus",
            "@type": "rdf:Property",
            "schema:rangeIncludes": {
                "@id": "fisheries:Status"
            },
            "schema:domainIncludes": [
                {
                    "@id": "fisheries:Document"
                },
                {
                    "@id": "fisheries:Report"
                }
            ],
            "rdfs:comment": [
                "A specified inspected vessel status in this IS report.",
                "An authorization status specified for this FLAP document."
            ],
            "rdfs:label": "specifiedStatus",
            "unece:cefactElementMetadata": [
                {
                    "@id": "cefact:FLAP_Document.Specified.Authorization_Status",
                    "@type": "unece:AssociationBIE",
                    "unece:cefactUNId": "UN01010864",
                    "unece:cefactBieDomainClass": "cefact:FLAP_Document.Details",
                    "rdfs:comment": "An authorization status specified for this FLAP document."
                },
                {
                    "@id": "cefact:IS_Report.Specified.InspectedVessel_Status",
                    "@type": "unece:AssociationBIE",
                    "unece:cefactUNId": "UN01013406",
                    "unece:cefactBieDomainClass": "cefact:IS_Report.Details",
                    "rdfs:comment": "A specified inspected vessel status in this IS report."
                }
            ]
        },
        {
            "@id": "fisheries:specifiedSuspicion",
            "@type": "rdf:Property",
            "schema:rangeIncludes": {
                "@id": "fisheries:Suspicion"
            },
            "schema:domainIncludes": {
                "@id": "fisheries:Report"
            },
            "rdfs:comment": "An Inspection or Surveillance Report (ISR) Infringement suspicion specified in this IS report.",
            "rdfs:label": "specifiedSuspicion",
            "unece:cefactElementMetadata": [
                {
                    "@id": "cefact:IS_Report.Specified.ISRInfringement_Suspicion",
                    "@type": "unece:AssociationBIE",
                    "unece:cefactUNId": "UN01013328",
                    "unece:cefactBieDomainClass": "cefact:IS_Report.Details",
                    "rdfs:comment": "An Inspection or Surveillance Report (ISR) Infringement suspicion specified in this IS report."
                }
            ]
        },
        {
            "@id": "fisheries:specifiedTransportCharter",
            "@type": "rdf:Property",
            "schema:rangeIncludes": {
                "@id": "fisheries:TransportCharter"
            },
            "schema:domainIncludes": {
                "@id": "fisheries:Document"
            },
            "rdfs:comment": "A vessel transport charter specified for this FLAP document.",
            "rdfs:label": "specifiedTransportCharter",
            "unece:cefactElementMetadata": [
                {
                    "@id": "cefact:FLAP_Document.Specified.Vessel_TransportCharter",
                    "@type": "unece:AssociationBIE",
                    "unece:cefactUNId": "UN01010857",
                    "unece:cefactBieDomainClass": "cefact:FLAP_Document.Details",
                    "rdfs:comment": "A vessel transport charter specified for this FLAP document."
                }
            ]
        },
        {
            "@id": "fisheries:specifiedTransportMeans",
            "@type": "rdf:Property",
            "schema:rangeIncludes": {
                "@id": "fisheries:TransportMeans"
            },
            "schema:domainIncludes": [
                {
                    "@id": "fisheries:ACDRReport"
                },
                {
                    "@id": "fisheries:Document"
                },
                {
                    "@id": "fisheries:Report"
                }
            ],
            "rdfs:comment": [
                "A vehicle transport means specified in this IS report.",
                "A vessel transport means specified in this FLAP document.",
                "A vessel transport means specified in this IS report.",
                "The vehicle transport means specified in this sales document.",
                "The vessel transport means specified for this FA report document.",
                "The vessel transport means specified in this FLUX ACDR report."
            ],
            "rdfs:label": "specifiedTransportMeans",
            "unece:cefactElementMetadata": [
                {
                    "@id": "cefact:IS_Report.Specified.Vehicle_TransportMeans",
                    "@type": "unece:AssociationBIE",
                    "unece:cefactUNId": "UN01012594",
                    "unece:cefactBieDomainClass": "cefact:IS_Report.Details",
                    "rdfs:comment": "A vehicle transport means specified in this IS report."
                },
                {
                    "@id": "cefact:Sales_Document.Specified.Vehicle_TransportMeans",
                    "@type": "unece:AssociationBIE",
                    "unece:cefactUNId": "UN01010920",
                    "unece:cefactBieDomainClass": "cefact:Sales_Document.Details",
                    "rdfs:comment": "The vehicle transport means specified in this sales document."
                },
                {
                    "@id": "cefact:FLUX_ACDRReport.Specified.Vessel_TransportMeans",
                    "@type": "unece:AssociationBIE",
                    "unece:cefactUNId": "UN01010274",
                    "unece:cefactBieDomainClass": "cefact:FLUX_ACDRReport.Details",
                    "rdfs:comment": "The vessel transport means specified in this FLUX ACDR report."
                },
                {
                    "@id": "cefact:FLAP_Document.Specified.Vessel_TransportMeans",
                    "@type": "unece:AssociationBIE",
                    "unece:cefactUNId": "UN01012654",
                    "unece:cefactBieDomainClass": "cefact:FLAP_Document.Details",
                    "rdfs:comment": "A vessel transport means specified in this FLAP document."
                },
                {
                    "@id": "cefact:IS_Report.Specified.Vessel_TransportMeans",
                    "@type": "unece:AssociationBIE",
                    "unece:cefactUNId": "UN01012593",
                    "unece:cefactBieDomainClass": "cefact:IS_Report.Details",
                    "rdfs:comment": "A vessel transport means specified in this IS report."
                },
                {
                    "@id": "cefact:FAReport_Document.Specified.Vessel_TransportMeans",
                    "@type": "unece:AssociationBIE",
                    "unece:cefactUNId": "UN01011163",
                    "unece:cefactBieDomainClass": "cefact:FAReport_Document.Details",
                    "rdfs:comment": "The vessel transport means specified for this FA report document."
                }
            ]
        },
        {
            "@id": "fisheries:specifiedTrip",
            "@type": "rdf:Property",
            "schema:rangeIncludes": {
                "@id": "fisheries:Trip"
            },
            "schema:domainIncludes": {
                "@id": "fisheries:Activity"
            },
            "rdfs:comment": "The fishing trip specified for this fishing activity.",
            "rdfs:label": "specifiedTrip",
            "unece:cefactElementMetadata": [
                {
                    "@id": "cefact:Fishing_Activity.Specified.Fishing_Trip",
                    "@type": "unece:AssociationBIE",
                    "unece:cefactUNId": "UN01011188",
                    "unece:cefactBieDomainClass": "cefact:Fishing_Activity.Details",
                    "rdfs:comment": "The fishing trip specified for this fishing activity."
                }
            ]
        },
        {
            "@id": "fisheries:specifiedVersion",
            "@type": "rdf:Property",
            "schema:rangeIncludes": {
                "@id": "fisheries:Version"
            },
            "schema:domainIncludes": {
                "@id": "fisheries:DataSet"
            },
            "rdfs:comment": "A version specified for this MDR data set.",
            "rdfs:label": "specifiedVersion",
            "unece:cefactElementMetadata": [
                {
                    "@id": "cefact:MDR_DataSet.Specified.DataSet_Version",
                    "@type": "unece:AssociationBIE",
                    "unece:cefactUNId": "UN01010587",
                    "unece:cefactBieDomainClass": "cefact:MDR_DataSet.Details",
                    "rdfs:comment": "A version specified for this MDR data set."
                }
            ]
        },
        {
            "@id": "fisheries:speedMeasure",
            "@type": "rdf:Property",
            "schema:rangeIncludes": {
                "@id": "xsd:decimal"
            },
            "schema:domainIncludes": {
                "@id": "fisheries:TransportMeans"
            },
            "rdfs:comment": "The speed measured for this transport means vessel.",
            "rdfs:label": "speedMeasure",
            "unece:cefactElementMetadata": [
                {
                    "@id": "cefact:Vessel_TransportMeans.Speed.Measure",
                    "@type": "unece:BasicBIE",
                    "unece:cefactUNId": "UN01010769",
                    "unece:cefactBieDomainClass": "cefact:Vessel_TransportMeans.Details",
                    "rdfs:comment": "The speed measured for this transport means vessel."
                }
            ]
        },
        {
            "@id": "fisheries:speedValueMeasure",
            "@type": "rdf:Property",
            "schema:rangeIncludes": {
                "@id": "xsd:decimal"
            },
            "schema:domainIncludes": {
                "@id": "fisheries:Event"
            },
            "rdfs:comment": "The measure of speed of the vessel for this vessel position event.",
            "rdfs:label": "speedValueMeasure",
            "unece:cefactElementMetadata": [
                {
                    "@id": "cefact:VesselPosition_Event.Speed_Value.Measure",
                    "@type": "unece:BasicBIE",
                    "unece:cefactUNId": "UN01010236",
                    "unece:cefactBieDomainClass": "cefact:VesselPosition_Event.Details",
                    "rdfs:comment": "The measure of speed of the vessel for this vessel position event."
                }
            ]
        },
        {
            "@id": "fisheries:statusCode",
            "@type": "rdf:Property",
            "schema:rangeIncludes": {
                "@id": "xsd:token"
            },
            "schema:domainIncludes": {
                "@id": "fisheries:Identity"
            },
            "rdfs:comment": "A code specifying the status of this FLAP identity.",
            "rdfs:label": "statusCode",
            "unece:cefactElementMetadata": [
                {
                    "@id": "cefact:FLAP_Identity.Status.Code",
                    "@type": "unece:BasicBIE",
                    "unece:cefactUNId": "UN01010899",
                    "unece:cefactBieDomainClass": "cefact:FLAP_Identity.Details",
                    "rdfs:comment": "A code specifying the status of this FLAP identity."
                }
            ]
        },
        {
            "@id": "fisheries:subjectIdentity",
            "@type": "rdf:Property",
            "schema:rangeIncludes": {
                "@id": "fisheries:Identity"
            },
            "schema:domainIncludes": {
                "@id": "fisheries:Query"
            },
            "rdfs:comment": [
                "A vessel identity of a subject of this FLAP query.",
                "An identity of a subject of this FLAP query.",
                "The identity of a subject of this MDR query.",
                "The identity of a subject of this vessel query.",
                "The vessel identity as the subject of this vessel position query."
            ],
            "rdfs:label": "subjectIdentity",
            "unece:cefactElementMetadata": [
                {
                    "@id": "cefact:VesselPosition_Query.Subject.Vessel_Identity",
                    "@type": "unece:AssociationBIE",
                    "unece:cefactUNId": "UN01012653",
                    "unece:cefactBieDomainClass": "cefact:VesselPosition_Query.Details",
                    "rdfs:comment": "The vessel identity as the subject of this vessel position query."
                },
                {
                    "@id": "cefact:FLAP_Query.Subject.Vessel_Identity",
                    "@type": "unece:AssociationBIE",
                    "unece:cefactUNId": "UN01010892",
                    "unece:cefactBieDomainClass": "cefact:FLAP_Query.Details",
                    "rdfs:comment": "A vessel identity of a subject of this FLAP query."
                },
                {
                    "@id": "cefact:Vessel_Query.Subject.Vessel_Identity",
                    "@type": "unece:AssociationBIE",
                    "unece:cefactUNId": "UN01010742",
                    "unece:cefactBieDomainClass": "cefact:Vessel_Query.Details",
                    "rdfs:comment": "The identity of a subject of this vessel query."
                },
                {
                    "@id": "cefact:MDR_Query.Subject.MDRQuery_Identity",
                    "@type": "unece:AssociationBIE",
                    "unece:cefactUNId": "UN01010576",
                    "unece:cefactBieDomainClass": "cefact:MDR_Query.Details",
                    "rdfs:comment": "The identity of a subject of this MDR query."
                },
                {
                    "@id": "cefact:FLAP_Query.Subject.FLAP_Identity",
                    "@type": "unece:AssociationBIE",
                    "unece:cefactUNId": "UN01010891",
                    "unece:cefactBieDomainClass": "cefact:FLAP_Query.Details",
                    "rdfs:comment": "An identity of a subject of this FLAP query."
                }
            ]
        },
        {
            "@id": "fisheries:submittedDateTime",
            "@type": "rdf:Property",
            "schema:rangeIncludes": {
                "@id": "xsd:dateTime"
            },
            "schema:domainIncludes": {
                "@id": "fisheries:Query"
            },
            "rdfs:comment": [
                "The date, time, date time, or other date time value when this FA query was submitted.",
                "The date, time, date time, or other date time value when this FLAP query was submitted.",
                "The date, time, date time, or other date time value when this ISR query was submitted.",
                "The date, time, date time, or other date time value when this MDR query was submitted.",
                "The date, time, date time, or other date time value when this sales query was submitted.",
                "The date, time, date time, or other date time value when this vessel position query was submitted.",
                "The date, time, date time, or other date time value when this vessel query was submitted."
            ],
            "rdfs:label": "submittedDateTime",
            "unece:cefactElementMetadata": [
                {
                    "@id": "cefact:Vessel_Query.Submitted.DateTime",
                    "@type": "unece:BasicBIE",
                    "unece:cefactUNId": "UN01010737",
                    "unece:cefactBieDomainClass": "cefact:Vessel_Query.Details",
                    "rdfs:comment": "The date, time, date time, or other date time value when this vessel query was submitted."
                },
                {
                    "@id": "cefact:FLAP_Query.Submitted.DateTime",
                    "@type": "unece:BasicBIE",
                    "unece:cefactUNId": "UN01010888",
                    "unece:cefactBieDomainClass": "cefact:FLAP_Query.Details",
                    "rdfs:comment": "The date, time, date time, or other date time value when this FLAP query was submitted."
                },
                {
                    "@id": "cefact:FA_Query.Submitted.DateTime",
                    "@type": "unece:BasicBIE",
                    "unece:cefactUNId": "UN01011219",
                    "unece:cefactBieDomainClass": "cefact:FA_Query.Details",
                    "rdfs:comment": "The date, time, date time, or other date time value when this FA query was submitted."
                },
                {
                    "@id": "cefact:ISR_Query.Submitted.DateTime",
                    "@type": "unece:BasicBIE",
                    "unece:cefactUNId": "UN01012636",
                    "unece:cefactBieDomainClass": "cefact:ISR_Query.Details",
                    "rdfs:comment": "The date, time, date time, or other date time value when this ISR query was submitted."
                },
                {
                    "@id": "cefact:MDR_Query.Submitted.DateTime",
                    "@type": "unece:BasicBIE",
                    "unece:cefactUNId": "UN01010572",
                    "unece:cefactBieDomainClass": "cefact:MDR_Query.Details",
                    "rdfs:comment": "The date, time, date time, or other date time value when this MDR query was submitted."
                },
                {
                    "@id": "cefact:VesselPosition_Query.Submitted.DateTime",
                    "@type": "unece:BasicBIE",
                    "unece:cefactUNId": "UN01012648",
                    "unece:cefactBieDomainClass": "cefact:VesselPosition_Query.Details",
                    "rdfs:comment": "The date, time, date time, or other date time value when this vessel position query was submitted."
                },
                {
                    "@id": "cefact:Sales_Query.Submitted.DateTime",
                    "@type": "unece:BasicBIE",
                    "unece:cefactUNId": "UN01010995",
                    "unece:cefactBieDomainClass": "cefact:Sales_Query.Details",
                    "rdfs:comment": "The date, time, date time, or other date time value when this sales query was submitted."
                }
            ]
        },
        {
            "@id": "fisheries:submitterParty",
            "@type": "rdf:Property",
            "schema:rangeIncludes": {
                "@id": "fisheries:Party"
            },
            "schema:domainIncludes": {
                "@id": "fisheries:Query"
            },
            "rdfs:comment": [
                "The Fisheries Language for Universal Exchange (FLUX) party that submits this MDR query.",
                "The Fisheries Language for Universal eXchange (FLUX) party that submits this FLAP query.",
                "The Fisheries Language for Universal eXchange (FLUX) party that submits this sales query.",
                "The Fisheries Language for Universal eXchange (FLUX) party that submits this vessel query.",
                "The Fisheries Language for Universal eXchange (FLUX) party that submitted this FA query.",
                "The Fisheries Language for Universal eXchange (FLUX) party that submitted this ISR query.",
                "The Fisheries Language for Universal eXchange (FLUX) party that submitted this vessel position query."
            ],
            "rdfs:label": "submitterParty",
            "unece:cefactElementMetadata": [
                {
                    "@id": "cefact:Sales_Query.Submitter.FLUX_Party",
                    "@type": "unece:AssociationBIE",
                    "unece:cefactUNId": "UN01010998",
                    "unece:cefactBieDomainClass": "cefact:Sales_Query.Details",
                    "rdfs:comment": "The Fisheries Language for Universal eXchange (FLUX) party that submits this sales query."
                },
                {
                    "@id": "cefact:ISR_Query.Submitter.FLUX_Party",
                    "@type": "unece:AssociationBIE",
                    "unece:cefactUNId": "UN01012638",
                    "unece:cefactBieDomainClass": "cefact:ISR_Query.Details",
                    "rdfs:comment": "The Fisheries Language for Universal eXchange (FLUX) party that submitted this ISR query."
                },
                {
                    "@id": "cefact:VesselPosition_Query.Submitter.FLUX_Party",
                    "@type": "unece:AssociationBIE",
                    "unece:cefactUNId": "UN01012650",
                    "unece:cefactBieDomainClass": "cefact:VesselPosition_Query.Details",
                    "rdfs:comment": "The Fisheries Language for Universal eXchange (FLUX) party that submitted this vessel position query."
                },
                {
                    "@id": "cefact:MDR_Query.Submitter.FLUX_Party",
                    "@type": "unece:AssociationBIE",
                    "unece:cefactUNId": "UN01010575",
                    "unece:cefactBieDomainClass": "cefact:MDR_Query.Details",
                    "rdfs:comment": "The Fisheries Language for Universal Exchange (FLUX) party that submits this MDR query."
                },
                {
                    "@id": "cefact:FLAP_Query.Submitter.FLUX_Party",
                    "@type": "unece:AssociationBIE",
                    "unece:cefactUNId": "UN01010893",
                    "unece:cefactBieDomainClass": "cefact:FLAP_Query.Details",
                    "rdfs:comment": "The Fisheries Language for Universal eXchange (FLUX) party that submits this FLAP query."
                },
                {
                    "@id": "cefact:Vessel_Query.Submitter.FLUX_Party",
                    "@type": "unece:AssociationBIE",
                    "unece:cefactUNId": "UN01010739",
                    "unece:cefactBieDomainClass": "cefact:Vessel_Query.Details",
                    "rdfs:comment": "The Fisheries Language for Universal eXchange (FLUX) party that submits this vessel query."
                },
                {
                    "@id": "cefact:FA_Query.Submitter.FLUX_Party",
                    "@type": "unece:AssociationBIE",
                    "unece:cefactUNId": "UN01011222",
                    "unece:cefactBieDomainClass": "cefact:FA_Query.Details",
                    "rdfs:comment": "The Fisheries Language for Universal eXchange (FLUX) party that submitted this FA query."
                }
            ]
        },
        {
            "@id": "fisheries:subordinateDataNode",
            "@type": "rdf:Property",
            "schema:rangeIncludes": {
                "@id": "fisheries:DataNode"
            },
            "schema:domainIncludes": {
                "@id": "fisheries:DataNode"
            },
            "rdfs:comment": "An element data node that is subordinate to this MDR data node.",
            "rdfs:label": "subordinateDataNode",
            "unece:cefactElementMetadata": [
                {
                    "@id": "cefact:MDR_DataNode.Subordinate.MDRElement_DataNode",
                    "@type": "unece:AssociationBIE",
                    "unece:cefactUNId": "UN01010594",
                    "unece:cefactBieDomainClass": "cefact:MDR_DataNode.Details",
                    "rdfs:comment": "An element data node that is subordinate to this MDR data node."
                }
            ]
        },
        {
            "@id": "fisheries:subordinateEvent",
            "@type": "rdf:Property",
            "schema:rangeIncludes": {
                "@id": "fisheries:Event"
            },
            "schema:domainIncludes": {
                "@id": "fisheries:Event"
            },
            "rdfs:comment": "An IS event subordinate to this IS event.",
            "rdfs:label": "subordinateEvent",
            "unece:cefactElementMetadata": [
                {
                    "@id": "cefact:IS_Event.Subordinate.IS_Event",
                    "@type": "unece:AssociationBIE",
                    "unece:cefactUNId": "UN01012619",
                    "unece:cefactBieDomainClass": "cefact:IS_Event.Details",
                    "rdfs:comment": "An IS event subordinate to this IS event."
                }
            ]
        },
        {
            "@id": "fisheries:systemId",
            "@type": "rdf:Property",
            "schema:rangeIncludes": {
                "@id": "xsd:token"
            },
            "schema:domainIncludes": {
                "@id": "fisheries:GeographicalCoordinate"
            },
            "rdfs:comment": [
                "The identifier of the system used for measuring this specified FLUX geographical coordinate.",
                "The identifier of the system used for measuring this specified geographical coordinate."
            ],
            "rdfs:label": "systemId",
            "unece:cefactElementMetadata": [
                {
                    "@id": "cefact:Vessel_GeographicalCoordinate.System.Identifier",
                    "@type": "unece:BasicBIE",
                    "unece:cefactUNId": "UN01010225",
                    "unece:cefactBieDomainClass": "cefact:Vessel_GeographicalCoordinate.Details",
                    "rdfs:comment": "The identifier of the system used for measuring this specified geographical coordinate."
                },
                {
                    "@id": "cefact:FLUX_GeographicalCoordinate.System.Identifier",
                    "@type": "unece:BasicBIE",
                    "unece:cefactUNId": "UN01010970",
                    "unece:cefactBieDomainClass": "cefact:FLUX_GeographicalCoordinate.Details",
                    "rdfs:comment": "The identifier of the system used for measuring this specified FLUX geographical coordinate."
                }
            ]
        },
        {
            "@id": "fisheries:takenDateTime",
            "@type": "rdf:Property",
            "schema:rangeIncludes": {
                "@id": "xsd:dateTime"
            },
            "schema:domainIncludes": {
                "@id": "fisheries:Picture"
            },
            "rdfs:comment": "The date, time, date time, or other date value of when this FLUX picture was created.",
            "rdfs:label": "takenDateTime",
            "unece:cefactElementMetadata": [
                {
                    "@id": "cefact:FLUX_Picture.Taken.DateTime",
                    "@type": "unece:BasicBIE",
                    "unece:cefactUNId": "UN01010732",
                    "unece:cefactBieDomainClass": "cefact:FLUX_Picture.Details",
                    "rdfs:comment": "The date, time, date time, or other date value of when this FLUX picture was created."
                }
            ]
        },
        {
            "@id": "fisheries:takeoverDocumentId",
            "@type": "rdf:Property",
            "schema:rangeIncludes": {
                "@id": "xsd:token"
            },
            "schema:domainIncludes": {
                "@id": "fisheries:Document"
            },
            "rdfs:comment": "A takeover document identifier for this sales document.",
            "rdfs:label": "takeoverDocumentId",
            "unece:cefactElementMetadata": [
                {
                    "@id": "cefact:Sales_Document.TakeoverDocument_Identification.Identifier",
                    "@type": "unece:BasicBIE",
                    "unece:TDED": "1004",
                    "unece:cefactUNId": "UN01010914",
                    "unece:cefactBieDomainClass": "cefact:Sales_Document.Details",
                    "rdfs:comment": "A takeover document identifier for this sales document."
                }
            ]
        },
        {
            "@id": "fisheries:telephoneCommunication",
            "@type": "rdf:Property",
            "schema:rangeIncludes": {
                "@id": "fisheries:Communication"
            },
            "schema:domainIncludes": {
                "@id": "fisheries:Party"
            },
            "rdfs:comment": "Telephone communication information for this contact party.",
            "rdfs:label": "telephoneCommunication",
            "unece:cefactElementMetadata": [
                {
                    "@id": "cefact:Contact_Party.Telephone.Telecommunication_Communication",
                    "@type": "unece:AssociationBIE",
                    "unece:cefactUNId": "UN01010786",
                    "unece:cefactBieDomainClass": "cefact:Contact_Party.Details",
                    "rdfs:comment": "Telephone communication information for this contact party."
                }
            ]
        },
        {
            "@id": "fisheries:temperatureValueMeasure",
            "@type": "rdf:Property",
            "schema:rangeIncludes": {
                "@id": "xsd:decimal"
            },
            "schema:domainIncludes": {
                "@id": "fisheries:Characteristic"
            },
            "rdfs:comment": "A value of temperature, expressed as a measure, for this vessel storage characteristic.",
            "rdfs:label": "temperatureValueMeasure",
            "unece:cefactElementMetadata": [
                {
                    "@id": "cefact:VesselStorage_Characteristic.Temperature_Value.Measure",
                    "@type": "unece:BasicBIE",
                    "unece:cefactUNId": "UN01010810",
                    "unece:cefactBieDomainClass": "cefact:VesselStorage_Characteristic.Details",
                    "rdfs:comment": "A value of temperature, expressed as a measure, for this vessel storage characteristic."
                }
            ]
        },
        {
            "@id": "fisheries:title",
            "@type": "rdf:Property",
            "schema:rangeIncludes": {
                "@id": "xsd:string"
            },
            "schema:domainIncludes": {
                "@id": "fisheries:BinaryFile"
            },
            "rdfs:comment": "The title, expressed as text, for this FLUX binary file.",
            "rdfs:label": "title",
            "unece:cefactElementMetadata": [
                {
                    "@id": "cefact:FLUX_BinaryFile.Title.Text",
                    "@type": "unece:BasicBIE",
                    "unece:cefactUNId": "UN01010800",
                    "unece:cefactBieDomainClass": "cefact:FLUX_BinaryFile.Details",
                    "rdfs:comment": "The title, expressed as text, for this FLUX binary file."
                }
            ]
        },
        {
            "@id": "fisheries:toleranceMarginNumeric",
            "@type": "rdf:Property",
            "schema:rangeIncludes": {
                "@id": "xsd:decimal"
            },
            "schema:domainIncludes": {
                "@id": "fisheries:Catch"
            },
            "rdfs:comment": "The value, expressed as a number, of a margin of tolerance applied to the weight or the count specified for this FA catch.",
            "rdfs:label": "toleranceMarginNumeric",
            "unece:cefactElementMetadata": [
                {
                    "@id": "cefact:FA_Catch.ToleranceMargin.Numeric",
                    "@type": "unece:BasicBIE",
                    "unece:cefactUNId": "UN01012656",
                    "unece:cefactBieDomainClass": "cefact:FA_Catch.Details",
                    "rdfs:comment": "The value, expressed as a number, of a margin of tolerance applied to the weight or the count specified for this FA catch."
                }
            ]
        },
        {
            "@id": "fisheries:totalPrice",
            "@type": "rdf:Property",
            "schema:rangeIncludes": {
                "@id": "fisheries:Price"
            },
            "schema:domainIncludes": [
                {
                    "@id": "fisheries:Batch"
                },
                {
                    "@id": "fisheries:Document"
                },
                {
                    "@id": "fisheries:Product"
                }
            ],
            "rdfs:comment": [
                "The total sales price for this AAP product.",
                "The total sales price for this batch.",
                "The total sales price in this sales document."
            ],
            "rdfs:label": "totalPrice",
            "unece:cefactElementMetadata": [
                {
                    "@id": "cefact:AAP_Product.Total.Sales_Price",
                    "@type": "unece:AssociationBIE",
                    "unece:cefactUNId": "UN01010941",
                    "unece:cefactBieDomainClass": "cefact:AAP_Product.Details",
                    "rdfs:comment": "The total sales price for this AAP product."
                },
                {
                    "@id": "cefact:Sales_Batch.Total.Sales_Price",
                    "@type": "unece:AssociationBIE",
                    "unece:cefactUNId": "UN01010932",
                    "unece:cefactBieDomainClass": "cefact:Sales_Batch.Details",
                    "rdfs:comment": "The total sales price for this batch."
                },
                {
                    "@id": "cefact:Sales_Document.Total.Sales_Price",
                    "@type": "unece:AssociationBIE",
                    "unece:cefactUNId": "UN01011142",
                    "unece:cefactBieDomainClass": "cefact:Sales_Document.Details",
                    "rdfs:comment": "The total sales price in this sales document."
                }
            ]
        },
        {
            "@id": "fisheries:transmissionDateTime",
            "@type": "rdf:Property",
            "schema:rangeIncludes": {
                "@id": "xsd:dateTime"
            },
            "schema:domainIncludes": {
                "@id": "fisheries:Document"
            },
            "rdfs:comment": "The date, time, date time, or other date time value, of the transmission of a document referenced in this FA report document.",
            "rdfs:label": "transmissionDateTime",
            "unece:cefactElementMetadata": [
                {
                    "@id": "cefact:FAReport_Document.Transmission.DateTime",
                    "@type": "unece:BasicBIE",
                    "unece:cefactUNId": "UN01013077",
                    "unece:cefactBieDomainClass": "cefact:FAReport_Document.Details",
                    "rdfs:comment": "The date, time, date time, or other date time value, of the transmission of a document referenced in this FA report document."
                }
            ]
        },
        {
            "@id": "fisheries:transportDocumentId",
            "@type": "rdf:Property",
            "schema:rangeIncludes": {
                "@id": "xsd:token"
            },
            "schema:domainIncludes": {
                "@id": "fisheries:Document"
            },
            "rdfs:comment": "A transport document identifier for this sales document.",
            "rdfs:label": "transportDocumentId",
            "unece:cefactElementMetadata": [
                {
                    "@id": "cefact:Sales_Document.TransportDocument_Identification.Identifier",
                    "@type": "unece:BasicBIE",
                    "unece:TDED": "1004",
                    "unece:cefactUNId": "UN01010912",
                    "unece:cefactBieDomainClass": "cefact:Sales_Document.Details",
                    "rdfs:comment": "A transport document identifier for this sales document."
                }
            ]
        },
        {
            "@id": "fisheries:transportEquipmentId",
            "@type": "rdf:Property",
            "schema:rangeIncludes": {
                "@id": "xsd:token"
            },
            "schema:domainIncludes": {
                "@id": "fisheries:TransportMeans"
            },
            "rdfs:comment": "An identifier for a piece of transport equipment for this vehicle transport means.",
            "rdfs:label": "transportEquipmentId",
            "unece:cefactElementMetadata": [
                {
                    "@id": "cefact:Vehicle_TransportMeans.TransportEquipment.Identifier",
                    "@type": "unece:BasicBIE",
                    "unece:cefactUNId": "UN01013338",
                    "unece:cefactBieDomainClass": "cefact:Vehicle_TransportMeans.Details",
                    "rdfs:comment": "An identifier for a piece of transport equipment for this vehicle transport means."
                }
            ]
        },
        {
            "@id": "fisheries:trawlingSpeedMeasure",
            "@type": "rdf:Property",
            "schema:rangeIncludes": {
                "@id": "xsd:decimal"
            },
            "schema:domainIncludes": {
                "@id": "fisheries:TransportMeans"
            },
            "rdfs:comment": "The trawling speed measured for this transport means vessel.",
            "rdfs:label": "trawlingSpeedMeasure",
            "unece:cefactElementMetadata": [
                {
                    "@id": "cefact:Vessel_TransportMeans.Trawling_Speed.Measure",
                    "@type": "unece:BasicBIE",
                    "unece:cefactUNId": "UN01010770",
                    "unece:cefactBieDomainClass": "cefact:Vessel_TransportMeans.Details",
                    "rdfs:comment": "The trawling speed measured for this transport means vessel."
                }
            ]
        },
        {
            "@id": "fisheries:typeCode",
            "@type": "rdf:Property",
            "schema:rangeIncludes": {
                "@id": "xsd:token"
            },
            "schema:domainIncludes": [
                {
                    "@id": "fisheries:ACDRReport"
                },
                {
                    "@id": "fisheries:Activity"
                },
                {
                    "@id": "fisheries:BinaryFile"
                },
                {
                    "@id": "fisheries:Catch"
                },
                {
                    "@id": "fisheries:Category"
                },
                {
                    "@id": "fisheries:Characteristic"
                },
                {
                    "@id": "fisheries:Crew"
                },
                {
                    "@id": "fisheries:DataNode"
                },
                {
                    "@id": "fisheries:Engine"
                },
                {
                    "@id": "fisheries:Equipment"
                },
                {
                    "@id": "fisheries:Event"
                },
                {
                    "@id": "fisheries:Gear"
                },
                {
                    "@id": "fisheries:Means"
                },
                {
                    "@id": "fisheries:Party"
                },
                {
                    "@id": "fisheries:Picture"
                },
                {
                    "@id": "fisheries:Problem"
                },
                {
                    "@id": "fisheries:QualityAnalysis"
                },
                {
                    "@id": "fisheries:Query"
                },
                {
                    "@id": "fisheries:QueryParameter"
                },
                {
                    "@id": "fisheries:Quota"
                },
                {
                    "@id": "fisheries:Report"
                },
                {
                    "@id": "fisheries:Suspicion"
                },
                {
                    "@id": "fisheries:TransportCharter"
                },
                {
                    "@id": "fisheries:Trip"
                }
            ],
            "rdfs:comment": [
                "A code specifying a type of fish catch characteristic.",
                "A code specifying the type of ISR infringement suspicion.",
                "A code specifying the type of sales query.",
                "A code specifying the type of this vessel storage characteristic.",
                "The code specifying a type for this FA catch, such as retained on board or discarded.",
                "The code specifying a type for this MDR element data node.",
                "The code specifying a type of FLUX characteristic.",
                "The code specifying a type of FLUX picture.",
                "The code specifying a type of IS report, such as inspection at sea, inspection in port or surveillance report.",
                "The code specifying a type of ISR item characteristic.",
                "The code specifying a type of fishing activity, such as depart from port, return to port, fishing operation.",
                "The code specifying a type of fishing category.",
                "The code specifying a type of fishing trip.",
                "The code specifying a type of gear characteristic.",
                "The code specifying a type of gear problem.",
                "The code specifying a type of historical characteristic of a vessel.",
                "The code specifying a type of quality analysis of a validation process.",
                "The code specifying a type of surveillance means.",
                "The code specifying a type of this vessel crew.",
                "The code specifying a type of vessel administrative characteristic, such as mainland fleet, aquaculture, public aid code, administrative decision code.",
                "The code specifying a type of vessel equipment characteristic, such as Vessel Monitoring System (VMS), Automatic Identification System (AIS).",
                "The code specifying a type of vessel technical characteristic, such as maximum speed, trawling speed or hull material.",
                "The code specifying the type of FA query parameter.",
                "The code specifying the type of FA query.",
                "The code specifying the type of FLAP query.",
                "The code specifying the type of FLUX binary file, such as photo, spreadsheet.",
                "The code specifying the type of IS event.",
                "The code specifying the type of ISR query parameter.",
                "The code specifying the type of ISR query.",
                "The code specifying the type of MDR query.",
                "The code specifying the type of fishing gear equipment, such as a chafer, a codline or a flapper.",
                "The code specifying the type of fishing gear.",
                "The code specifying the type of sales party.",
                "The code specifying the type of sales query parameter.",
                "The code specifying the type of targeted quota.",
                "The code specifying the type of this ACDR Report.",
                "The code specifying the type of vessel engine.",
                "The code specifying the type of vessel event.",
                "The code specifying the type of vessel position event.",
                "The code specifying the type of vessel position query.",
                "The code specifying the type of vessel query.",
                "The code specifying the type of vessel transport charter."
            ],
            "rdfs:label": "typeCode",
            "unece:cefactElementMetadata": [
                {
                    "@id": "cefact:VesselEquipment_Characteristic.Type.Code",
                    "@type": "unece:BasicBIE",
                    "unece:cefactUNId": "UN01010693",
                    "unece:cefactBieDomainClass": "cefact:VesselEquipment_Characteristic.Details",
                    "rdfs:comment": "The code specifying a type of vessel equipment characteristic, such as Vessel Monitoring System (VMS), Automatic Identification System (AIS)."
                },
                {
                    "@id": "cefact:FLUX_ACDRReport.Type.Code",
                    "@type": "unece:BasicBIE",
                    "unece:cefactUNId": "UN01010758",
                    "unece:cefactBieDomainClass": "cefact:FLUX_ACDRReport.Details",
                    "rdfs:comment": "The code specifying the type of this ACDR Report."
                },
                {
                    "@id": "cefact:Fishing_Gear.Type.Code",
                    "@type": "unece:BasicBIE",
                    "unece:cefactUNId": "UN01010727",
                    "unece:cefactBieDomainClass": "cefact:Fishing_Gear.Details",
                    "rdfs:comment": "The code specifying the type of fishing gear."
                },
                {
                    "@id": "cefact:ISRItem_Characteristic.Type.Code",
                    "@type": "unece:BasicBIE",
                    "unece:cefactUNId": "UN01012603",
                    "unece:cefactBieDomainClass": "cefact:ISRItem_Characteristic.Details",
                    "rdfs:comment": "The code specifying a type of ISR item characteristic."
                },
                {
                    "@id": "cefact:FLUX_Characteristic.Type.Code",
                    "@type": "unece:BasicBIE",
                    "unece:cefactUNId": "UN01010866",
                    "unece:cefactBieDomainClass": "cefact:FLUX_Characteristic.Details",
                    "rdfs:comment": "The code specifying a type of FLUX characteristic."
                },
                {
                    "@id": "cefact:ISR_Query.Type.Code",
                    "@type": "unece:BasicBIE",
                    "unece:cefactUNId": "UN01012637",
                    "unece:cefactBieDomainClass": "cefact:ISR_Query.Details",
                    "rdfs:comment": "The code specifying the type of ISR query."
                },
                {
                    "@id": "cefact:Surveillance_Means.Type.Code",
                    "@type": "unece:BasicBIE",
                    "unece:cefactUNId": "UN01012631",
                    "unece:cefactBieDomainClass": "cefact:Surveillance_Means.Details",
                    "rdfs:comment": "The code specifying a type of surveillance means."
                },
                {
                    "@id": "cefact:VesselTechnical_Characteristic.Type.Code",
                    "@type": "unece:BasicBIE",
                    "unece:cefactUNId": "UN01010790",
                    "unece:cefactBieDomainClass": "cefact:VesselTechnical_Characteristic.Details",
                    "rdfs:comment": "The code specifying a type of vessel technical characteristic, such as maximum speed, trawling speed or hull material."
                },
                {
                    "@id": "cefact:FA_QueryParameter.Type.Code",
                    "@type": "unece:BasicBIE",
                    "unece:cefactUNId": "UN01011225",
                    "unece:cefactBieDomainClass": "cefact:FA_QueryParameter.Details",
                    "rdfs:comment": "The code specifying the type of FA query parameter."
                },
                {
                    "@id": "cefact:Sales_QueryParameter.Type.Code",
                    "@type": "unece:BasicBIE",
                    "unece:cefactUNId": "UN01011001",
                    "unece:cefactBieDomainClass": "cefact:Sales_QueryParameter.Details",
                    "rdfs:comment": "The code specifying the type of sales query parameter."
                },
                {
                    "@id": "cefact:Fishing_Activity.Type.Code",
                    "@type": "unece:BasicBIE",
                    "unece:cefactUNId": "UN01011170",
                    "unece:cefactBieDomainClass": "cefact:Fishing_Activity.Details",
                    "rdfs:comment": "The code specifying a type of fishing activity, such as depart from port, return to port, fishing operation."
                },
                {
                    "@id": "cefact:Fishing_Trip.Type.Code",
                    "@type": "unece:BasicBIE",
                    "unece:cefactUNId": "UN01011166",
                    "unece:cefactBieDomainClass": "cefact:Fishing_Trip.Details",
                    "rdfs:comment": "The code specifying a type of fishing trip."
                },
                {
                    "@id": "cefact:MDRElement_DataNode.Type.Code",
                    "@type": "unece:BasicBIE",
                    "unece:cefactUNId": "UN01010603",
                    "unece:cefactBieDomainClass": "cefact:MDRElement_DataNode.Details",
                    "rdfs:comment": "The code specifying a type for this MDR element data node."
                },
                {
                    "@id": "cefact:VesselAdministrative_Characteristic.Type.Code",
                    "@type": "unece:BasicBIE",
                    "unece:cefactUNId": "UN01010701",
                    "unece:cefactBieDomainClass": "cefact:VesselAdministrative_Characteristic.Details",
                    "rdfs:comment": "The code specifying a type of vessel administrative characteristic, such as mainland fleet, aquaculture, public aid code, administrative decision code."
                },
                {
                    "@id": "cefact:Gear_Characteristic.Type.Code",
                    "@type": "unece:BasicBIE",
                    "unece:cefactUNId": "UN01010820",
                    "unece:cefactBieDomainClass": "cefact:Gear_Characteristic.Details",
                    "rdfs:comment": "The code specifying a type of gear characteristic."
                },
                {
                    "@id": "cefact:Sales_Query.Type.Code",
                    "@type": "unece:BasicBIE",
                    "unece:cefactUNId": "UN01010996",
                    "unece:cefactBieDomainClass": "cefact:Sales_Query.Details",
                    "rdfs:comment": "A code specifying the type of sales query."
                },
                {
                    "@id": "cefact:VesselStorage_Characteristic.Type.Code",
                    "@type": "unece:BasicBIE",
                    "unece:cefactUNId": "UN01010807",
                    "unece:cefactBieDomainClass": "cefact:VesselStorage_Characteristic.Details",
                    "rdfs:comment": "A code specifying the type of this vessel storage characteristic."
                },
                {
                    "@id": "cefact:Vessel_TransportCharter.Type.Code",
                    "@type": "unece:BasicBIE",
                    "unece:cefactUNId": "UN01010875",
                    "unece:cefactBieDomainClass": "cefact:Vessel_TransportCharter.Details",
                    "rdfs:comment": "The code specifying the type of vessel transport charter."
                },
                {
                    "@id": "cefact:Gear_Problem.Type.Code",
                    "@type": "unece:BasicBIE",
                    "unece:cefactUNId": "UN01011209",
                    "unece:cefactBieDomainClass": "cefact:Gear_Problem.Details",
                    "rdfs:comment": "The code specifying a type of gear problem."
                },
                {
                    "@id": "cefact:FishingGear_Equipment.Type.Code",
                    "@type": "unece:BasicBIE",
                    "unece:cefactUNId": "UN01012658",
                    "unece:cefactBieDomainClass": "cefact:FishingGear_Equipment.Details",
                    "rdfs:comment": "The code specifying the type of fishing gear equipment, such as a chafer, a codline or a flapper."
                },
                {
                    "@id": "cefact:FLUX_BinaryFile.Type.Code",
                    "@type": "unece:BasicBIE",
                    "unece:cefactUNId": "UN01010804",
                    "unece:cefactBieDomainClass": "cefact:FLUX_BinaryFile.Details",
                    "rdfs:comment": "The code specifying the type of FLUX binary file, such as photo, spreadsheet."
                },
                {
                    "@id": "cefact:Targeted_Quota.Type.Code",
                    "@type": "unece:BasicBIE",
                    "unece:cefactUNId": "UN01010879",
                    "unece:cefactBieDomainClass": "cefact:Targeted_Quota.Details",
                    "rdfs:comment": "The code specifying the type of targeted quota."
                },
                {
                    "@id": "cefact:VesselHistorical_Characteristic.Type.Code",
                    "@type": "unece:BasicBIE",
                    "unece:cefactUNId": "UN01010651",
                    "unece:cefactBieDomainClass": "cefact:VesselHistorical_Characteristic.Details",
                    "rdfs:comment": "The code specifying a type of historical characteristic of a vessel."
                },
                {
                    "@id": "cefact:FA_Catch.Type.Code",
                    "@type": "unece:BasicBIE",
                    "unece:cefactUNId": "UN01011190",
                    "unece:cefactBieDomainClass": "cefact:FA_Catch.Details",
                    "rdfs:comment": "The code specifying a type for this FA catch, such as retained on board or discarded."
                },
                {
                    "@id": "cefact:Vessel_Query.Type.Code",
                    "@type": "unece:BasicBIE",
                    "unece:cefactUNId": "UN01010738",
                    "unece:cefactBieDomainClass": "cefact:Vessel_Query.Details",
                    "rdfs:comment": "The code specifying the type of vessel query."
                },
                {
                    "@id": "cefact:FLAP_Query.Type.Code",
                    "@type": "unece:BasicBIE",
                    "unece:cefactUNId": "UN01010889",
                    "unece:cefactBieDomainClass": "cefact:FLAP_Query.Details",
                    "rdfs:comment": "The code specifying the type of FLAP query."
                },
                {
                    "@id": "cefact:FishCatch_Characteristic.Type.Code",
                    "@type": "unece:BasicBIE",
                    "unece:cefactUNId": "UN01011285",
                    "unece:cefactBieDomainClass": "cefact:FishCatch_Characteristic.Details",
                    "rdfs:comment": "A code specifying a type of fish catch characteristic."
                },
                {
                    "@id": "cefact:ISR_QueryParameter.Type.Code",
                    "@type": "unece:BasicBIE",
                    "unece:cefactUNId": "UN01012642",
                    "unece:cefactBieDomainClass": "cefact:ISR_QueryParameter.Details",
                    "rdfs:comment": "The code specifying the type of ISR query parameter."
                },
                {
                    "@id": "cefact:Vessel_Event.Type.Code",
                    "@type": "unece:BasicBIE",
                    "unece:TDED": "9171",
                    "unece:cefactUNId": "UN01010660",
                    "unece:cefactBieDomainClass": "cefact:Vessel_Event.Details",
                    "rdfs:comment": "The code specifying the type of vessel event."
                },
                {
                    "@id": "cefact:VesselPosition_Query.Type.Code",
                    "@type": "unece:BasicBIE",
                    "unece:cefactUNId": "UN01012649",
                    "unece:cefactBieDomainClass": "cefact:VesselPosition_Query.Details",
                    "rdfs:comment": "The code specifying the type of vessel position query."
                },
                {
                    "@id": "cefact:FA_Query.Type.Code",
                    "@type": "unece:BasicBIE",
                    "unece:cefactUNId": "UN01011220",
                    "unece:cefactBieDomainClass": "cefact:FA_Query.Details",
                    "rdfs:comment": "The code specifying the type of FA query."
                },
                {
                    "@id": "cefact:VesselPosition_Event.Type.Code",
                    "@type": "unece:BasicBIE",
                    "unece:TDED": "9171",
                    "unece:cefactUNId": "UN01010235",
                    "unece:cefactBieDomainClass": "cefact:VesselPosition_Event.Details",
                    "rdfs:comment": "The code specifying the type of vessel position event."
                },
                {
                    "@id": "cefact:ISRInfringement_Suspicion.Type.Code",
                    "@type": "unece:BasicBIE",
                    "unece:cefactUNId": "UN01013323",
                    "unece:cefactBieDomainClass": "cefact:ISRInfringement_Suspicion.Details",
                    "rdfs:comment": "A code specifying the type of ISR infringement suspicion."
                },
                {
                    "@id": "cefact:IS_Event.Type.Code",
                    "@type": "unece:BasicBIE",
                    "unece:cefactUNId": "UN01012617",
                    "unece:cefactBieDomainClass": "cefact:IS_Event.Details",
                    "rdfs:comment": "The code specifying the type of IS event."
                },
                {
                    "@id": "cefact:IS_Report.Type.Code",
                    "@type": "unece:BasicBIE",
                    "unece:cefactUNId": "UN01012589",
                    "unece:cefactBieDomainClass": "cefact:IS_Report.Details",
                    "rdfs:comment": "The code specifying a type of IS report, such as inspection at sea, inspection in port or surveillance report."
                },
                {
                    "@id": "cefact:Vessel_Crew.Type.Code",
                    "@type": "unece:BasicBIE",
                    "unece:cefactUNId": "UN01010813",
                    "unece:cefactBieDomainClass": "cefact:Vessel_Crew.Details",
                    "rdfs:comment": "The code specifying a type of this vessel crew."
                },
                {
                    "@id": "cefact:FLUX_Picture.Type.Code",
                    "@type": "unece:BasicBIE",
                    "unece:cefactUNId": "UN01010731",
                    "unece:cefactBieDomainClass": "cefact:FLUX_Picture.Details",
                    "rdfs:comment": "The code specifying a type of FLUX picture."
                },
                {
                    "@id": "cefact:Fishing_Category.Type.Code",
                    "@type": "unece:BasicBIE",
                    "unece:cefactUNId": "UN01010838",
                    "unece:cefactBieDomainClass": "cefact:Fishing_Category.Details",
                    "rdfs:comment": "The code specifying a type of fishing category."
                },
                {
                    "@id": "cefact:Sales_Party.Type.Code",
                    "@type": "unece:BasicBIE",
                    "unece:cefactUNId": "UN01010925",
                    "unece:cefactBieDomainClass": "cefact:Sales_Party.Details",
                    "rdfs:comment": "The code specifying the type of sales party."
                },
                {
                    "@id": "cefact:Vessel_Engine.Type.Code",
                    "@type": "unece:BasicBIE",
                    "unece:cefactUNId": "UN01010719",
                    "unece:cefactBieDomainClass": "cefact:Vessel_Engine.Details",
                    "rdfs:comment": "The code specifying the type of vessel engine."
                },
                {
                    "@id": "cefact:MDR_Query.Type.Code",
                    "@type": "unece:BasicBIE",
                    "unece:cefactUNId": "UN01010573",
                    "unece:cefactBieDomainClass": "cefact:MDR_Query.Details",
                    "rdfs:comment": "The code specifying the type of MDR query."
                },
                {
                    "@id": "cefact:Validation_QualityAnalysis.Type.Code",
                    "@type": "unece:BasicBIE",
                    "unece:cefactUNId": "UN01010756",
                    "unece:cefactBieDomainClass": "cefact:Validation_QualityAnalysis.Details",
                    "rdfs:comment": "The code specifying a type of quality analysis of a validation process."
                }
            ]
        },
        {
            "@id": "fisheries:uRICommunication",
            "@type": "rdf:Property",
            "schema:rangeIncludes": {
                "@id": "fisheries:Communication"
            },
            "schema:domainIncludes": {
                "@id": "fisheries:Party"
            },
            "rdfs:comment": "Email Uniform Resource Identifier (URI) communication for this contact party.",
            "rdfs:label": "uRICommunication",
            "unece:cefactElementMetadata": [
                {
                    "@id": "cefact:Contact_Party.URI.Email_Communication",
                    "@type": "unece:AssociationBIE",
                    "unece:cefactUNId": "UN01010788",
                    "unece:cefactBieDomainClass": "cefact:Contact_Party.Details",
                    "rdfs:comment": "Email Uniform Resource Identifier (URI) communication for this contact party."
                }
            ]
        },
        {
            "@id": "fisheries:unitQuantity",
            "@type": "rdf:Property",
            "schema:rangeIncludes": {
                "@id": "xsd:decimal"
            },
            "schema:domainIncludes": [
                {
                    "@id": "fisheries:Catch"
                },
                {
                    "@id": "fisheries:Product"
                }
            ],
            "rdfs:comment": [
                "The quantity of fish units for this FA catch.",
                "The quantity of fish, according to the unit used to declare catches, for this ACDR catch.",
                "The unit quantity for this AAP product."
            ],
            "rdfs:label": "unitQuantity",
            "unece:cefactElementMetadata": [
                {
                    "@id": "cefact:FA_Catch.Unit.Quantity",
                    "@type": "unece:BasicBIE",
                    "unece:cefactUNId": "UN01010973",
                    "unece:cefactBieDomainClass": "cefact:FA_Catch.Details",
                    "rdfs:comment": "The quantity of fish units for this FA catch."
                },
                {
                    "@id": "cefact:ACDR_Catch.Unit.Quantity",
                    "@type": "unece:BasicBIE",
                    "unece:cefactUNId": "UN01010266",
                    "unece:cefactBieDomainClass": "cefact:ACDR_Catch.Details",
                    "rdfs:comment": "The quantity of fish, according to the unit used to declare catches, for this ACDR catch."
                },
                {
                    "@id": "cefact:AAP_Product.Unit.Quantity",
                    "@type": "unece:BasicBIE",
                    "unece:cefactUNId": "UN01010935",
                    "unece:cefactBieDomainClass": "cefact:AAP_Product.Details",
                    "rdfs:comment": "The unit quantity for this AAP product."
                }
            ]
        },
        {
            "@id": "fisheries:unitValueQuantity",
            "@type": "rdf:Property",
            "schema:rangeIncludes": {
                "@id": "xsd:decimal"
            },
            "schema:domainIncludes": {
                "@id": "fisheries:Characteristic"
            },
            "rdfs:comment": "The unit value, expressed as a quantity, for this vessel storage characteristic.",
            "rdfs:label": "unitValueQuantity",
            "unece:cefactElementMetadata": [
                {
                    "@id": "cefact:VesselStorage_Characteristic.Unit_Value.Quantity",
                    "@type": "unece:BasicBIE",
                    "unece:cefactUNId": "UN01010811",
                    "unece:cefactBieDomainClass": "cefact:VesselStorage_Characteristic.Details",
                    "rdfs:comment": "The unit value, expressed as a quantity, for this vessel storage characteristic."
                }
            ]
        },
        {
            "@id": "fisheries:usageCode",
            "@type": "rdf:Property",
            "schema:rangeIncludes": {
                "@id": "xsd:token"
            },
            "schema:domainIncludes": [
                {
                    "@id": "fisheries:Catch"
                },
                {
                    "@id": "fisheries:Product"
                }
            ],
            "rdfs:comment": [
                "The code specifying a usage for this AAP product.",
                "The code specifying a usage for this FA catch, such as commercial or discard.",
                "The code specifying a usage of this ACDR catch, such as commercial or discard."
            ],
            "rdfs:label": "usageCode",
            "unece:cefactElementMetadata": [
                {
                    "@id": "cefact:ACDR_Catch.Usage.Code",
                    "@type": "unece:BasicBIE",
                    "unece:cefactUNId": "UN01010268",
                    "unece:cefactBieDomainClass": "cefact:ACDR_Catch.Details",
                    "rdfs:comment": "The code specifying a usage of this ACDR catch, such as commercial or discard."
                },
                {
                    "@id": "cefact:AAP_Product.Usage.Code",
                    "@type": "unece:BasicBIE",
                    "unece:cefactUNId": "UN01010938",
                    "unece:cefactBieDomainClass": "cefact:AAP_Product.Details",
                    "rdfs:comment": "The code specifying a usage for this AAP product."
                },
                {
                    "@id": "cefact:FA_Catch.Usage.Code",
                    "@type": "unece:BasicBIE",
                    "unece:cefactUNId": "UN01010976",
                    "unece:cefactBieDomainClass": "cefact:FA_Catch.Details",
                    "rdfs:comment": "The code specifying a usage for this FA catch, such as commercial or discard."
                }
            ]
        },
        {
            "@id": "fisheries:usedCatch",
            "@type": "rdf:Property",
            "schema:rangeIncludes": {
                "@id": "fisheries:Catch"
            },
            "schema:domainIncludes": {
                "@id": "fisheries:Process"
            },
            "rdfs:comment": "A Fishing Activity (FA) catch used for this AAP process.",
            "rdfs:label": "usedCatch",
            "unece:cefactElementMetadata": [
                {
                    "@id": "cefact:AAP_Process.Used.FA_Catch",
                    "@type": "unece:AssociationBIE",
                    "unece:cefactUNId": "UN01011150",
                    "unece:cefactBieDomainClass": "cefact:AAP_Process.Details",
                    "rdfs:comment": "A Fishing Activity (FA) catch used for this AAP process."
                }
            ]
        },
        {
            "@id": "fisheries:usedGear",
            "@type": "rdf:Property",
            "schema:rangeIncludes": {
                "@id": "fisheries:Gear"
            },
            "schema:domainIncludes": {
                "@id": "fisheries:Catch"
            },
            "rdfs:comment": "A fishing gear used for this FA catch.",
            "rdfs:label": "usedGear",
            "unece:cefactElementMetadata": [
                {
                    "@id": "cefact:FA_Catch.Used.Fishing_Gear",
                    "@type": "unece:AssociationBIE",
                    "unece:cefactUNId": "UN01011197",
                    "unece:cefactBieDomainClass": "cefact:FA_Catch.Details",
                    "rdfs:comment": "A fishing gear used for this FA catch."
                }
            ]
        },
        {
            "@id": "fisheries:validFromDateTime",
            "@type": "rdf:Property",
            "schema:rangeIncludes": {
                "@id": "xsd:dateTime"
            },
            "schema:domainIncludes": {
                "@id": "fisheries:Identity"
            },
            "rdfs:comment": "A date, time, date time or other date time value from which this MDR query identity is valid.",
            "rdfs:label": "validFromDateTime",
            "unece:cefactElementMetadata": [
                {
                    "@id": "cefact:MDRQuery_Identity.ValidFrom.DateTime",
                    "@type": "unece:BasicBIE",
                    "unece:cefactUNId": "UN01010579",
                    "unece:cefactBieDomainClass": "cefact:MDRQuery_Identity.Details",
                    "rdfs:comment": "A date, time, date time or other date time value from which this MDR query identity is valid."
                }
            ]
        },
        {
            "@id": "fisheries:validatorId",
            "@type": "rdf:Property",
            "schema:rangeIncludes": {
                "@id": "xsd:token"
            },
            "schema:domainIncludes": {
                "@id": "fisheries:Document"
            },
            "rdfs:comment": "The identifier of the validator for this validation result document.",
            "rdfs:label": "validatorId",
            "unece:cefactElementMetadata": [
                {
                    "@id": "cefact:ValidationResult_Document.Validator_Identification.Identifier",
                    "@type": "unece:BasicBIE",
                    "unece:TDED": "1004",
                    "unece:cefactUNId": "UN01010751",
                    "unece:cefactBieDomainClass": "cefact:ValidationResult_Document.Details",
                    "rdfs:comment": "The identifier of the validator for this validation result document."
                }
            ]
        },
        {
            "@id": "fisheries:validityEndDateTime",
            "@type": "rdf:Property",
            "schema:rangeIncludes": {
                "@id": "xsd:dateTime"
            },
            "schema:domainIncludes": {
                "@id": "fisheries:Version"
            },
            "rdfs:comment": "The date, time or other date time value up to which this data set version is valid.",
            "rdfs:label": "validityEndDateTime",
            "unece:cefactElementMetadata": [
                {
                    "@id": "cefact:DataSet_Version.ValidityEnd.DateTime",
                    "@type": "unece:BasicBIE",
                    "unece:cefactUNId": "UN01010602",
                    "unece:cefactBieDomainClass": "cefact:DataSet_Version.Details",
                    "rdfs:comment": "The date, time or other date time value up to which this data set version is valid."
                }
            ]
        },
        {
            "@id": "fisheries:validityPeriod",
            "@type": "rdf:Property",
            "schema:rangeIncludes": {
                "@id": "fisheries:Period"
            },
            "schema:domainIncludes": {
                "@id": "fisheries:Identity"
            },
            "rdfs:comment": "The delimited period for which this MDR query identity is valid.",
            "rdfs:label": "validityPeriod",
            "unece:cefactElementMetadata": [
                {
                    "@id": "cefact:MDRQuery_Identity.Validity.Delimited_Period",
                    "@type": "unece:AssociationBIE",
                    "unece:cefactUNId": "UN01010581",
                    "unece:cefactBieDomainClass": "cefact:MDRQuery_Identity.Details",
                    "rdfs:comment": "The delimited period for which this MDR query identity is valid."
                }
            ]
        },
        {
            "@id": "fisheries:validityStartDateTime",
            "@type": "rdf:Property",
            "schema:rangeIncludes": {
                "@id": "xsd:dateTime"
            },
            "schema:domainIncludes": {
                "@id": "fisheries:Version"
            },
            "rdfs:comment": "The date, time or other date time value from which this data set version is valid.",
            "rdfs:label": "validityStartDateTime",
            "unece:cefactElementMetadata": [
                {
                    "@id": "cefact:DataSet_Version.ValidityStart.DateTime",
                    "@type": "unece:BasicBIE",
                    "unece:cefactUNId": "UN01010601",
                    "unece:cefactBieDomainClass": "cefact:DataSet_Version.Details",
                    "rdfs:comment": "The date, time or other date time value from which this data set version is valid."
                }
            ]
        },
        {
            "@id": "fisheries:value",
            "@type": "rdf:Property",
            "schema:rangeIncludes": {
                "@id": "xsd:string"
            },
            "schema:domainIncludes": [
                {
                    "@id": "fisheries:Characteristic"
                },
                {
                    "@id": "fisheries:DataNode"
                }
            ],
            "rdfs:comment": [
                "A value, expressed as text, of this FLUX characteristic.",
                "A value, expressed as text, of this ISR item characteristic.",
                "A value, expressed as text, of this vessel equipment characteristic.",
                "The value, expressed as text, of this MDR element data node.",
                "The value, expressed as text, of this gear characteristic.",
                "The value, expressed as text, of this historical characteristic of a vessel.",
                "The value, expressed as text, of this vessel administrative characteristic.",
                "The value, expressed as text, of this vessel technical characteristic."
            ],
            "rdfs:label": "value",
            "unece:cefactElementMetadata": [
                {
                    "@id": "cefact:MDRElement_DataNode.Value.Text",
                    "@type": "unece:BasicBIE",
                    "unece:cefactUNId": "UN01010597",
                    "unece:cefactBieDomainClass": "cefact:MDRElement_DataNode.Details",
                    "rdfs:comment": "The value, expressed as text, of this MDR element data node."
                },
                {
                    "@id": "cefact:VesselTechnical_Characteristic.Value.Text",
                    "@type": "unece:BasicBIE",
                    "unece:TDED": "7110",
                    "unece:cefactUNId": "UN01010793",
                    "unece:cefactBieDomainClass": "cefact:VesselTechnical_Characteristic.Details",
                    "rdfs:comment": "The value, expressed as text, of this vessel technical characteristic."
                },
                {
                    "@id": "cefact:VesselAdministrative_Characteristic.Value.Text",
                    "@type": "unece:BasicBIE",
                    "unece:TDED": "7110",
                    "unece:cefactUNId": "UN01010704",
                    "unece:cefactBieDomainClass": "cefact:VesselAdministrative_Characteristic.Details",
                    "rdfs:comment": "The value, expressed as text, of this vessel administrative characteristic."
                },
                {
                    "@id": "cefact:FLUX_Characteristic.Value.Text",
                    "@type": "unece:BasicBIE",
                    "unece:TDED": "7110",
                    "unece:cefactUNId": "UN01010872",
                    "unece:cefactBieDomainClass": "cefact:FLUX_Characteristic.Details",
                    "rdfs:comment": "A value, expressed as text, of this FLUX characteristic."
                },
                {
                    "@id": "cefact:Gear_Characteristic.Value.Text",
                    "@type": "unece:BasicBIE",
                    "unece:TDED": "7110",
                    "unece:cefactUNId": "UN01010826",
                    "unece:cefactBieDomainClass": "cefact:Gear_Characteristic.Details",
                    "rdfs:comment": "The value, expressed as text, of this gear characteristic."
                },
                {
                    "@id": "cefact:ISRItem_Characteristic.Value.Text",
                    "@type": "unece:BasicBIE",
                    "unece:cefactUNId": "UN01012609",
                    "unece:cefactBieDomainClass": "cefact:ISRItem_Characteristic.Details",
                    "rdfs:comment": "A value, expressed as text, of this ISR item characteristic."
                },
                {
                    "@id": "cefact:VesselEquipment_Characteristic.Value.Text",
                    "@type": "unece:BasicBIE",
                    "unece:TDED": "7110",
                    "unece:cefactUNId": "UN01010696",
                    "unece:cefactBieDomainClass": "cefact:VesselEquipment_Characteristic.Details",
                    "rdfs:comment": "A value, expressed as text, of this vessel equipment characteristic."
                },
                {
                    "@id": "cefact:VesselHistorical_Characteristic.Value.Text",
                    "@type": "unece:BasicBIE",
                    "unece:TDED": "7110",
                    "unece:cefactUNId": "UN01010653",
                    "unece:cefactBieDomainClass": "cefact:VesselHistorical_Characteristic.Details",
                    "rdfs:comment": "The value, expressed as text, of this historical characteristic of a vessel."
                }
            ]
        },
        {
            "@id": "fisheries:valueBinaryFile",
            "@type": "rdf:Property",
            "schema:rangeIncludes": {
                "@id": "fisheries:BinaryFile"
            },
            "schema:domainIncludes": [
                {
                    "@id": "fisheries:Characteristic"
                },
                {
                    "@id": "fisheries:DataNode"
                }
            ],
            "rdfs:comment": [
                "The value for this gear characteristic expressed in a Fisheries Language for Universal eXchange (FLUX) binary file.",
                "The value for this vessel administrative characteristic, such as a registration certificate, expressed in a Fisheries Language for Universal eXchange (FLUX) binary file.",
                "The value for this vessel equipment characteristic, such as a radio certificate, expressed in a Fisheries Language for Universal eXchange (FLUX) binary file.",
                "The value for this vessel technical characteristic, such as a tonnage certificate, expressed in a Fisheries Language for Universal eXchange (FLUX) binary file.",
                "The value, expressed in a FLUX binary file, for this MDR element data node."
            ],
            "rdfs:label": "valueBinaryFile",
            "unece:cefactElementMetadata": [
                {
                    "@id": "cefact:Gear_Characteristic.Value.FLUX_BinaryFile",
                    "@type": "unece:AssociationBIE",
                    "unece:cefactUNId": "UN01012655",
                    "unece:cefactBieDomainClass": "cefact:Gear_Characteristic.Details",
                    "rdfs:comment": "The value for this gear characteristic expressed in a Fisheries Language for Universal eXchange (FLUX) binary file."
                },
                {
                    "@id": "cefact:VesselAdministrative_Characteristic.Value.FLUX_BinaryFile",
                    "@type": "unece:AssociationBIE",
                    "unece:cefactUNId": "UN01010784",
                    "unece:cefactBieDomainClass": "cefact:VesselAdministrative_Characteristic.Details",
                    "rdfs:comment": "The value for this vessel administrative characteristic, such as a registration certificate, expressed in a Fisheries Language for Universal eXchange (FLUX) binary file."
                },
                {
                    "@id": "cefact:VesselEquipment_Characteristic.Value.FLUX_BinaryFile",
                    "@type": "unece:AssociationBIE",
                    "unece:cefactUNId": "UN01010782",
                    "unece:cefactBieDomainClass": "cefact:VesselEquipment_Characteristic.Details",
                    "rdfs:comment": "The value for this vessel equipment characteristic, such as a radio certificate, expressed in a Fisheries Language for Universal eXchange (FLUX) binary file."
                },
                {
                    "@id": "cefact:MDRElement_DataNode.Value.FLUX_BinaryFile",
                    "@type": "unece:AssociationBIE",
                    "unece:cefactUNId": "UN01010764",
                    "unece:cefactBieDomainClass": "cefact:MDRElement_DataNode.Details",
                    "rdfs:comment": "The value, expressed in a FLUX binary file, for this MDR element data node."
                },
                {
                    "@id": "cefact:VesselTechnical_Characteristic.Value.FLUX_BinaryFile",
                    "@type": "unece:AssociationBIE",
                    "unece:cefactUNId": "UN01010798",
                    "unece:cefactBieDomainClass": "cefact:VesselTechnical_Characteristic.Details",
                    "rdfs:comment": "The value for this vessel technical characteristic, such as a tonnage certificate, expressed in a Fisheries Language for Universal eXchange (FLUX) binary file."
                }
            ]
        },
        {
            "@id": "fisheries:valueCode",
            "@type": "rdf:Property",
            "schema:rangeIncludes": {
                "@id": "xsd:token"
            },
            "schema:domainIncludes": [
                {
                    "@id": "fisheries:Characteristic"
                },
                {
                    "@id": "fisheries:QueryParameter"
                }
            ],
            "rdfs:comment": [
                "The code specifying a value of this ISR item characteristic.",
                "The value, expressed as a code, for this FA query parameter.",
                "The value, expressed as a code, for this ISR query parameter.",
                "The value, expressed as a code, for this sales query parameter."
            ],
            "rdfs:label": "valueCode",
            "unece:cefactElementMetadata": [
                {
                    "@id": "cefact:ISR_QueryParameter.Value.Code",
                    "@type": "unece:BasicBIE",
                    "unece:cefactUNId": "UN01012643",
                    "unece:cefactBieDomainClass": "cefact:ISR_QueryParameter.Details",
                    "rdfs:comment": "The value, expressed as a code, for this ISR query parameter."
                },
                {
                    "@id": "cefact:Sales_QueryParameter.Value.Code",
                    "@type": "unece:BasicBIE",
                    "unece:cefactUNId": "UN01011002",
                    "unece:cefactBieDomainClass": "cefact:Sales_QueryParameter.Details",
                    "rdfs:comment": "The value, expressed as a code, for this sales query parameter."
                },
                {
                    "@id": "cefact:ISRItem_Characteristic.Value.Code",
                    "@type": "unece:BasicBIE",
                    "unece:cefactUNId": "UN01012608",
                    "unece:cefactBieDomainClass": "cefact:ISRItem_Characteristic.Details",
                    "rdfs:comment": "The code specifying a value of this ISR item characteristic."
                },
                {
                    "@id": "cefact:FA_QueryParameter.Value.Code",
                    "@type": "unece:BasicBIE",
                    "unece:cefactUNId": "UN01011226",
                    "unece:cefactBieDomainClass": "cefact:FA_QueryParameter.Details",
                    "rdfs:comment": "The value, expressed as a code, for this FA query parameter."
                }
            ]
        },
        {
            "@id": "fisheries:valueDateTime",
            "@type": "rdf:Property",
            "schema:rangeIncludes": {
                "@id": "xsd:dateTime"
            },
            "schema:domainIncludes": [
                {
                    "@id": "fisheries:Characteristic"
                },
                {
                    "@id": "fisheries:QueryParameter"
                }
            ],
            "rdfs:comment": [
                "The value, expressed as a date, time, date time, or other date time value, for this FA query parameter.",
                "The value, expressed as a date, time, date time, or other date time value, for this ISR query parameter.",
                "The value, expressed as a date, time, date time, or other date time value, for this sales query parameter.",
                "The value, expressed as a date, time, date time, or other date time value, of this FLUX characteristic.",
                "The value, expressed as a date, time, date time, or other date time value, of this ISR item characteristic.",
                "The value, expressed as a date, time, date time, or other date time value, of this gear characteristic.",
                "The value, expressed as a date, time, date time, or other date time value, of this historical characteristic of a vessel.",
                "The value, expressed as a date, time, date time, or other date time value, of this vessel administrative characteristic.",
                "The value, expressed as a date, time, date time, or other date time value, of this vessel equipment characteristic.",
                "The value, expressed as a date, time, date time, or other date time value, of this vessel technical characteristic."
            ],
            "rdfs:label": "valueDateTime",
            "unece:cefactElementMetadata": [
                {
                    "@id": "cefact:FA_QueryParameter.Value.DateTime",
                    "@type": "unece:BasicBIE",
                    "unece:cefactUNId": "UN01011227",
                    "unece:cefactBieDomainClass": "cefact:FA_QueryParameter.Details",
                    "rdfs:comment": "The value, expressed as a date, time, date time, or other date time value, for this FA query parameter."
                },
                {
                    "@id": "cefact:VesselEquipment_Characteristic.Value.DateTime",
                    "@type": "unece:BasicBIE",
                    "unece:cefactUNId": "UN01010698",
                    "unece:cefactBieDomainClass": "cefact:VesselEquipment_Characteristic.Details",
                    "rdfs:comment": "The value, expressed as a date, time, date time, or other date time value, of this vessel equipment characteristic."
                },
                {
                    "@id": "cefact:ISR_QueryParameter.Value.DateTime",
                    "@type": "unece:BasicBIE",
                    "unece:cefactUNId": "UN01012644",
                    "unece:cefactBieDomainClass": "cefact:ISR_QueryParameter.Details",
                    "rdfs:comment": "The value, expressed as a date, time, date time, or other date time value, for this ISR query parameter."
                },
                {
                    "@id": "cefact:VesselAdministrative_Characteristic.Value.DateTime",
                    "@type": "unece:BasicBIE",
                    "unece:cefactUNId": "UN01010706",
                    "unece:cefactBieDomainClass": "cefact:VesselAdministrative_Characteristic.Details",
                    "rdfs:comment": "The value, expressed as a date, time, date time, or other date time value, of this vessel administrative characteristic."
                },
                {
                    "@id": "cefact:VesselTechnical_Characteristic.Value.DateTime",
                    "@type": "unece:BasicBIE",
                    "unece:cefactUNId": "UN01010795",
                    "unece:cefactBieDomainClass": "cefact:VesselTechnical_Characteristic.Details",
                    "rdfs:comment": "The value, expressed as a date, time, date time, or other date time value, of this vessel technical characteristic."
                },
                {
                    "@id": "cefact:Gear_Characteristic.Value.DateTime",
                    "@type": "unece:BasicBIE",
                    "unece:cefactUNId": "UN01010823",
                    "unece:cefactBieDomainClass": "cefact:Gear_Characteristic.Details",
                    "rdfs:comment": "The value, expressed as a date, time, date time, or other date time value, of this gear characteristic."
                },
                {
                    "@id": "cefact:Sales_QueryParameter.Value.DateTime",
                    "@type": "unece:BasicBIE",
                    "unece:cefactUNId": "UN01011003",
                    "unece:cefactBieDomainClass": "cefact:Sales_QueryParameter.Details",
                    "rdfs:comment": "The value, expressed as a date, time, date time, or other date time value, for this sales query parameter."
                },
                {
                    "@id": "cefact:VesselHistorical_Characteristic.Value.DateTime",
                    "@type": "unece:BasicBIE",
                    "unece:cefactUNId": "UN01010656",
                    "unece:cefactBieDomainClass": "cefact:VesselHistorical_Characteristic.Details",
                    "rdfs:comment": "The value, expressed as a date, time, date time, or other date time value, of this historical characteristic of a vessel."
                },
                {
                    "@id": "cefact:FLUX_Characteristic.Value.DateTime",
                    "@type": "unece:BasicBIE",
                    "unece:cefactUNId": "UN01010869",
                    "unece:cefactBieDomainClass": "cefact:FLUX_Characteristic.Details",
                    "rdfs:comment": "The value, expressed as a date, time, date time, or other date time value, of this FLUX characteristic."
                },
                {
                    "@id": "cefact:ISRItem_Characteristic.Value.DateTime",
                    "@type": "unece:BasicBIE",
                    "unece:cefactUNId": "UN01012606",
                    "unece:cefactBieDomainClass": "cefact:ISRItem_Characteristic.Details",
                    "rdfs:comment": "The value, expressed as a date, time, date time, or other date time value, of this ISR item characteristic."
                }
            ]
        },
        {
            "@id": "fisheries:valueId",
            "@type": "rdf:Property",
            "schema:rangeIncludes": {
                "@id": "xsd:token"
            },
            "schema:domainIncludes": {
                "@id": "fisheries:QueryParameter"
            },
            "rdfs:comment": [
                "The value, expressed as an identifier, for this FA query parameter.",
                "The value, expressed as an identifier, for this ISR query parameter.",
                "The value, expressed as an identifier, for this sales query parameter."
            ],
            "rdfs:label": "valueId",
            "unece:cefactElementMetadata": [
                {
                    "@id": "cefact:Sales_QueryParameter.Value.Identifier",
                    "@type": "unece:BasicBIE",
                    "unece:cefactUNId": "UN01011004",
                    "unece:cefactBieDomainClass": "cefact:Sales_QueryParameter.Details",
                    "rdfs:comment": "The value, expressed as an identifier, for this sales query parameter."
                },
                {
                    "@id": "cefact:FA_QueryParameter.Value.Identifier",
                    "@type": "unece:BasicBIE",
                    "unece:cefactUNId": "UN01011228",
                    "unece:cefactBieDomainClass": "cefact:FA_QueryParameter.Details",
                    "rdfs:comment": "The value, expressed as an identifier, for this FA query parameter."
                },
                {
                    "@id": "cefact:ISR_QueryParameter.Value.Identifier",
                    "@type": "unece:BasicBIE",
                    "unece:cefactUNId": "UN01012645",
                    "unece:cefactBieDomainClass": "cefact:ISR_QueryParameter.Details",
                    "rdfs:comment": "The value, expressed as an identifier, for this ISR query parameter."
                }
            ]
        },
        {
            "@id": "fisheries:valueIndicator",
            "@type": "rdf:Property",
            "schema:rangeIncludes": {
                "@id": "xsd:boolean"
            },
            "schema:domainIncludes": {
                "@id": "fisheries:Characteristic"
            },
            "rdfs:comment": [
                "The value, expressed as an indicator, for this FLUX characteristic.",
                "The value, expressed as an indicator, for this ISR item characteristic.",
                "The value, expressed as an indicator, for this gear characteristic.",
                "The value, expressed as an indicator, for this historical characteristic of a vessel .",
                "The value, expressed as an indicator, for this vessel administrative characteristic.",
                "The value, expressed as an indicator, for this vessel equipment characteristic .",
                "The value, expressed as an indicator, for this vessel technical characteristic."
            ],
            "rdfs:label": "valueIndicator",
            "unece:cefactElementMetadata": [
                {
                    "@id": "cefact:ISRItem_Characteristic.Value.Indicator",
                    "@type": "unece:BasicBIE",
                    "unece:cefactUNId": "UN01012607",
                    "unece:cefactBieDomainClass": "cefact:ISRItem_Characteristic.Details",
                    "rdfs:comment": "The value, expressed as an indicator, for this ISR item characteristic."
                },
                {
                    "@id": "cefact:FLUX_Characteristic.Value.Indicator",
                    "@type": "unece:BasicBIE",
                    "unece:cefactUNId": "UN01010870",
                    "unece:cefactBieDomainClass": "cefact:FLUX_Characteristic.Details",
                    "rdfs:comment": "The value, expressed as an indicator, for this FLUX characteristic."
                },
                {
                    "@id": "cefact:Gear_Characteristic.Value.Indicator",
                    "@type": "unece:BasicBIE",
                    "unece:cefactUNId": "UN01010824",
                    "unece:cefactBieDomainClass": "cefact:Gear_Characteristic.Details",
                    "rdfs:comment": "The value, expressed as an indicator, for this gear characteristic."
                },
                {
                    "@id": "cefact:VesselTechnical_Characteristic.Value.Indicator",
                    "@type": "unece:BasicBIE",
                    "unece:cefactUNId": "UN01010796",
                    "unece:cefactBieDomainClass": "cefact:VesselTechnical_Characteristic.Details",
                    "rdfs:comment": "The value, expressed as an indicator, for this vessel technical characteristic."
                },
                {
                    "@id": "cefact:VesselAdministrative_Characteristic.Value.Indicator",
                    "@type": "unece:BasicBIE",
                    "unece:cefactUNId": "UN01010707",
                    "unece:cefactBieDomainClass": "cefact:VesselAdministrative_Characteristic.Details",
                    "rdfs:comment": "The value, expressed as an indicator, for this vessel administrative characteristic."
                },
                {
                    "@id": "cefact:VesselEquipment_Characteristic.Value.Indicator",
                    "@type": "unece:BasicBIE",
                    "unece:cefactUNId": "UN01010699",
                    "unece:cefactBieDomainClass": "cefact:VesselEquipment_Characteristic.Details",
                    "rdfs:comment": "The value, expressed as an indicator, for this vessel equipment characteristic ."
                },
                {
                    "@id": "cefact:VesselHistorical_Characteristic.Value.Indicator",
                    "@type": "unece:BasicBIE",
                    "unece:cefactUNId": "UN01010654",
                    "unece:cefactBieDomainClass": "cefact:VesselHistorical_Characteristic.Details",
                    "rdfs:comment": "The value, expressed as an indicator, for this historical characteristic of a vessel ."
                }
            ]
        },
        {
            "@id": "fisheries:valueMeasure",
            "@type": "rdf:Property",
            "schema:rangeIncludes": {
                "@id": "xsd:decimal"
            },
            "schema:domainIncludes": [
                {
                    "@id": "fisheries:Characteristic"
                },
                {
                    "@id": "fisheries:Dimension"
                }
            ],
            "rdfs:comment": [
                "A measure of a value for this fish catch characteristic.",
                "The measure of the value for this historical characteristic of a vessel.",
                "The measure of the value for this vessel dimension.",
                "The value, expressed as a measure, for this FLUX characteristic.",
                "The value, expressed as a measure, for this ISR item characteristic.",
                "The value, expressed as a measure, for this gear characteristic.",
                "The value, expressed as a measure, for this vessel administrative characteristic.",
                "The value, expressed as a measure, for this vessel equipment characteristic.",
                "The value, expressed as a measure, for this vessel technical characteristic."
            ],
            "rdfs:label": "valueMeasure",
            "unece:cefactElementMetadata": [
                {
                    "@id": "cefact:Gear_Characteristic.Value.Measure",
                    "@type": "unece:BasicBIE",
                    "unece:cefactUNId": "UN01010822",
                    "unece:cefactBieDomainClass": "cefact:Gear_Characteristic.Details",
                    "rdfs:comment": "The value, expressed as a measure, for this gear characteristic."
                },
                {
                    "@id": "cefact:VesselAdministrative_Characteristic.Value.Measure",
                    "@type": "unece:BasicBIE",
                    "unece:cefactUNId": "UN01010703",
                    "unece:cefactBieDomainClass": "cefact:VesselAdministrative_Characteristic.Details",
                    "rdfs:comment": "The value, expressed as a measure, for this vessel administrative characteristic."
                },
                {
                    "@id": "cefact:ISRItem_Characteristic.Value.Measure",
                    "@type": "unece:BasicBIE",
                    "unece:cefactUNId": "UN01012605",
                    "unece:cefactBieDomainClass": "cefact:ISRItem_Characteristic.Details",
                    "rdfs:comment": "The value, expressed as a measure, for this ISR item characteristic."
                },
                {
                    "@id": "cefact:Vessel_Dimension.Value.Measure",
                    "@type": "unece:BasicBIE",
                    "unece:cefactUNId": "UN01010691",
                    "unece:cefactBieDomainClass": "cefact:Vessel_Dimension.Details",
                    "rdfs:comment": "The measure of the value for this vessel dimension."
                },
                {
                    "@id": "cefact:FLUX_Characteristic.Value.Measure",
                    "@type": "unece:BasicBIE",
                    "unece:cefactUNId": "UN01010868",
                    "unece:cefactBieDomainClass": "cefact:FLUX_Characteristic.Details",
                    "rdfs:comment": "The value, expressed as a measure, for this FLUX characteristic."
                },
                {
                    "@id": "cefact:FishCatch_Characteristic.Value.Measure",
                    "@type": "unece:BasicBIE",
                    "unece:cefactUNId": "UN01011284",
                    "unece:cefactBieDomainClass": "cefact:FishCatch_Characteristic.Details",
                    "rdfs:comment": "A measure of a value for this fish catch characteristic."
                },
                {
                    "@id": "cefact:VesselHistorical_Characteristic.Value.Measure",
                    "@type": "unece:BasicBIE",
                    "unece:cefactUNId": "UN01010657",
                    "unece:cefactBieDomainClass": "cefact:VesselHistorical_Characteristic.Details",
                    "rdfs:comment": "The measure of the value for this historical characteristic of a vessel."
                },
                {
                    "@id": "cefact:VesselTechnical_Characteristic.Value.Measure",
                    "@type": "unece:BasicBIE",
                    "unece:cefactUNId": "UN01010792",
                    "unece:cefactBieDomainClass": "cefact:VesselTechnical_Characteristic.Details",
                    "rdfs:comment": "The value, expressed as a measure, for this vessel technical characteristic."
                },
                {
                    "@id": "cefact:VesselEquipment_Characteristic.Value.Measure",
                    "@type": "unece:BasicBIE",
                    "unece:cefactUNId": "UN01010695",
                    "unece:cefactBieDomainClass": "cefact:VesselEquipment_Characteristic.Details",
                    "rdfs:comment": "The value, expressed as a measure, for this vessel equipment characteristic."
                }
            ]
        },
        {
            "@id": "fisheries:valueNumeric",
            "@type": "rdf:Property",
            "schema:rangeIncludes": {
                "@id": "xsd:decimal"
            },
            "schema:domainIncludes": {
                "@id": "fisheries:Characteristic"
            },
            "rdfs:comment": "The value, expressed as a number, for this ISR item characteristic.",
            "rdfs:label": "valueNumeric",
            "unece:cefactElementMetadata": [
                {
                    "@id": "cefact:ISRItem_Characteristic.Value.Numeric",
                    "@type": "unece:BasicBIE",
                    "unece:cefactUNId": "UN01012611",
                    "unece:cefactBieDomainClass": "cefact:ISRItem_Characteristic.Details",
                    "rdfs:comment": "The value, expressed as a number, for this ISR item characteristic."
                }
            ]
        },
        {
            "@id": "fisheries:valueQuantity",
            "@type": "rdf:Property",
            "schema:rangeIncludes": {
                "@id": "xsd:decimal"
            },
            "schema:domainIncludes": {
                "@id": "fisheries:Characteristic"
            },
            "rdfs:comment": [
                "The value, expressed as a quantity, for this FLUX characteristic.",
                "The value, expressed as a quantity, for this ISR item characteristic.",
                "The value, expressed as a quantity, for this gear characteristic.",
                "The value, expressed as a quantity, for this historical characteristic of a vessel.",
                "The value, expressed as a quantity, for this vessel administrative characteristic.",
                "The value, expressed as a quantity, for this vessel equipment characteristic.",
                "The value, expressed as a quantity, for this vessel technical characteristic."
            ],
            "rdfs:label": "valueQuantity",
            "unece:cefactElementMetadata": [
                {
                    "@id": "cefact:VesselTechnical_Characteristic.Value.Quantity",
                    "@type": "unece:BasicBIE",
                    "unece:cefactUNId": "UN01010797",
                    "unece:cefactBieDomainClass": "cefact:VesselTechnical_Characteristic.Details",
                    "rdfs:comment": "The value, expressed as a quantity, for this vessel technical characteristic."
                },
                {
                    "@id": "cefact:FLUX_Characteristic.Value.Quantity",
                    "@type": "unece:BasicBIE",
                    "unece:cefactUNId": "UN01010873",
                    "unece:cefactBieDomainClass": "cefact:FLUX_Characteristic.Details",
                    "rdfs:comment": "The value, expressed as a quantity, for this FLUX characteristic."
                },
                {
                    "@id": "cefact:VesselHistorical_Characteristic.Value.Quantity",
                    "@type": "unece:BasicBIE",
                    "unece:cefactUNId": "UN01010768",
                    "unece:cefactBieDomainClass": "cefact:VesselHistorical_Characteristic.Details",
                    "rdfs:comment": "The value, expressed as a quantity, for this historical characteristic of a vessel."
                },
                {
                    "@id": "cefact:ISRItem_Characteristic.Value.Quantity",
                    "@type": "unece:BasicBIE",
                    "unece:cefactUNId": "UN01012610",
                    "unece:cefactBieDomainClass": "cefact:ISRItem_Characteristic.Details",
                    "rdfs:comment": "The value, expressed as a quantity, for this ISR item characteristic."
                },
                {
                    "@id": "cefact:VesselEquipment_Characteristic.Value.Quantity",
                    "@type": "unece:BasicBIE",
                    "unece:cefactUNId": "UN01010781",
                    "unece:cefactBieDomainClass": "cefact:VesselEquipment_Characteristic.Details",
                    "rdfs:comment": "The value, expressed as a quantity, for this vessel equipment characteristic."
                },
                {
                    "@id": "cefact:Gear_Characteristic.Value.Quantity",
                    "@type": "unece:BasicBIE",
                    "unece:cefactUNId": "UN01010827",
                    "unece:cefactBieDomainClass": "cefact:Gear_Characteristic.Details",
                    "rdfs:comment": "The value, expressed as a quantity, for this gear characteristic."
                },
                {
                    "@id": "cefact:VesselAdministrative_Characteristic.Value.Quantity",
                    "@type": "unece:BasicBIE",
                    "unece:cefactUNId": "UN01010783",
                    "unece:cefactBieDomainClass": "cefact:VesselAdministrative_Characteristic.Details",
                    "rdfs:comment": "The value, expressed as a quantity, for this vessel administrative characteristic."
                }
            ]
        },
        {
            "@id": "fisheries:vehicleTransportMeansTypeCode",
            "@type": "rdf:Property",
            "schema:rangeIncludes": {
                "@id": "unece:UNECECL8179Code"
            },
            "schema:domainIncludes": {
                "@id": "fisheries:TransportMeans"
            },
            "rdfs:comment": "The code specifying a type of vehicle transport means.",
            "rdfs:label": "vehicleTransportMeansTypeCode",
            "unece:cefactElementMetadata": [
                {
                    "@id": "cefact:Vehicle_TransportMeans.Type.Code",
                    "@type": "unece:BasicBIE",
                    "unece:TDED": "8179",
                    "unece:cefactUNId": "UN01010991",
                    "unece:cefactBieDomainClass": "cefact:Vehicle_TransportMeans.Details",
                    "rdfs:comment": "The code specifying a type of vehicle transport means."
                }
            ]
        },
        {
            "@id": "fisheries:versionId",
            "@type": "rdf:Property",
            "schema:rangeIncludes": {
                "@id": "xsd:token"
            },
            "schema:domainIncludes": {
                "@id": "fisheries:Identity"
            },
            "rdfs:comment": "The identifier of the version of this MDR query identity.",
            "rdfs:label": "versionId",
            "unece:cefactElementMetadata": [
                {
                    "@id": "cefact:MDRQuery_Identity.Version.Identifier",
                    "@type": "unece:BasicBIE",
                    "unece:cefactUNId": "UN01010580",
                    "unece:cefactBieDomainClass": "cefact:MDRQuery_Identity.Details",
                    "rdfs:comment": "The identifier of the version of this MDR query identity."
                }
            ]
        },
        {
            "@id": "fisheries:vesselAdministrativeCharacteristicValueCode",
            "@type": "rdf:Property",
            "schema:rangeIncludes": {
                "@id": "unece:UNECECL7111Code"
            },
            "schema:domainIncludes": {
                "@id": "fisheries:Characteristic"
            },
            "rdfs:comment": "The code specifying a value of this vessel administrative characteristic.",
            "rdfs:label": "vesselAdministrativeCharacteristicValueCode",
            "unece:cefactElementMetadata": [
                {
                    "@id": "cefact:VesselAdministrative_Characteristic.Value.Code",
                    "@type": "unece:BasicBIE",
                    "unece:TDED": "7111",
                    "unece:cefactUNId": "UN01010705",
                    "unece:cefactBieDomainClass": "cefact:VesselAdministrative_Characteristic.Details",
                    "rdfs:comment": "The code specifying a value of this vessel administrative characteristic."
                }
            ]
        },
        {
            "@id": "fisheries:vesselDimensionTypeCode",
            "@type": "rdf:Property",
            "schema:rangeIncludes": {
                "@id": "unece:UNECECL6145Code"
            },
            "schema:domainIncludes": {
                "@id": "fisheries:Dimension"
            },
            "rdfs:comment": "The code specifying a type of dimension of this vessel.",
            "rdfs:label": "vesselDimensionTypeCode",
            "unece:cefactElementMetadata": [
                {
                    "@id": "cefact:Vessel_Dimension.Type.Code",
                    "@type": "unece:BasicBIE",
                    "unece:TDED": "6145",
                    "unece:cefactUNId": "UN01010690",
                    "unece:cefactBieDomainClass": "cefact:Vessel_Dimension.Details",
                    "rdfs:comment": "The code specifying a type of dimension of this vessel."
                }
            ]
        },
        {
            "@id": "fisheries:vesselEquipmentCharacteristicValueCode",
            "@type": "rdf:Property",
            "schema:rangeIncludes": {
                "@id": "unece:UNECECL7111Code"
            },
            "schema:domainIncludes": {
                "@id": "fisheries:Characteristic"
            },
            "rdfs:comment": "A code specifying a value of this vessel equipment characteristic.",
            "rdfs:label": "vesselEquipmentCharacteristicValueCode",
            "unece:cefactElementMetadata": [
                {
                    "@id": "cefact:VesselEquipment_Characteristic.Value.Code",
                    "@type": "unece:BasicBIE",
                    "unece:TDED": "7111",
                    "unece:cefactUNId": "UN01010697",
                    "unece:cefactBieDomainClass": "cefact:VesselEquipment_Characteristic.Details",
                    "rdfs:comment": "A code specifying a value of this vessel equipment characteristic."
                }
            ]
        },
        {
            "@id": "fisheries:vesselHistoricalCharacteristicValueCode",
            "@type": "rdf:Property",
            "schema:rangeIncludes": {
                "@id": "unece:UNECECL7111Code"
            },
            "schema:domainIncludes": {
                "@id": "fisheries:Characteristic"
            },
            "rdfs:comment": "The code specifying a value of this historical characteristic of a vessel.",
            "rdfs:label": "vesselHistoricalCharacteristicValueCode",
            "unece:cefactElementMetadata": [
                {
                    "@id": "cefact:VesselHistorical_Characteristic.Value.Code",
                    "@type": "unece:BasicBIE",
                    "unece:TDED": "7111",
                    "unece:cefactUNId": "UN01010655",
                    "unece:cefactBieDomainClass": "cefact:VesselHistorical_Characteristic.Details",
                    "rdfs:comment": "The code specifying a value of this historical characteristic of a vessel."
                }
            ]
        },
        {
            "@id": "fisheries:vesselId",
            "@type": "rdf:Property",
            "schema:rangeIncludes": {
                "@id": "xsd:token"
            },
            "schema:domainIncludes": [
                {
                    "@id": "fisheries:Document"
                },
                {
                    "@id": "fisheries:Event"
                },
                {
                    "@id": "fisheries:Identity"
                }
            ],
            "rdfs:comment": [
                "A vessel identifier for this vessel identity, such as an identifier defined by the Food and Agriculture Organisation (FAO), the radio call sign, or an external marking.",
                "A vessel identifier, such as an identifier defined by the Food and Agriculture Organization (FAO), the radio call sign, or an external marking, for this FLAP document.",
                "The vessel identifier for this event."
            ],
            "rdfs:label": "vesselId",
            "unece:cefactElementMetadata": [
                {
                    "@id": "cefact:FLAP_Document.Vessel_Identification.Identifier",
                    "@type": "unece:BasicBIE",
                    "unece:TDED": "8313",
                    "unece:cefactUNId": "UN01010847",
                    "unece:cefactBieDomainClass": "cefact:FLAP_Document.Details",
                    "rdfs:comment": "A vessel identifier, such as an identifier defined by the Food and Agriculture Organization (FAO), the radio call sign, or an external marking, for this FLAP document."
                },
                {
                    "@id": "cefact:Vessel_Event.Vessel_Identification.Identifier",
                    "@type": "unece:BasicBIE",
                    "unece:TDED": "1007",
                    "unece:cefactUNId": "UN01010659",
                    "unece:cefactBieDomainClass": "cefact:Vessel_Event.Details",
                    "rdfs:comment": "The vessel identifier for this event."
                },
                {
                    "@id": "cefact:Vessel_Identity.Vessel_Identification.Identifier",
                    "@type": "unece:BasicBIE",
                    "unece:cefactUNId": "UN01010744",
                    "unece:cefactBieDomainClass": "cefact:Vessel_Identity.Details",
                    "rdfs:comment": "A vessel identifier for this vessel identity, such as an identifier defined by the Food and Agriculture Organisation (FAO), the radio call sign, or an external marking."
                }
            ]
        },
        {
            "@id": "fisheries:vesselName",
            "@type": "rdf:Property",
            "schema:rangeIncludes": {
                "@id": "xsd:string"
            },
            "schema:domainIncludes": {
                "@id": "fisheries:Identity"
            },
            "rdfs:comment": "A vessel name, expressed as a text, for this vessel identity.",
            "rdfs:label": "vesselName",
            "unece:cefactElementMetadata": [
                {
                    "@id": "cefact:Vessel_Identity.Vessel_Name.Text",
                    "@type": "unece:BasicBIE",
                    "unece:cefactUNId": "UN01010745",
                    "unece:cefactBieDomainClass": "cefact:Vessel_Identity.Details",
                    "rdfs:comment": "A vessel name, expressed as a text, for this vessel identity."
                }
            ]
        },
        {
            "@id": "fisheries:vesselRegistrationCountryId",
            "@type": "rdf:Property",
            "schema:rangeIncludes": {
                "@id": "xsd:token"
            },
            "schema:domainIncludes": {
                "@id": "fisheries:Identity"
            },
            "rdfs:comment": "The identifier of the registration country for this vessel identity.",
            "rdfs:label": "vesselRegistrationCountryId",
            "unece:cefactElementMetadata": [
                {
                    "@id": "cefact:Vessel_Identity.VesselRegistrationCountry_Identification.Identifier",
                    "@type": "unece:BasicBIE",
                    "unece:cefactUNId": "UN01010746",
                    "unece:cefactBieDomainClass": "cefact:Vessel_Identity.Details",
                    "rdfs:comment": "The identifier of the registration country for this vessel identity."
                }
            ]
        },
        {
            "@id": "fisheries:vesselRelatedActivityCode",
            "@type": "rdf:Property",
            "schema:rangeIncludes": {
                "@id": "xsd:token"
            },
            "schema:domainIncludes": {
                "@id": "fisheries:Activity"
            },
            "rdfs:comment": "The code specifying a related activity of a vessel, such as searching for fish or trawling, for this fishing activity.",
            "rdfs:label": "vesselRelatedActivityCode",
            "unece:cefactElementMetadata": [
                {
                    "@id": "cefact:Fishing_Activity.Vessel_RelatedActivity.Code",
                    "@type": "unece:BasicBIE",
                    "unece:cefactUNId": "UN01011173",
                    "unece:cefactBieDomainClass": "cefact:Fishing_Activity.Details",
                    "rdfs:comment": "The code specifying a related activity of a vessel, such as searching for fish or trawling, for this fishing activity."
                }
            ]
        },
        {
            "@id": "fisheries:vesselTechnicalCharacteristicValueCode",
            "@type": "rdf:Property",
            "schema:rangeIncludes": {
                "@id": "unece:UNECECL7111Code"
            },
            "schema:domainIncludes": {
                "@id": "fisheries:Characteristic"
            },
            "rdfs:comment": "The code specifying a value of this vessel technical characteristic.",
            "rdfs:label": "vesselTechnicalCharacteristicValueCode",
            "unece:cefactElementMetadata": [
                {
                    "@id": "cefact:VesselTechnical_Characteristic.Value.Code",
                    "@type": "unece:BasicBIE",
                    "unece:TDED": "7111",
                    "unece:cefactUNId": "UN01010794",
                    "unece:cefactBieDomainClass": "cefact:VesselTechnical_Characteristic.Details",
                    "rdfs:comment": "The code specifying a value of this vessel technical characteristic."
                }
            ]
        },
        {
            "@id": "fisheries:vesselTransportMeansTypeCode",
            "@type": "rdf:Property",
            "schema:rangeIncludes": {
                "@id": "unece:UNECECL8179Code"
            },
            "schema:domainIncludes": {
                "@id": "fisheries:TransportMeans"
            },
            "rdfs:comment": "A code specifying a type of vessel transport means.",
            "rdfs:label": "vesselTransportMeansTypeCode",
            "unece:cefactElementMetadata": [
                {
                    "@id": "cefact:Vessel_TransportMeans.Type.Code",
                    "@type": "unece:BasicBIE",
                    "unece:TDED": "8179",
                    "unece:cefactUNId": "UN01010636",
                    "unece:cefactBieDomainClass": "cefact:Vessel_TransportMeans.Details",
                    "rdfs:comment": "A code specifying a type of vessel transport means."
                }
            ]
        },
        {
            "@id": "fisheries:vesselTypeCode",
            "@type": "rdf:Property",
            "schema:rangeIncludes": {
                "@id": "xsd:token"
            },
            "schema:domainIncludes": {
                "@id": "fisheries:Identity"
            },
            "rdfs:comment": "The code specifying the type of vessel for this vessel identity.",
            "rdfs:label": "vesselTypeCode",
            "unece:cefactElementMetadata": [
                {
                    "@id": "cefact:Vessel_Identity.Vessel_Type.Code",
                    "@type": "unece:BasicBIE",
                    "unece:cefactUNId": "UN01010747",
                    "unece:cefactBieDomainClass": "cefact:Vessel_Identity.Details",
                    "rdfs:comment": "The code specifying the type of vessel for this vessel identity."
                }
            ]
        },
        {
            "@id": "fisheries:weighingMeansCode",
            "@type": "rdf:Property",
            "schema:rangeIncludes": {
                "@id": "xsd:token"
            },
            "schema:domainIncludes": [
                {
                    "@id": "fisheries:Catch"
                },
                {
                    "@id": "fisheries:Product"
                }
            ],
            "rdfs:comment": [
                "The code specifying the means of weighing for this AAP product.",
                "The code specifying the means of weighing for this FA catch."
            ],
            "rdfs:label": "weighingMeansCode",
            "unece:cefactElementMetadata": [
                {
                    "@id": "cefact:AAP_Product.WeighingMeans.Code",
                    "@type": "unece:BasicBIE",
                    "unece:cefactUNId": "UN01010937",
                    "unece:cefactBieDomainClass": "cefact:AAP_Product.Details",
                    "rdfs:comment": "The code specifying the means of weighing for this AAP product."
                },
                {
                    "@id": "cefact:FA_Catch.WeighingMeans.Code",
                    "@type": "unece:BasicBIE",
                    "unece:cefactUNId": "UN01010975",
                    "unece:cefactBieDomainClass": "cefact:FA_Catch.Details",
                    "rdfs:comment": "The code specifying the means of weighing for this FA catch."
                }
            ]
        },
        {
            "@id": "fisheries:weightMeasure",
            "@type": "rdf:Property",
            "schema:rangeIncludes": {
                "@id": "xsd:decimal"
            },
            "schema:domainIncludes": [
                {
                    "@id": "fisheries:Catch"
                },
                {
                    "@id": "fisheries:Product"
                },
                {
                    "@id": "fisheries:Quota"
                }
            ],
            "rdfs:comment": [
                "A measure of the weight for this targeted quota.",
                "The measure of the weight of this AAP product.",
                "The measure of the weight of this ACDR catch.",
                "The measure of the weight of this FA catch."
            ],
            "rdfs:label": "weightMeasure",
            "unece:cefactElementMetadata": [
                {
                    "@id": "cefact:ACDR_Catch.Weight.Measure",
                    "@type": "unece:BasicBIE",
                    "unece:cefactUNId": "UN01010267",
                    "unece:cefactBieDomainClass": "cefact:ACDR_Catch.Details",
                    "rdfs:comment": "The measure of the weight of this ACDR catch."
                },
                {
                    "@id": "cefact:Targeted_Quota.Weight.Measure",
                    "@type": "unece:BasicBIE",
                    "unece:cefactUNId": "UN01010881",
                    "unece:cefactBieDomainClass": "cefact:Targeted_Quota.Details",
                    "rdfs:comment": "A measure of the weight for this targeted quota."
                },
                {
                    "@id": "cefact:AAP_Product.Weight.Measure",
                    "@type": "unece:BasicBIE",
                    "unece:cefactUNId": "UN01010936",
                    "unece:cefactBieDomainClass": "cefact:AAP_Product.Details",
                    "rdfs:comment": "The measure of the weight of this AAP product."
                },
                {
                    "@id": "cefact:FA_Catch.Weight.Measure",
                    "@type": "unece:BasicBIE",
                    "unece:cefactUNId": "UN01010974",
                    "unece:cefactBieDomainClass": "cefact:FA_Catch.Details",
                    "rdfs:comment": "The measure of the weight of this FA catch."
                }
            ]
        }
    ]
}